redo foundations

Computability/SingleOracle/Encoding.lean
@@ -13,17 +13,41 @@ open Denumerable Encodable
 -- This section provides and encoding for oracle partial recursive functions and a definition
 -- of the universal partial recursive function relative to an oracle, along with a proof that it is universal.
 
-variable {α : Type} [Denumerable α]
+-- variable {α : Type} [Denumerable α]
+
+
+
 
 theorem RecursiveIn.rfind' {f : ℕ →. ℕ} (hf : RecursiveIn O f) :
   RecursiveIn O (Nat.unpaired fun a m =>
     (Nat.rfind fun n => (fun m => m = 0) <$> f (Nat.pair a (n + m))).map (· + m))
   := by sorry
+-- theorem rfind' {f} (hf : Nat.Partrec f) :
+--     Nat.Partrec
+--       (Nat.unpaired fun a m =>
+--         (Nat.rfind fun n => (fun m => m = 0) <$> f (Nat.pair a (n + m))).map (· + m)) :=
+-- theorem RecursiveIn.rfind' {f : ℕ →. ℕ} (hf : RecursiveIn O f) :
+--   RecursiveIn O (Nat.unpaired fun a m =>
+--     (Nat.rfind fun n => (fun m => m = 0) <$> f (Nat.pair a (n + m))).map (· + m))
+--   :=
+--   RecursiveIn₂.unpaired'.2 <| by
+--     refine
+--       Partrec.map
+--         ((@Partrec₂.unpaired' fun a b : ℕ =>
+--               Nat.rfind fun n => (fun m => m = 0) <$> f (Nat.pair a (n + b))).1
+--           ?_)
+--         (Primrec.nat_add.comp Primrec.snd <| Primrec.snd.comp Primrec.fst).to_comp.to₂
+--     have : Nat.Partrec (fun a => Nat.rfind (fun n => (fun m => decide (m = 0)) <$>
+--       Nat.unpaired (fun a b => f (Nat.pair (Nat.unpair a).1 (b + (Nat.unpair a).2)))
+--         (Nat.pair a n))) :=
+--       rfind
+--         (Partrec₂.unpaired'.2
+--           ((Partrec.nat_iff.2 hf).comp
+--               (Primrec₂.pair.comp (Primrec.fst.comp <| Primrec.unpair.comp Primrec.fst)
+--                   (Primrec.nat_add.comp Primrec.snd
+--                     (Primrec.snd.comp <| Primrec.unpair.comp Primrec.fst))).to_comp))
+--     simpa
 
-def oracleCode (f : α → ℕ →. ℕ) : ℕ → ℕ →. ℕ :=
-  λ i n => match decode i with
-           | some a => f a n
-           | none   => ⊥
 
 inductive codeo : Type
 | zero : codeo
@@ -36,9 +60,7 @@ inductive codeo : Type
 | prec : codeo → codeo → codeo
 | rfind' : codeo → codeo
 
--- instance Primcodable.codeo : Primcodable codeo := by
---   exact?
-
+namespace Nat.OracleComp.Code
 
 /-- Semantics of `codeo`, relative to an indexed oracle family. -/
 def evalo (O : ℕ →. ℕ) : codeo → ℕ →. ℕ
@@ -113,7 +135,6 @@ instance : Coe codeo ℕ := ⟨encodeCodeo⟩
 
 @[simp] theorem decodeCodeo_encodeCodeo : ∀ c, decodeCodeo (encodeCodeo c) = c := fun c => by
   induction c <;> (simp [encodeCodeo, decodeCodeo, Nat.div2_val, *])
-
 @[simp] theorem encodeCodeo_decodeCodeo : ∀ c, encodeCodeo (decodeCodeo c) = c :=
 λ c => match c with
   | 0 => by simp only [decodeCodeo, encodeCodeo]
@@ -134,7 +155,6 @@ instance : Coe codeo ℕ := ⟨encodeCodeo⟩
     conv_rhs => rw [← Nat.bit_decomp n, ← Nat.bit_decomp n.div2]
     simp only [decodeCodeo.eq_6]
     cases n.bodd <;> cases n.div2.bodd <;> simp [m, encodeCodeo, IH, IH1, IH2, Nat.bit_val]
-
 instance instDenumerable : Denumerable codeo := mk' ⟨encodeCodeo, decodeCodeo, decodeCodeo_encodeCodeo, encodeCodeo_decodeCodeo⟩
 
 /-- Returns a code for the constant function outputting a particular natural. -/
@@ -152,13 +172,13 @@ def const_inj : ∀ {n₁ n₂}, codeo_const n₁ = codeo_const n₂ → n₁ = 
 theorem evalo_const (g : ℕ →. ℕ) : evalo g (codeo_const a) _b = a := by sorry
 
 /-- A code for the identity function. -/
-def id_code : codeo :=
+def id : codeo :=
   codeo.pair codeo.left codeo.right
 
 /-- Given a code `c` taking a pair as input, returns a code using `n` as the first argument to `c`.
 -/
 def curry (c : codeo) (n : ℕ) : codeo :=
-  codeo.comp c (codeo.pair (codeo_const n) id_code)
+  codeo.comp c (codeo.pair (codeo_const n) id)
 
 -- -- helper lemma to prove rfind' case of univ theorem, since rfind' is defined differently from rfind
 theorem rfind'o {g : ℕ →. ℕ} {cf : codeo}
@@ -169,6 +189,41 @@ theorem rfind'o {g : ℕ →. ℕ} {cf : codeo}
         (fun m => m = 0) <$> evalo g cf (Nat.pair a (n + m))
       ).map (· + m))
  := sorry
+
+open Nat.Partrec.Code in
+theorem exists_code {f : ℕ →. ℕ} : Nat.Partrec f ↔ ∃ c : Partrec.Code, eval c = f := by
+  refine ⟨fun h => ?_, ?_⟩
+  · induction h with
+    | zero => exact ⟨Nat.Partrec.Code.zero, rfl⟩
+    | succ => exact ⟨Nat.Partrec.Code.succ, rfl⟩
+    | left => exact ⟨left, rfl⟩
+    | right => exact ⟨right, rfl⟩
+    | pair pf pg hf hg =>
+      rcases hf with ⟨cf, rfl⟩; rcases hg with ⟨cg, rfl⟩
+      exact ⟨Nat.Partrec.Code.pair cf cg, rfl⟩
+    | comp pf pg hf hg =>
+      rcases hf with ⟨cf, rfl⟩; rcases hg with ⟨cg, rfl⟩
+      exact ⟨Nat.Partrec.Code.comp cf cg, rfl⟩
+    | prec pf pg hf hg =>
+      rcases hf with ⟨cf, rfl⟩; rcases hg with ⟨cg, rfl⟩
+      exact ⟨prec cf cg, rfl⟩
+    | rfind pf hf =>
+      rcases hf with ⟨cf, rfl⟩
+      refine ⟨Nat.Partrec.Code.comp (Nat.Partrec.Code.rfind' cf) (Nat.Partrec.Code.pair Nat.Partrec.Code.id Nat.Partrec.Code.zero), ?_⟩
+      -- simp [eval, Seq.seq, pure, PFun.pure, Part.map_id']
+      simp only [eval]
+      simp
+      sorry
+  · rintro ⟨c, rfl⟩
+    induction c with
+    | zero => exact Nat.Partrec.zero
+    | succ => exact Nat.Partrec.succ
+    | left => exact Nat.Partrec.left
+    | right => exact Nat.Partrec.right
+    | pair cf cg pf pg => exact pf.pair pg
+    | comp cf cg pf pg => exact pf.comp pg
+    | prec cf cg pf pg => exact pf.prec pg
+    | rfind' cf pf => exact pf.rfind'
 
 /-- A function is partial recursive relative to an indexed set of oracles `O` if and only if there is a code implementing it.
 Therefore, `evalo` is a **universal partial recursive function relative to `g`**. -/
@@ -181,13 +236,7 @@ theorem exists_code_rel (O : ℕ →. ℕ) (f : ℕ →. ℕ) :
     · exact ⟨codeo.succ, rfl⟩
     · exact ⟨codeo.left, rfl⟩
     · exact ⟨codeo.right, rfl⟩
-    · sorry
-    -- · case mp.oracle hf =>
-    --   rcases hf with ⟨cf, rfl⟩
-    --   exact ⟨codeo.oracle (encode cf), by
-    --     funext n
-    --     simp only [evalo, codeo.oracle]
-    --     rw [encodek]⟩
+    · exact ⟨codeo.oracle, rfl⟩
     · case mp.pair hf hg =>
       rcases hf with ⟨cf, rfl⟩; rcases hg with ⟨cg, rfl⟩
       exact ⟨codeo.pair cf cg, rfl⟩
@@ -198,9 +247,17 @@ theorem exists_code_rel (O : ℕ →. ℕ) (f : ℕ →. ℕ) :
       rcases hf with ⟨cf, rfl⟩; rcases hg with ⟨cg, rfl⟩
       exact ⟨codeo.prec cf cg, rfl⟩
     · case mp.rfind f' pf hf =>
-      rcases hf with ⟨cg, h⟩
-      use (cg.rfind'.comp (id_code.pair codeo.zero))
-      simp [evalo]
+
+      rcases hf with ⟨cf, rfl⟩
+      refine ⟨codeo.comp (codeo.rfind' cf) (pair id zero), ?_⟩
+      -- simp [evalo, Seq.seq, pure, PFun.pure, Part.map_id']
+      simp only [evalo]
+
+      -- rcases hf with ⟨cg, h⟩
+      -- use (cg.rfind'.comp (id.pair codeo.zero))
+      -- simp [evalo]
+      -- simp [Seq.seq, pure, PFun.pure, Part.map_id']
+      -- simp [*]
       sorry
   · rintro ⟨c, rfl⟩
     induction c with
