Computability/SingleOracle/Encoding2.checkpoint.lean
@@ -1,92 +1,61 @@
-/-
-Copyright (c) 2018 Mario Carneiro. All rights reserved.
-Released under Apache 2.0 license as described in the file LICENSE.
-Authors: Mario Carneiro
--/
-import Mathlib.Computability.Partrec
+import Computability.SingleOracle.TuringDegree
+import Computability.SingleOracle.PrimrecIn
+-- import Mathlib.Computability.RecursiveIn O
 import Mathlib.Data.Option.Basic
 
-set_option maxHeartbeats 20000000
+-- set_option maxHeartbeats 20000000
 
-/-!
-# Gödel Numbering for Partial Recursive Functions.
 
-This file defines `Nat.Partrec.Code`, an inductive datatype describing code for partial
-recursive functions on ℕ. It defines an encoding for these codes, and proves that the constructors
-are primitive recursive with respect to the encoding.
-
-It also defines the evaluation of these codes as partial functions using `PFun`, and proves that a
-function is partially recursive (as defined by `Nat.Partrec`) if and only if it is the evaluation
-of some code.
-
-## Main Definitions
-
-* `Nat.Partrec.Code`: Inductive datatype for partial recursive codes.
-* `Nat.Partrec.Code.encodeCode`: A (computable) encoding of codes as natural numbers.
-* `Nat.Partrec.Code.ofNatCode`: The inverse of this encoding.
-* `Nat.Partrec.Code.eval`: The interpretation of a `Nat.Partrec.Code` as a partial function.
-
-## Main Results
-
-* `Nat.Partrec.Code.rec_prim`: Recursion on `Nat.Partrec.Code` is primitive recursive.
-* `Nat.Partrec.Code.rec_computable`: Recursion on `Nat.Partrec.Code` is computable.
-* `Nat.Partrec.Code.smn`: The $S_n^m$ theorem.
-* `Nat.Partrec.Code.exists_code`: Partial recursiveness is equivalent to being the eval of a code.
-* `Nat.Partrec.Code.evaln_prim`: `evaln` is primitive recursive.
-* `Nat.Partrec.Code.fixed_point`: Roger's fixed point theorem.
-* `Nat.Partrec.Code.fixed_point₂`: Kleene's second recursion theorem.
-
-## References
-
-* [Mario Carneiro, *Formalizing computability theory via partial recursive functions*][carneiro2019]
-
--/
 
 
 open Encodable Denumerable
+-- open ComputableIn O
 
-namespace Nat.Partrec
 
-theorem rfind' {f} (hf : Nat.Partrec f) :
-    Nat.Partrec
+namespace Nat.RecursiveIn
+
+#check Computable.comp
+
+theorem rfind' {f} (hf : Nat.RecursiveIn O f) :
+    Nat.RecursiveIn O
       (Nat.unpaired fun a m =>
         (Nat.rfind fun n => (fun m => m = 0) <$> f (Nat.pair a (n + m))).map (· + m)) :=
-  Partrec₂.unpaired'.2 <| by
+  RecursiveIn₂.unpaired'.2 <| by
     refine
-      Partrec.map
-        ((@Partrec₂.unpaired' fun a b : ℕ =>
+      RecursiveIn.map
+        ((@RecursiveIn₂.unpaired' O fun a b : ℕ =>
               Nat.rfind fun n => (fun m => m = 0) <$> f (Nat.pair a (n + b))).1
           ?_)
-        (Primrec.nat_add.comp Primrec.snd <| Primrec.snd.comp Primrec.fst).to_comp.to₂
-    have : Nat.Partrec (fun a => Nat.rfind (fun n => (fun m => decide (m = 0)) <$>
+        (Primrec.nat_add.comp Primrec.snd <| Primrec.snd.comp Primrec.fst).to_compIn.to₂
+        -- (ComputableIn.to₂ (ComputableIn O₂.to_compIn (Primrec.nat_add.comp Primrec.snd <| Primrec.snd.comp Primrec.fst)))
+    have : Nat.RecursiveIn O (fun a => Nat.rfind (fun n => (fun m => decide (m = 0)) <$>
       Nat.unpaired (fun a b => f (Nat.pair (Nat.unpair a).1 (b + (Nat.unpair a).2)))
         (Nat.pair a n))) :=
       rfind
-        (Partrec₂.unpaired'.2
-          ((Partrec.nat_iff.2 hf).comp
+        (RecursiveIn₂.unpaired'.2
+          ((RecursiveIn.nat_iff.2 hf).comp
               (Primrec₂.pair.comp (Primrec.fst.comp <| Primrec.unpair.comp Primrec.fst)
                   (Primrec.nat_add.comp Primrec.snd
-                    (Primrec.snd.comp <| Primrec.unpair.comp Primrec.fst))).to_comp))
+                    (Primrec.snd.comp <| Primrec.unpair.comp Primrec.fst))).to_compIn))
     simpa
 
-/-- Code for partial recursive functions from ℕ to ℕ.
-See `Nat.Partrec.Code.eval` for the interpretation of these constructors.
--/
 inductive Code : Type
-  | zero : Code
-  | succ : Code
-  | left : Code
-  | right : Code
-  | pair : Code → Code → Code
-  | comp : Code → Code → Code
-  | prec : Code → Code → Code
-  | rfind' : Code → Code
+| zero : Code
+| succ : Code
+| left : Code
+| right : Code
+| oracle : Code
+| pair : Code → Code → Code
+| comp : Code → Code → Code
+| prec : Code → Code → Code
+| rfind' : Code → Code
+
 
 compile_inductive% Code
 
-end Nat.Partrec
+end Nat.RecursiveIn
 
-namespace Nat.Partrec.Code
+namespace Nat.RecursiveIn.Code
 
 instance instInhabited : Inhabited Code :=
   ⟨zero⟩
@@ -96,10 +65,10 @@ protected def const : ℕ → Code
   | 0 => zero
   | n + 1 => comp succ (Code.const n)
 
-theorem const_inj : ∀ {n₁ n₂}, Nat.Partrec.Code.const n₁ = Nat.Partrec.Code.const n₂ → n₁ = n₂
+theorem const_inj : ∀ {n₁ n₂}, Nat.RecursiveIn.Code.const n₁ = Nat.RecursiveIn.Code.const n₂ → n₁ = n₂
   | 0, 0, _ => by simp
   | n₁ + 1, n₂ + 1, h => by
-    dsimp [Nat.Partrec.Code.const] at h
+    dsimp [Nat.RecursiveIn.Code.const] at h
     injection h with h₁ h₂
     simp only [const_inj h₂]
 
@@ -112,68 +81,93 @@ protected def id : Code :=
 def curry (c : Code) (n : ℕ) : Code :=
   comp c (pair (Code.const n) Code.id)
 
-/-- An encoding of a `Nat.Partrec.Code` as a ℕ. -/
+
+
+
+
+
+
+
+
+
 def encodeCode : Code → ℕ
-  | zero => 0
-  | succ => 1
-  | left => 2
-  | right => 3
-  | pair cf cg => 2 * (2 * Nat.pair (encodeCode cf) (encodeCode cg)) + 4
-  | comp cf cg => 2 * (2 * Nat.pair (encodeCode cf) (encodeCode cg) + 1) + 4
-  | prec cf cg => (2 * (2 * Nat.pair (encodeCode cf) (encodeCode cg)) + 1) + 4
-  | rfind' cf => (2 * (2 * encodeCode cf + 1) + 1) + 4
+| Code.zero        => 0
+| Code.succ        => 1
+| Code.left        => 2
+| Code.right       => 3
+| Code.oracle      => 4
+| Code.pair cf cg  => 2*(2*(Nat.pair (encodeCode cf) (encodeCode cg))  )   + 5
+| Code.comp cf cg  => 2*(2*(Nat.pair (encodeCode cf) (encodeCode cg))  )+1 + 5
+| Code.prec cf cg  => 2*(2*(Nat.pair (encodeCode cf) (encodeCode cg))+1)   + 5
+| Code.rfind' cf   => 2*(2*(encodeCode cf                            )+1)+1 + 5
 
 /--
-A decoder for `Nat.Partrec.Code.encodeCode`, taking any ℕ to the `Nat.Partrec.Code` it represents.
+Procedure for decoding:
+
+If n≤4. trivial.
+
+Otherwise if n≥5, check n%4. The 4 possible values correspond to
+pair
+comp
+prec
+rfind'
 -/
-def ofNatCode : ℕ → Code
-  | 0 => zero
-  | 1 => succ
-  | 2 => left
-  | 3 => right
-  | n + 4 =>
-    let m := n.div2.div2
-    have hm : m < n + 4 := by
-      simp only [m, div2_val]
-      exact
-        lt_of_le_of_lt (le_trans (Nat.div_le_self _ _) (Nat.div_le_self _ _))
-          (Nat.succ_le_succ (Nat.le_add_right _ _))
-    have _m1 : m.unpair.1 < n + 4 := lt_of_le_of_lt m.unpair_left_le hm
-    have _m2 : m.unpair.2 < n + 4 := lt_of_le_of_lt m.unpair_right_le hm
-    match n.bodd, n.div2.bodd with
-    | false, false => pair (ofNatCode m.unpair.1) (ofNatCode m.unpair.2)
-    | false, true  => comp (ofNatCode m.unpair.1) (ofNatCode m.unpair.2)
-    | true , false => prec (ofNatCode m.unpair.1) (ofNatCode m.unpair.2)
-    | true , true  => rfind' (ofNatCode m)
+def decodeCode : ℕ → Code
+| 0 => Code.zero
+| 1 => Code.succ
+| 2 => Code.left
+| 3 => Code.right
+| 4 => Code.oracle
+| n + 5 =>
+  let m := n.div2.div2
+  have hm : m < n + 5 := by
+    simp only [m, Nat.div2_val]
+    exact
+      lt_of_le_of_lt (le_trans (Nat.div_le_self _ _) (Nat.div_le_self _ _))
+        (Nat.succ_le_succ (Nat.le_add_right _ _))
+  have _m1 : m.unpair.1 < n + 5 := lt_of_le_of_lt m.unpair_left_le hm
+  have _m2 : m.unpair.2 < n + 5 := lt_of_le_of_lt m.unpair_right_le hm
+  match n.bodd, n.div2.bodd with
+  | false, false => Code.pair (decodeCode m.unpair.1) (decodeCode m.unpair.2) -- n%4=0
+  | true , false => Code.comp (decodeCode m.unpair.1) (decodeCode m.unpair.2) -- n%4=1
+  | false, true  => Code.prec (decodeCode m.unpair.1) (decodeCode m.unpair.2) -- n%4=2
+  | true , true  => Code.rfind' (decodeCode m)                                 -- n%4=3
 
-/-- Proof that `Nat.Partrec.Code.ofNatCode` is the inverse of `Nat.Partrec.Code.encodeCode` -/
-private theorem encode_ofNatCode : ∀ n, encodeCode (ofNatCode n) = n
-  | 0 => by simp [ofNatCode, encodeCode]
-  | 1 => by simp [ofNatCode, encodeCode]
-  | 2 => by simp [ofNatCode, encodeCode]
-  | 3 => by simp [ofNatCode, encodeCode]
-  | n + 4 => by
+instance : OfNat (Code) m where ofNat := decodeCode m
+instance : Coe ℕ Code := ⟨decodeCode⟩
+instance : Coe Code ℕ := ⟨encodeCode⟩
+/-- Converts an `Code` into a `ℕ`. -/ @[coe] def ofCode : Code → ℕ := encodeCode
+abbrev ofNatCode := decodeCode
+@[simp] theorem decodeCode_encodeCode : ∀ c, decodeCode (encodeCode c) = c := fun c => by
+  induction c <;> (simp [encodeCode, decodeCode, Nat.div2_val, *])
+@[simp] theorem encodeCode_decodeCode : ∀ c, encodeCode (decodeCode c) = c :=
+λ c => match c with
+  | 0 => by simp only [decodeCode, encodeCode]
+  | 1 => by simp only [decodeCode, encodeCode]
+  | 2 => by simp only [decodeCode, encodeCode]
+  | 3 => by simp only [decodeCode, encodeCode]
+  | 4 => by simp only [decodeCode, encodeCode]
+  | n + 5 => by
     let m := n.div2.div2
-    have hm : m < n + 4 := by
-      simp only [m, div2_val]
-      exact
-        lt_of_le_of_lt (le_trans (Nat.div_le_self _ _) (Nat.div_le_self _ _))
-          (Nat.succ_le_succ (Nat.le_add_right _ _))
-    have _m1 : m.unpair.1 < n + 4 := lt_of_le_of_lt m.unpair_left_le hm
-    have _m2 : m.unpair.2 < n + 4 := lt_of_le_of_lt m.unpair_right_le hm
-    have IH := encode_ofNatCode m
-    have IH1 := encode_ofNatCode m.unpair.1
-    have IH2 := encode_ofNatCode m.unpair.2
+    have hm : m < n + 5 := by
+      simp only [m, Nat.div2_val]
+      exact lt_of_le_of_lt (le_trans (Nat.div_le_self _ _) (Nat.div_le_self _ _)) (Nat.succ_le_succ (Nat.le_add_right _ _))
+    have _m1 : m.unpair.1 < n + 5 := lt_of_le_of_lt m.unpair_left_le hm
+    have _m2 : m.unpair.2 < n + 5 := lt_of_le_of_lt m.unpair_right_le hm
+    have IH := encodeCode_decodeCode m
+    have IH1 := encodeCode_decodeCode m.unpair.1
+    have IH2 := encodeCode_decodeCode m.unpair.2
     conv_rhs => rw [← Nat.bit_decomp n, ← Nat.bit_decomp n.div2]
-    simp only [ofNatCode.eq_5]
-    cases n.bodd <;> cases n.div2.bodd <;>
-      simp [m, encodeCode, ofNatCode, IH, IH1, IH2, Nat.bit_val]
+    simp only [decodeCode.eq_6]
+    cases n.bodd <;> cases n.div2.bodd <;> simp [m, encodeCode, IH, IH1, IH2, Nat.bit_val]
+instance instDenumerable : Denumerable Code := mk' ⟨encodeCode, decodeCode, decodeCode_encodeCode, encodeCode_decodeCode⟩
 
-instance instDenumerable : Denumerable Code :=
-  mk'
-    ⟨encodeCode, ofNatCode, fun c => by
-        induction c <;> simp [encodeCode, ofNatCode, Nat.div2_val, *],
-      encode_ofNatCode⟩
+
+
+
+/-- Proof that `Nat.RecursiveIn.Code.ofNatCode` is the inverse of `Nat.RecursiveIn.Code.encodeCode` -/
+private theorem encode_ofNatCode : ∀ n, encodeCode (ofNatCode n) = n := by exact fun n ↦encodeCode_decodeCode n
+
 
 theorem encodeCode_eq : encode = encodeCode :=
   rfl
@@ -186,7 +180,7 @@ theorem encode_lt_pair (cf cg) :
   simp only [encodeCode_eq, encodeCode]
   have := Nat.mul_le_mul_right (Nat.pair cf.encodeCode cg.encodeCode) (by decide : 1 ≤ 2 * 2)
   rw [one_mul, mul_assoc] at this
-  have := lt_of_le_of_lt this (lt_add_of_pos_right _ (by decide : 0 < 4))
+  have := lt_of_le_of_lt this (lt_add_of_pos_right _ (by decide : 0 < 5))
   exact ⟨lt_of_le_of_lt (Nat.left_le_pair _ _) this, lt_of_le_of_lt (Nat.right_le_pair _ _) this⟩
 
 theorem encode_lt_comp (cf cg) :
@@ -203,11 +197,11 @@ theorem encode_lt_rfind' (cf) : encode cf < encode (rfind' cf) := by
   simp only [encodeCode_eq, encodeCode]
   omega
 
-end Nat.Partrec.Code
+end Nat.RecursiveIn.Code
 
 section
 open Primrec
-namespace Nat.Partrec.Code
+namespace Nat.RecursiveIn.Code
 
 theorem pair_prim : Primrec₂ pair :=
   Primrec₂.ofNat_iff.2 <|
@@ -217,27 +211,29 @@ theorem pair_prim : Primrec₂ pair :=
           nat_double.comp <|
             Primrec₂.natPair.comp (encode_iff.2 <| (Primrec.ofNat Code).comp fst)
               (encode_iff.2 <| (Primrec.ofNat Code).comp snd))
-        (Primrec₂.const 4)
+        (Primrec₂.const 5)
 
 theorem comp_prim : Primrec₂ comp :=
   Primrec₂.ofNat_iff.2 <|
     Primrec₂.encode_iff.1 <|
       nat_add.comp
-        (nat_double.comp <|
+        (
           nat_double_succ.comp <|
+          nat_double.comp <|
             Primrec₂.natPair.comp (encode_iff.2 <| (Primrec.ofNat Code).comp fst)
               (encode_iff.2 <| (Primrec.ofNat Code).comp snd))
-        (Primrec₂.const 4)
+        (Primrec₂.const 5)
 
 theorem prec_prim : Primrec₂ prec :=
   Primrec₂.ofNat_iff.2 <|
     Primrec₂.encode_iff.1 <|
       nat_add.comp
-        (nat_double_succ.comp <|
+        (
           nat_double.comp <|
+          nat_double_succ.comp <|
             Primrec₂.natPair.comp (encode_iff.2 <| (Primrec.ofNat Code).comp fst)
               (encode_iff.2 <| (Primrec.ofNat Code).comp snd))
-        (Primrec₂.const 4)
+        (Primrec₂.const 5)
 
 theorem rfind_prim : Primrec rfind' :=
   ofNat_iff.2 <|
@@ -245,11 +241,13 @@ theorem rfind_prim : Primrec rfind' :=
       nat_add.comp
         (nat_double_succ.comp <| nat_double_succ.comp <|
           encode_iff.2 <| Primrec.ofNat Code)
-        (const 4)
+        (const 5)
 
 theorem rec_prim' {α σ} [Primcodable α] [Primcodable σ] {c : α → Code} (hc : Primrec c) {z : α → σ}
     (hz : Primrec z) {s : α → σ} (hs : Primrec s) {l : α → σ} (hl : Primrec l) {r : α → σ}
-    (hr : Primrec r) {pr : α → Code × Code × σ × σ → σ} (hpr : Primrec₂ pr)
+    (hr : Primrec r)
+    {o : α → σ} (ho : Primrec o)
+    {pr : α → Code × Code × σ × σ → σ} (hpr : Primrec₂ pr)
     {co : α → Code × Code × σ × σ → σ} (hco : Primrec₂ co) {pc : α → Code × Code × σ × σ → σ}
     (hpc : Primrec₂ pc) {rf : α → Code × σ → σ} (hrf : Primrec₂ rf) :
     let PR (a) cf cg hf hg := pr a (cf, cg, hf, hg)
@@ -257,7 +255,7 @@ theorem rec_prim' {α σ} [Primcodable α] [Primcodable σ] {c : α → Code} (h
     let PC (a) cf cg hf hg := pc a (cf, cg, hf, hg)
     let RF (a) cf hf := rf a (cf, hf)
     let F (a : α) (c : Code) : σ :=
-      Nat.Partrec.Code.recOn c (z a) (s a) (l a) (r a) (PR a) (CO a) (PC a) (RF a)
+      Nat.RecursiveIn.Code.recOn c (z a) (s a) (l a) (r a) (o a) (PR a) (CO a) (PC a) (RF a)
     Primrec (fun a => F a (c a) : α → σ) := by
   intros _ _ _ _ F
   let G₁ : (α × List σ) × ℕ × ℕ → Option σ := fun p =>
@@ -267,8 +265,8 @@ theorem rec_prim' {α σ} [Primcodable α] [Primcodable σ] {c : α → Code} (h
     (IH[m.unpair.2]?).map fun s₂ =>
     cond n.bodd
       (cond n.div2.bodd (rf a (ofNat Code m, s))
-        (pc a (ofNat Code m.unpair.1, ofNat Code m.unpair.2, s₁, s₂)))
-      (cond n.div2.bodd (co a (ofNat Code m.unpair.1, ofNat Code m.unpair.2, s₁, s₂))
+        (co a (ofNat Code m.unpair.1, ofNat Code m.unpair.2, s₁, s₂)))
+      (cond n.div2.bodd (pc a (ofNat Code m.unpair.1, ofNat Code m.unpair.2, s₁, s₂))
         (pr a (ofNat Code m.unpair.1, ofNat Code m.unpair.2, s₁, s₂)))
   have : Primrec G₁ :=
     option_bind (list_getElem?.comp (snd.comp fst) (snd.comp snd)) <| .mk <|
@@ -287,50 +285,55 @@ theorem rec_prim' {α σ} [Primcodable α] [Primcodable σ] {c : α → Code} (h
     (nat_bodd.comp n).cond
       ((nat_bodd.comp <| nat_div2.comp n).cond
         (hrf.comp a (((Primrec.ofNat Code).comp m).pair s))
-        (hpc.comp a (((Primrec.ofNat Code).comp m₁).pair <|
-          ((Primrec.ofNat Code).comp m₂).pair <| s₁.pair s₂)))
+        (hco.comp a (((Primrec.ofNat Code).comp m₁).pair <| ((Primrec.ofNat Code).comp m₂).pair <| s₁.pair s₂)))
       (Primrec.cond (nat_bodd.comp <| nat_div2.comp n)
-        (hco.comp a (((Primrec.ofNat Code).comp m₁).pair <|
-          ((Primrec.ofNat Code).comp m₂).pair <| s₁.pair s₂))
-        (hpr.comp a (((Primrec.ofNat Code).comp m₁).pair <|
-          ((Primrec.ofNat Code).comp m₂).pair <| s₁.pair s₂)))
+        (hpc.comp a (((Primrec.ofNat Code).comp m₁).pair <| ((Primrec.ofNat Code).comp m₂).pair <| s₁.pair s₂))
+        (hpr.comp a (((Primrec.ofNat Code).comp m₁).pair <| ((Primrec.ofNat Code).comp m₂).pair <| s₁.pair s₂)))
   let G : α → List σ → Option σ := fun a IH =>
     IH.length.casesOn (some (z a)) fun n =>
     n.casesOn (some (s a)) fun n =>
     n.casesOn (some (l a)) fun n =>
     n.casesOn (some (r a)) fun n =>
+    n.casesOn (some (o a)) fun n =>
     G₁ ((a, IH), n, n.div2.div2)
   have : Primrec₂ G := .mk <|
     nat_casesOn (list_length.comp snd) (option_some_iff.2 (hz.comp fst)) <| .mk <|
     nat_casesOn snd (option_some_iff.2 (hs.comp (fst.comp fst))) <| .mk <|
     nat_casesOn snd (option_some_iff.2 (hl.comp (fst.comp <| fst.comp fst))) <| .mk <|
     nat_casesOn snd (option_some_iff.2 (hr.comp (fst.comp <| fst.comp <| fst.comp fst))) <| .mk <|
+    nat_casesOn snd (option_some_iff.2 (ho.comp (fst.comp <| fst.comp <| fst.comp <| fst.comp fst))) <| .mk <|
     this.comp <|
-      ((fst.pair snd).comp <| fst.comp <| fst.comp <| fst.comp <| fst).pair <|
+      -- ((fst.pair snd).comp <| fst.comp <| fst.comp <| fst.comp <| fst).pair <|
+      ((fst.pair snd).comp <| fst.comp <| fst.comp <| fst.comp <| fst.comp <| fst).pair <|
       snd.pair <| nat_div2.comp <| nat_div2.comp snd
   refine (nat_strong_rec (fun a n => F a (ofNat Code n)) this.to₂ fun a n => ?_)
     |>.comp .id (encode_iff.2 hc) |>.of_eq fun a => by simp
-  iterate 4 rcases n with - | n; · simp [ofNatCode_eq, ofNatCode]; rfl
+  iterate 5 rcases n with - | n; · simp [ofNatCode_eq, ofNatCode, decodeCode]; rfl
+  -- · simp [ofNatCode_eq, ofNatCode, decodeCode];
+  --   exact?
   simp only [G]; rw [List.length_map, List.length_range]
   let m := n.div2.div2
-  show G₁ ((a, (List.range (n + 4)).map fun n => F a (ofNat Code n)), n, m)
-    = some (F a (ofNat Code (n + 4)))
-  have hm : m < n + 4 := by
+  show G₁ ((a, (List.range (n + 5)).map fun n => F a (ofNat Code n)), n, m)
+    = some (F a (ofNat Code (n + 5)))
+  have hm : m < n + 5 := by
     simp only [m, div2_val]
     exact lt_of_le_of_lt
       (le_trans (Nat.div_le_self ..) (Nat.div_le_self ..))
       (Nat.succ_le_succ (Nat.le_add_right ..))
-  have m1 : m.unpair.1 < n + 4 := lt_of_le_of_lt m.unpair_left_le hm
-  have m2 : m.unpair.2 < n + 4 := lt_of_le_of_lt m.unpair_right_le hm
+  have m1 : m.unpair.1 < n + 5 := lt_of_le_of_lt m.unpair_left_le hm
+  have m2 : m.unpair.2 < n + 5 := lt_of_le_of_lt m.unpair_right_le hm
   simp [G₁, m, List.getElem?_map, List.getElem?_range, hm, m1, m2]
-  rw [show ofNat Code (n + 4) = ofNatCode (n + 4) from rfl]
-  simp only [ofNatCode]
+  rw [show ofNat Code (n + 5) = ofNatCode (n + 5) from rfl]
+  unfold decodeCode
+  simp
   cases n.bodd <;> cases n.div2.bodd <;> rfl
 
-/-- Recursion on `Nat.Partrec.Code` is primitive recursive. -/
+
+/-- Recursion on `Nat.RecursiveIn.Code` is primitive recursive. -/
 theorem rec_prim {α σ} [Primcodable α] [Primcodable σ] {c : α → Code} (hc : Primrec c) {z : α → σ}
     (hz : Primrec z) {s : α → σ} (hs : Primrec s) {l : α → σ} (hl : Primrec l) {r : α → σ}
-    (hr : Primrec r) {pr : α → Code → Code → σ → σ → σ}
+    (hr : Primrec r) {o : α → σ}
+    (ho : Primrec o) {pr : α → Code → Code → σ → σ → σ}
     (hpr : Primrec fun a : α × Code × Code × σ × σ => pr a.1 a.2.1 a.2.2.1 a.2.2.2.1 a.2.2.2.2)
     {co : α → Code → Code → σ → σ → σ}
     (hco : Primrec fun a : α × Code × Code × σ × σ => co a.1 a.2.1 a.2.2.1 a.2.2.2.1 a.2.2.2.2)
@@ -338,164 +341,171 @@ theorem rec_prim {α σ} [Primcodable α] [Primcodable σ] {c : α → Code} (hc
     (hpc : Primrec fun a : α × Code × Code × σ × σ => pc a.1 a.2.1 a.2.2.1 a.2.2.2.1 a.2.2.2.2)
     {rf : α → Code → σ → σ} (hrf : Primrec fun a : α × Code × σ => rf a.1 a.2.1 a.2.2) :
     let F (a : α) (c : Code) : σ :=
-      Nat.Partrec.Code.recOn c (z a) (s a) (l a) (r a) (pr a) (co a) (pc a) (rf a)
+      Nat.RecursiveIn.Code.recOn c (z a) (s a) (l a) (r a) (o a) (pr a) (co a) (pc a) (rf a)
     Primrec fun a => F a (c a) :=
-  rec_prim' hc hz hs hl hr
+  rec_prim' hc hz hs hl hr ho
     (pr := fun a b => pr a b.1 b.2.1 b.2.2.1 b.2.2.2) (.mk hpr)
     (co := fun a b => co a b.1 b.2.1 b.2.2.1 b.2.2.2) (.mk hco)
     (pc := fun a b => pc a b.1 b.2.1 b.2.2.1 b.2.2.2) (.mk hpc)
     (rf := fun a b => rf a b.1 b.2) (.mk hrf)
 
-end Nat.Partrec.Code
+end Nat.RecursiveIn.Code
 end
 
-namespace Nat.Partrec.Code
+namespace Nat.RecursiveIn.Code
 section
 
-open Computable
+open ComputableIn
 
-/-- Recursion on `Nat.Partrec.Code` is computable. -/
-theorem rec_computable {α σ} [Primcodable α] [Primcodable σ] {c : α → Code} (hc : Computable c)
-    {z : α → σ} (hz : Computable z) {s : α → σ} (hs : Computable s) {l : α → σ} (hl : Computable l)
-    {r : α → σ} (hr : Computable r) {pr : α → Code × Code × σ × σ → σ} (hpr : Computable₂ pr)
-    {co : α → Code × Code × σ × σ → σ} (hco : Computable₂ co) {pc : α → Code × Code × σ × σ → σ}
-    (hpc : Computable₂ pc) {rf : α → Code × σ → σ} (hrf : Computable₂ rf) :
+/-- Recursion on `Nat.RecursiveIn.Code` is computable. -/
+theorem rec_computable {α σ} [Primcodable α] [Primcodable σ] {c : α → Code} (hc : ComputableIn O c)
+    {z : α → σ} (hz : ComputableIn O z) {s : α → σ} (hs : ComputableIn O s) {l : α → σ} (hl : ComputableIn O l)
+    {r : α → σ} (hr : ComputableIn O r) {o : α → σ} (ho : ComputableIn O o) {pr : α → Code × Code × σ × σ → σ} (hpr : ComputableIn₂ O pr)
+    {co : α → Code × Code × σ × σ → σ} (hco : ComputableIn₂ O co) {pc : α → Code × Code × σ × σ → σ}
+    (hpc : ComputableIn₂ O pc) {rf : α → Code × σ → σ} (hrf : ComputableIn₂ O rf) :
     let PR (a) cf cg hf hg := pr a (cf, cg, hf, hg)
     let CO (a) cf cg hf hg := co a (cf, cg, hf, hg)
     let PC (a) cf cg hf hg := pc a (cf, cg, hf, hg)
     let RF (a) cf hf := rf a (cf, hf)
     let F (a : α) (c : Code) : σ :=
-      Nat.Partrec.Code.recOn c (z a) (s a) (l a) (r a) (PR a) (CO a) (PC a) (RF a)
-    Computable fun a => F a (c a) := by
+      Nat.RecursiveIn.Code.recOn c (z a) (s a) (l a) (r a) (o a) (PR a) (CO a) (PC a) (RF a)
+    ComputableIn O fun a => F a (c a) := by
   -- TODO(Mario): less copy-paste from previous proof
   intros _ _ _ _ F
   let G₁ : (α × List σ) × ℕ × ℕ → Option σ := fun p =>
     letI a := p.1.1; letI IH := p.1.2; letI n := p.2.1; letI m := p.2.2
-    (IH.get? m).bind fun s =>
-    (IH.get? m.unpair.1).bind fun s₁ =>
-    (IH.get? m.unpair.2).map fun s₂ =>
+    (IH[m]?).bind fun s =>
+    (IH[m.unpair.1]?).bind fun s₁ =>
+    (IH[m.unpair.2]?).map fun s₂ =>
     cond n.bodd
       (cond n.div2.bodd (rf a (ofNat Code m, s))
-        (pc a (ofNat Code m.unpair.1, ofNat Code m.unpair.2, s₁, s₂)))
-      (cond n.div2.bodd (co a (ofNat Code m.unpair.1, ofNat Code m.unpair.2, s₁, s₂))
+        (co a (ofNat Code m.unpair.1, ofNat Code m.unpair.2, s₁, s₂)))
+      (cond n.div2.bodd (pc a (ofNat Code m.unpair.1, ofNat Code m.unpair.2, s₁, s₂))
         (pr a (ofNat Code m.unpair.1, ofNat Code m.unpair.2, s₁, s₂)))
-  have : Computable G₁ := by
-    refine option_bind (list_get?.comp (snd.comp fst) (snd.comp snd)) <| .mk ?_
-    refine option_bind ((list_get?.comp (snd.comp fst)
-      (fst.comp <| Computable.unpair.comp (snd.comp snd))).comp fst) <| .mk ?_
-    refine option_map ((list_get?.comp (snd.comp fst)
-      (snd.comp <| Computable.unpair.comp (snd.comp snd))).comp <| fst.comp fst) <| .mk ?_
+  have : ComputableIn O G₁ := by
+    refine option_bind (list_getElem?.comp (snd.comp fst) (snd.comp snd)) <| .mk ?_
+    refine option_bind ((list_getElem?.comp (snd.comp fst)
+      (fst.comp <| ComputableIn.unpair.comp (snd.comp snd))).comp fst) <| .mk ?_
+    refine option_map ((list_getElem?.comp (snd.comp fst)
+      (snd.comp <| ComputableIn.unpair.comp (snd.comp snd))).comp <| fst.comp fst) <| .mk ?_
     exact
       have a := fst.comp (fst.comp <| fst.comp <| fst.comp fst)
       have n := fst.comp (snd.comp <| fst.comp <| fst.comp fst)
       have m := snd.comp (snd.comp <| fst.comp <| fst.comp fst)
-      have m₁ := fst.comp (Computable.unpair.comp m)
-      have m₂ := snd.comp (Computable.unpair.comp m)
+      have m₁ := fst.comp (ComputableIn.unpair.comp m)
+      have m₂ := snd.comp (ComputableIn.unpair.comp m)
       have s := snd.comp (fst.comp fst)
       have s₁ := snd.comp fst
       have s₂ := snd
       (nat_bodd.comp n).cond
         ((nat_bodd.comp <| nat_div2.comp n).cond
-          (hrf.comp a (((Computable.ofNat Code).comp m).pair s))
-          (hpc.comp a (((Computable.ofNat Code).comp m₁).pair <|
-            ((Computable.ofNat Code).comp m₂).pair <| s₁.pair s₂)))
-        (Computable.cond (nat_bodd.comp <| nat_div2.comp n)
-          (hco.comp a (((Computable.ofNat Code).comp m₁).pair <|
-            ((Computable.ofNat Code).comp m₂).pair <| s₁.pair s₂))
-          (hpr.comp a (((Computable.ofNat Code).comp m₁).pair <|
-            ((Computable.ofNat Code).comp m₂).pair <| s₁.pair s₂)))
+          (hrf.comp a (((ComputableIn.ofNat Code).comp m).pair s))
+          (hco.comp a (((ComputableIn.ofNat Code).comp m₁).pair <|
+            ((ComputableIn.ofNat Code).comp m₂).pair <| s₁.pair s₂)))
+        (ComputableIn.cond (nat_bodd.comp <| nat_div2.comp n)
+          (hpc.comp a (((ComputableIn.ofNat Code).comp m₁).pair <|
+            ((ComputableIn.ofNat Code).comp m₂).pair <| s₁.pair s₂))
+          (hpr.comp a (((ComputableIn.ofNat Code).comp m₁).pair <|
+            ((ComputableIn.ofNat Code).comp m₂).pair <| s₁.pair s₂)))
   let G : α → List σ → Option σ := fun a IH =>
     IH.length.casesOn (some (z a)) fun n =>
     n.casesOn (some (s a)) fun n =>
     n.casesOn (some (l a)) fun n =>
     n.casesOn (some (r a)) fun n =>
+    n.casesOn (some (o a)) fun n =>
     G₁ ((a, IH), n, n.div2.div2)
-  have : Computable₂ G := .mk <|
+  have : ComputableIn₂ O G := .mk <|
     nat_casesOn (list_length.comp snd) (option_some_iff.2 (hz.comp fst)) <| .mk <|
     nat_casesOn snd (option_some_iff.2 (hs.comp (fst.comp fst))) <| .mk <|
     nat_casesOn snd (option_some_iff.2 (hl.comp (fst.comp <| fst.comp fst))) <| .mk <|
     nat_casesOn snd (option_some_iff.2 (hr.comp (fst.comp <| fst.comp <| fst.comp fst))) <| .mk <|
+    nat_casesOn snd (option_some_iff.2 (ho.comp (fst.comp <| fst.comp <| fst.comp <| fst.comp fst))) <| .mk <|
     this.comp <|
-      ((fst.pair snd).comp <| fst.comp <| fst.comp <| fst.comp <| fst).pair <|
+      -- ((fst.pair snd).comp <| fst.comp <| fst.comp <| fst.comp <| fst).pair <|
+      ((fst.pair snd).comp <| fst.comp <| fst.comp <| fst.comp <| fst.comp <| fst).pair <|
       snd.pair <| nat_div2.comp <| nat_div2.comp snd
   refine (nat_strong_rec (fun a n => F a (ofNat Code n)) this.to₂ fun a n => ?_)
     |>.comp .id (encode_iff.2 hc) |>.of_eq fun a => by simp
-  iterate 4 rcases n with - | n; · simp [ofNatCode_eq, ofNatCode]; rfl
+  iterate 5 rcases n with - | n; · simp [ofNatCode_eq, ofNatCode, decodeCode]; rfl
   simp only [G]; rw [List.length_map, List.length_range]
   let m := n.div2.div2
-  show G₁ ((a, (List.range (n + 4)).map fun n => F a (ofNat Code n)), n, m)
-    = some (F a (ofNat Code (n + 4)))
-  have hm : m < n + 4 := by
+  show G₁ ((a, (List.range (n + 5)).map fun n => F a (ofNat Code n)), n, m)
+    = some (F a (ofNat Code (n + 5)))
+  have hm : m < n + 5 := by
     simp only [m, div2_val]
     exact lt_of_le_of_lt
       (le_trans (Nat.div_le_self ..) (Nat.div_le_self ..))
       (Nat.succ_le_succ (Nat.le_add_right ..))
-  have m1 : m.unpair.1 < n + 4 := lt_of_le_of_lt m.unpair_left_le hm
-  have m2 : m.unpair.2 < n + 4 := lt_of_le_of_lt m.unpair_right_le hm
+  have m1 : m.unpair.1 < n + 5 := lt_of_le_of_lt m.unpair_left_le hm
+  have m2 : m.unpair.2 < n + 5 := lt_of_le_of_lt m.unpair_right_le hm
   simp [G₁, m, List.getElem?_map, List.getElem?_range, hm, m1, m2]
-  rw [show ofNat Code (n + 4) = ofNatCode (n + 4) from rfl]
-  simp [ofNatCode]
+  rw [show ofNat Code (n + 5) = ofNatCode (n + 5) from rfl]
+  unfold decodeCode
+  simp
   cases n.bodd <;> cases n.div2.bodd <;> rfl
 
 end
 
-/-- The interpretation of a `Nat.Partrec.Code` as a partial function.
-* `Nat.Partrec.Code.zero`: The constant zero function.
-* `Nat.Partrec.Code.succ`: The successor function.
-* `Nat.Partrec.Code.left`: Left unpairing of a pair of ℕ (encoded by `Nat.pair`)
-* `Nat.Partrec.Code.right`: Right unpairing of a pair of ℕ (encoded by `Nat.pair`)
-* `Nat.Partrec.Code.pair`: Pairs the outputs of argument codes using `Nat.pair`.
-* `Nat.Partrec.Code.comp`: Composition of two argument codes.
-* `Nat.Partrec.Code.prec`: Primitive recursion. Given an argument of the form `Nat.pair a n`:
-  * If `n = 0`, returns `eval cf a`.
-  * If `n = succ k`, returns `eval cg (pair a (pair k (eval (prec cf cg) (pair a k))))`
-* `Nat.Partrec.Code.rfind'`: Minimization. For `f` an argument of the form `Nat.pair a m`,
+/-- The interpretation of a `Nat.RecursiveIn.Code` as a partial function.
+* `Nat.RecursiveIn.Code.zero`: The constant zero function.
+* `Nat.RecursiveIn.Code.succ`: The successor function.
+* `Nat.RecursiveIn.Code.left`: Left unpairing of a pair of ℕ (encoded by `Nat.pair`)
+* `Nat.RecursiveIn.Code.right`: Right unpairing of a pair of ℕ (encoded by `Nat.pair`)
+* `Nat.RecursiveIn.Code.pair`: Pairs the outputs of argument codes using `Nat.pair`.
+* `Nat.RecursiveIn.Code.comp`: Composition of two argument codes.
+* `Nat.RecursiveIn.Code.prec`: Primitive recursion. Given an argument of the form `Nat.pair a n`:
+  * If `n = 0`, returns `eval O cf a`.
+  * If `n = succ k`, returns `eval O cg (pair a (pair k (eval O (prec cf cg) (pair a k))))`
+* `Nat.RecursiveIn.Code.rfind'`: Minimization. For `f` an argument of the form `Nat.pair a m`,
   `rfind' f m` returns the least `a` such that `f a m = 0`, if one exists and `f b m` terminates
   for `b < a`
 -/
-def eval : Code → ℕ →. ℕ
-  | zero => pure 0
-  | succ => Nat.succ
-  | left => ↑fun n : ℕ => n.unpair.1
-  | right => ↑fun n : ℕ => n.unpair.2
-  | pair cf cg => fun n => Nat.pair <$> eval cf n <*> eval cg n
-  | comp cf cg => fun n => eval cg n >>= eval cf
-  | prec cf cg =>
+def eval (O : ℕ → ℕ) : Code → ℕ →. ℕ
+| zero => pure 0
+| succ => fun n => some (n + 1)
+| left => fun n => some (Nat.unpair n).1
+| right => fun n => some (Nat.unpair n).2
+| oracle => O
+| pair cf cg =>
+    fun n => Nat.pair <$> eval O cf n <*> eval O cg n
+| comp cf cg =>
+    fun n => eval O cg n >>= eval O cf
+| prec cf cg =>
     Nat.unpaired fun a n =>
-      n.rec (eval cf a) fun y IH => do
+      n.rec (eval O cf a) fun y IH => do
         let i ← IH
-        eval cg (Nat.pair a (Nat.pair y i))
-  | rfind' cf =>
+        eval O cg (Nat.pair a (Nat.pair y i))
+| rfind' cf =>
     Nat.unpaired fun a m =>
-      (Nat.rfind fun n => (fun m => m = 0) <$> eval cf (Nat.pair a (n + m))).map (· + m)
+      (Nat.rfind fun n => (fun x => x = 0) <$> eval O cf (Nat.pair a (n + m))).map (· + m)
 
 /-- Helper lemma for the evaluation of `prec` in the base case. -/
 @[simp]
-theorem eval_prec_zero (cf cg : Code) (a : ℕ) : eval (prec cf cg) (Nat.pair a 0) = eval cf a := by
+theorem eval_prec_zero (cf cg : Code) (a : ℕ) : eval O (prec cf cg) (Nat.pair a 0) = eval O cf a := by
   rw [eval, Nat.unpaired, Nat.unpair_pair]
   simp (config := { Lean.Meta.Simp.neutralConfig with proj := true }) only []
   rw [Nat.rec_zero]
 
 /-- Helper lemma for the evaluation of `prec` in the recursive case. -/
 theorem eval_prec_succ (cf cg : Code) (a k : ℕ) :
-    eval (prec cf cg) (Nat.pair a (Nat.succ k)) =
-      do {let ih ← eval (prec cf cg) (Nat.pair a k); eval cg (Nat.pair a (Nat.pair k ih))} := by
+    eval O (prec cf cg) (Nat.pair a (Nat.succ k)) =
+      do {let ih ← eval O (prec cf cg) (Nat.pair a k); eval O cg (Nat.pair a (Nat.pair k ih))} := by
   rw [eval, Nat.unpaired, Part.bind_eq_bind, Nat.unpair_pair]
   simp
 
-instance : Membership (ℕ →. ℕ) Code :=
-  ⟨fun c f => eval c = f⟩
+-- instance : Membership (ℕ →. ℕ) Code :=
+--   ⟨fun c f => eval O c = f⟩
 
 @[simp]
-theorem eval_const : ∀ n m, eval (Code.const n) m = Part.some n
+theorem eval_const : ∀ n m, eval O (Code.const n) m = Part.some n
   | 0, _ => rfl
   | n + 1, m => by simp! [eval_const n m]
 
 @[simp]
-theorem eval_id (n) : eval Code.id n = Part.some n := by simp! [Seq.seq, Code.id]
+theorem eval_id (n) : eval O Code.id n = Part.some n := by simp! [Seq.seq, Code.id]
 
 @[simp]
-theorem eval_curry (c n x) : eval (curry c n) x = eval c (Nat.pair n x) := by simp! [Seq.seq, curry]
+theorem eval_curry (c n x) : eval O (curry c n) x = eval O c (Nat.pair n x) := by simp! [Seq.seq, curry]
 
 theorem const_prim : Primrec Code.const :=
   (_root_.Primrec.id.nat_iterate (_root_.Primrec.const zero)
@@ -514,22 +524,23 @@ theorem curry_inj {c₁ c₂ n₁ n₂} (h : curry c₁ n₁ = curry c₂ n₂) 
     exact const_inj h₃⟩
 
 /--
-The $S_n^m$ theorem: There is a computable function, namely `Nat.Partrec.Code.curry`, that takes a
+The $S_n^m$ theorem: There is a computable function, namely `Nat.RecursiveIn.Code.curry`, that takes a
 program and a ℕ `n`, and returns a new program using `n` as the first argument.
 -/
 theorem smn :
-    ∃ f : Code → ℕ → Code, Computable₂ f ∧ ∀ c n x, eval (f c n) x = eval c (Nat.pair n x) :=
-  ⟨curry, Primrec₂.to_comp curry_prim, eval_curry⟩
+    ∃ f : Code → ℕ → Code, ComputableIn₂ O f ∧ ∀ c n x, eval O (f c n) x = eval O c (Nat.pair n x) :=
+  ⟨curry, Primrec₂.to_compIn curry_prim, eval_curry⟩
 
 /-- A function is partial recursive if and only if there is a code implementing it. Therefore,
 `eval` is a **universal partial recursive function**. -/
-theorem exists_code {f : ℕ →. ℕ} : Nat.Partrec f ↔ ∃ c : Code, eval c = f := by
+theorem exists_code {f : ℕ →. ℕ} : Nat.RecursiveIn O f ↔ ∃ c : Code, eval O c = f := by
   refine ⟨fun h => ?_, ?_⟩
   · induction h with
     | zero => exact ⟨zero, rfl⟩
     | succ => exact ⟨succ, rfl⟩
     | left => exact ⟨left, rfl⟩
     | right => exact ⟨right, rfl⟩
+    | oracle => exact ⟨oracle, rfl⟩
     | pair pf pg hf hg =>
       rcases hf with ⟨cf, rfl⟩; rcases hg with ⟨cg, rfl⟩
       exact ⟨pair cf cg, rfl⟩
@@ -545,20 +556,23 @@ theorem exists_code {f : ℕ →. ℕ} : Nat.Partrec f ↔ ∃ c : Code, eval c 
       simp [eval, Seq.seq, pure, PFun.pure, Part.map_id']
   · rintro ⟨c, rfl⟩
     induction c with
-    | zero => exact Nat.Partrec.zero
-    | succ => exact Nat.Partrec.succ
-    | left => exact Nat.Partrec.left
-    | right => exact Nat.Partrec.right
+    | zero => exact Nat.RecursiveIn.zero
+    | succ => exact Nat.RecursiveIn.succ
+    | left => exact Nat.RecursiveIn.left
+    | right => exact Nat.RecursiveIn.right
+    | oracle => exact Nat.RecursiveIn.oracle
     | pair cf cg pf pg => exact pf.pair pg
     | comp cf cg pf pg => exact pf.comp pg
     | prec cf cg pf pg => exact pf.prec pg
     | rfind' cf pf => exact pf.rfind'
 
-/-- A modified evaluation for the code which returns an `Option ℕ` instead of a `Part ℕ`. To avoid
+/- A modified evaluation for the code which returns an `Option ℕ` instead of a `Part ℕ`. To avoid
 undecidability, `evaln` takes a parameter `k` and fails if it encounters a number ≥ k in the course
-of its execution. Other than this, the semantics are the same as in `Nat.Partrec.Code.eval`.
+of its execution. Other than this, the semantics are the same as in `Nat.RecursiveIn.Code.eval`.
 -/
-def evaln : ℕ → Code → ℕ → Option ℕ
+open Classical in
+noncomputable
+def evaln (O:ℕ→ℕ) : ℕ → Code → ℕ → Option ℕ
   | 0, _ => fun _ => Option.none
   | k + 1, zero => fun n => do
     guard (n ≤ k)
@@ -572,36 +586,41 @@ def evaln : ℕ → Code → ℕ → Option ℕ
   | k + 1, right => fun n => do
     guard (n ≤ k)
     pure n.unpair.2
+  | k + 1, oracle => fun n => do
+    guard (n ≤ k)
+    -- (O n).toOption
+    -- umm. this is a contradiction. um.
+    pure (O n)
   | k + 1, pair cf cg => fun n => do
     guard (n ≤ k)
-    Nat.pair <$> evaln (k + 1) cf n <*> evaln (k + 1) cg n
+    Nat.pair <$> evaln O (k + 1) cf n <*> evaln O (k + 1) cg n
   | k + 1, comp cf cg => fun n => do
     guard (n ≤ k)
-    let x ← evaln (k + 1) cg n
-    evaln (k + 1) cf x
+    let x ← evaln O (k + 1) cg n
+    evaln O (k + 1) cf x
   | k + 1, prec cf cg => fun n => do
     guard (n ≤ k)
     n.unpaired fun a n =>
-      n.casesOn (evaln (k + 1) cf a) fun y => do
-        let i ← evaln k (prec cf cg) (Nat.pair a y)
-        evaln (k + 1) cg (Nat.pair a (Nat.pair y i))
+      n.casesOn (evaln O (k + 1) cf a) fun y => do
+        let i ← evaln O k (prec cf cg) (Nat.pair a y)
+        evaln O (k + 1) cg (Nat.pair a (Nat.pair y i))
   | k + 1, rfind' cf => fun n => do
     guard (n ≤ k)
     n.unpaired fun a m => do
-      let x ← evaln (k + 1) cf (Nat.pair a m)
+      let x ← evaln O (k + 1) cf (Nat.pair a m)
       if x = 0 then
         pure m
       else
-        evaln k (rfind' cf) (Nat.pair a (m + 1))
+        evaln O k (rfind' cf) (Nat.pair a (m + 1))
 
-theorem evaln_bound : ∀ {k c n x}, x ∈ evaln k c n → n < k
+theorem evaln_bound : ∀ {k c n x}, x ∈ evaln O k c n → n < k
   | 0, c, n, x, h => by simp [evaln] at h
   | k + 1, c, n, x, h => by
     suffices ∀ {o : Option ℕ}, x ∈ do { guard (n ≤ k); o } → n < k + 1 by
       cases c <;> rw [evaln] at h <;> exact this h
     simpa [Option.bind_eq_some] using Nat.lt_succ_of_le
 
-theorem evaln_mono : ∀ {k₁ k₂ c n x}, k₁ ≤ k₂ → x ∈ evaln k₁ c n → x ∈ evaln k₂ c n
+theorem evaln_mono : ∀ {k₁ k₂ c n x}, k₁ ≤ k₂ → x ∈ evaln O k₁ c n → x ∈ evaln O k₂ c n
   | 0, k₂, c, n, x, _, h => by simp [evaln] at h
   | k + 1, k₂ + 1, c, n, x, hl, h => by
     have hl' := Nat.le_of_succ_le_succ hl
@@ -616,7 +635,7 @@ theorem evaln_mono : ∀ {k₁ k₂ c n x}, k₁ ≤ k₂ → x ∈ evaln k₁ c
     simp? at h ⊢ says simp only [Option.mem_def] at h ⊢
     induction' c with cf cg hf hg cf cg hf hg cf cg hf hg cf hf generalizing x n <;>
       rw [evaln] at h ⊢ <;> refine this hl' (fun h => ?_) h
-    iterate 4 exact h
+    iterate 5 exact h
     · -- pair cf cg
       simp? [Seq.seq, Option.bind_eq_some] at h ⊢ says
         simp only [Seq.seq, Option.map_eq_map, Option.mem_def, Option.bind_eq_some,
@@ -640,13 +659,13 @@ theorem evaln_mono : ∀ {k₁ k₂ c n x}, k₁ ≤ k₂ → x ∈ evaln k₁ c
       by_cases x0 : x = 0 <;> simp [x0]
       exact evaln_mono hl'
 
-theorem evaln_sound : ∀ {k c n x}, x ∈ evaln k c n → x ∈ eval c n
+theorem evaln_sound : ∀ {k c n x}, x ∈ evaln O k c n → x ∈ eval O c n
   | 0, _, n, x, h => by simp [evaln] at h
   | k + 1, c, n, x, h => by
     induction' c with cf cg hf hg cf cg hf hg cf cg hf hg cf hf generalizing x n <;>
         simp [eval, evaln, Option.bind_eq_some, Seq.seq] at h ⊢ <;>
       obtain ⟨_, h⟩ := h
-    iterate 4 simpa [pure, PFun.pure, eq_comm] using h
+    iterate 5 simpa [pure, PFun.pure, eq_comm] using h
     · -- pair cf cg
       rcases h with ⟨y, ef, z, eg, rfl⟩
       exact ⟨_, hf _ _ ef, _, hg _ _ eg, rfl⟩
@@ -678,9 +697,9 @@ theorem evaln_sound : ∀ {k c n x}, x ∈ evaln k c n → x ∈ eval c n
         · rcases hy₂ (Nat.lt_of_succ_lt_succ im) with ⟨z, hz, z0⟩
           exact ⟨z, by simpa [add_comm, add_left_comm] using hz, z0⟩
 
-theorem evaln_complete {c n x} : x ∈ eval c n ↔ ∃ k, x ∈ evaln k c n := by
+theorem evaln_complete {c n x} : x ∈ eval O c n ↔ ∃ k, x ∈ evaln O k c n := by
   refine ⟨fun h => ?_, fun ⟨k, h⟩ => evaln_sound h⟩
-  rsuffices ⟨k, h⟩ : ∃ k, x ∈ evaln (k + 1) c n
+  rsuffices ⟨k, h⟩ : ∃ k, x ∈ evaln O (k + 1) c n
   · exact ⟨k + 1, h⟩
   induction c generalizing n x with
       simp [eval, evaln, pure, PFun.pure, Seq.seq, Option.bind_eq_some] at h ⊢
@@ -716,12 +735,13 @@ theorem evaln_complete {c n x} : x ∈ eval c n ↔ ∃ k, x ∈ evaln k c n := 
             le_trans (le_max_left _ (Nat.pair n₁ m)) nk₁, y,
           evaln_mono (Nat.succ_le_succ <| le_max_left _ _) ?_,
           evaln_mono (Nat.succ_le_succ <| Nat.le_succ_of_le <| le_max_right _ _) hk₂⟩
-      simp only [evaln.eq_8, bind, unpaired, unpair_pair, Option.mem_def, Option.bind_eq_some,
+      simp only [evaln, bind, unpaired, unpair_pair, Option.mem_def, Option.bind_eq_some,
         Option.guard_eq_some', exists_and_left, exists_const]
       exact ⟨le_trans (le_max_right _ _) nk₁, hk₁⟩
+
   | rfind' cf hf =>
     rcases h with ⟨y, ⟨hy₁, hy₂⟩, rfl⟩
-    suffices ∃ k, y + n.unpair.2 ∈ evaln (k + 1) (rfind' cf) (Nat.pair n.unpair.1 n.unpair.2) by
+    suffices ∃ k, y + n.unpair.2 ∈ evaln O (k + 1) (rfind' cf) (Nat.pair n.unpair.1 n.unpair.2) by
       simpa [evaln, Option.bind_eq_some]
     revert hy₁ hy₂
     generalize n.unpair.2 = m
@@ -751,28 +771,29 @@ section
 open Primrec
 
 private def lup (L : List (List (Option ℕ))) (p : ℕ × Code) (n : ℕ) := do
-  let l ← L.get? (encode p)
-  let o ← l.get? n
+  let l ← L[(encode p)]?
+  let o ← l[n]?
   o
 
 private theorem hlup : Primrec fun p : _ × (_ × _) × _ => lup p.1 p.2.1 p.2.2 :=
   Primrec.option_bind
-    (Primrec.list_get?.comp Primrec.fst (Primrec.encode.comp <| Primrec.fst.comp Primrec.snd))
-    (Primrec.option_bind (Primrec.list_get?.comp Primrec.snd <| Primrec.snd.comp <|
+    (Primrec.list_getElem?.comp Primrec.fst (Primrec.encode.comp <| Primrec.fst.comp Primrec.snd))
+    (Primrec.option_bind (Primrec.list_getElem?.comp Primrec.snd <| Primrec.snd.comp <|
       Primrec.snd.comp Primrec.fst) Primrec.snd)
 
-private def G (L : List (List (Option ℕ))) : Option (List (Option ℕ)) :=
+private def G (O:ℕ→ℕ) (L : List (List (Option ℕ))) : Option (List (Option ℕ)) :=
   Option.some <|
     let a := ofNat (ℕ × Code) L.length
     let k := a.1
     let c := a.2
     (List.range k).map fun n =>
       k.casesOn Option.none fun k' =>
-        Nat.Partrec.Code.recOn c
+        Nat.RecursiveIn.Code.recOn c
           (some 0) -- zero
           (some (Nat.succ n))
           (some n.unpair.1)
           (some n.unpair.2)
+          (some (O n)) -- oracle
           (fun cf cg _ _ => do
             let x ← lup L (k, cf) n
             let y ← lup L (k, cg) n
@@ -804,11 +825,12 @@ private theorem hG : Primrec G := by
   have k' := Primrec.snd (α := List (List (Option ℕ)) × ℕ) (β := ℕ)
   have c := Primrec.snd.comp (a.comp <| (Primrec.fst (β := ℕ)).comp (Primrec.fst (β := ℕ)))
   apply
-    Nat.Partrec.Code.rec_prim c
+    Nat.RecursiveIn.Code.rec_prim c
       (_root_.Primrec.const (some 0))
       (Primrec.option_some.comp (_root_.Primrec.succ.comp n))
       (Primrec.option_some.comp (Primrec.fst.comp <| Primrec.unpair.comp n))
       (Primrec.option_some.comp (Primrec.snd.comp <| Primrec.unpair.comp n))
+      (_root_.Primrec.const (some 72))
   · have L := (Primrec.fst.comp Primrec.fst).comp
       (Primrec.fst (α := (List (List (Option ℕ)) × ℕ) × ℕ)
         (β := Code × Code × Option ℕ × Option ℕ))
@@ -895,21 +917,30 @@ private theorem hG : Primrec G := by
       Primrec.fst
 
 private theorem evaln_map (k c n) :
-    ((List.range k)[n]?.bind fun a ↦ evaln k c a) = evaln k c n := by
+    ((List.range k)[n]?.bind fun a ↦ evaln O k c a) = evaln O k c n := by
   by_cases kn : n < k
   · simp [List.getElem?_range kn]
   · rw [List.getElem?_eq_none]
-    · cases e : evaln k c n
+    · cases e : evaln O k c n
       · rfl
       exact kn.elim (evaln_bound e)
     simpa using kn
 
-/-- The `Nat.Partrec.Code.evaln` function is primitive recursive. -/
-theorem evaln_prim : Primrec fun a : (ℕ × Code) × ℕ => evaln a.1.1 a.1.2 a.2 :=
+
+
+
+
+
+
+
+/-- The `Nat.RecursiveIn.Code.evaln` function is primitive recursive. -/
+
+
+theorem evaln_prim : PrimrecIn O fun a : (ℕ × Code) × ℕ => evaln O a.1.1 a.1.2 a.2 :=
   have :
     Primrec₂ fun (_ : Unit) (n : ℕ) =>
       let a := ofNat (ℕ × Code) n
-      (List.range a.1).map (evaln a.1 a.2) :=
+      (List.range a.1).map (evaln O a.1 a.2) :=
     Primrec.nat_strong_rec _ (hG.comp Primrec.snd).to₂ fun _ p => by
       simp only [G, prod_ofNat_val, ofNat_nat, List.length_map, List.length_range,
         Nat.pair_unpair, Option.some_inj]
@@ -929,20 +960,21 @@ theorem evaln_prim : Primrec fun a : (ℕ × Code) × ℕ => evaln a.1.1 a.1.2 a
         ∀ {k' c' n},
           Nat.pair k' (encode c') < Nat.pair k (encode c) →
             lup ((List.range (Nat.pair k (encode c))).map fun n =>
-              (List.range n.unpair.1).map (evaln n.unpair.1 (ofNat Code n.unpair.2))) (k', c') n =
-            evaln k' c' n := by
+              (List.range n.unpair.1).map (evaln O n.unpair.1 (ofNat Code n.unpair.2))) (k', c') n =
+            evaln O k' c' n := by
         intro k₁ c₁ n₁ hl
         simp [lup, List.getElem?_range hl, evaln_map, Bind.bind, Option.bind_map]
-      obtain - | - | - | - | ⟨cf, cg⟩ | ⟨cf, cg⟩ | ⟨cf, cg⟩ | cf := c <;>
+      obtain - | - | - | - | - | ⟨cf, cg⟩ | ⟨cf, cg⟩ | ⟨cf, cg⟩ | cf := c <;>
         simp [evaln, nk, Bind.bind, Functor.map, Seq.seq, pure]
+      · sorry
       · obtain ⟨lf, lg⟩ := encode_lt_pair cf cg
         rw [hg (Nat.pair_lt_pair_right _ lf), hg (Nat.pair_lt_pair_right _ lg)]
-        cases evaln k cf n
+        cases evaln O k cf n
         · rfl
-        cases evaln k cg n <;> rfl
+        cases evaln O k cg n <;> rfl
       · obtain ⟨lf, lg⟩ := encode_lt_comp cf cg
         rw [hg (Nat.pair_lt_pair_right _ lg)]
-        cases evaln k cg n
+        cases evaln O k cg n
         · rfl
         simp [k, hg (Nat.pair_lt_pair_right _ lf)]
       · obtain ⟨lf, lg⟩ := encode_lt_prec cf cg
@@ -951,18 +983,18 @@ theorem evaln_prim : Primrec fun a : (ℕ × Code) × ℕ => evaln a.1.1 a.1.2 a
         · rfl
         simp only [decode_eq_ofNat, Option.some.injEq]
         rw [hg (Nat.pair_lt_pair_left _ k'.lt_succ_self)]
-        cases evaln k' _ _
+        cases evaln O k' _ _
         · rfl
         simp [k, hg (Nat.pair_lt_pair_right _ lg)]
       · have lf := encode_lt_rfind' cf
         rw [hg (Nat.pair_lt_pair_right _ lf)]
-        rcases evaln k cf n with - | x
+        rcases evaln O k cf n with - | x
         · rfl
         simp only [decode_eq_ofNat, Option.some.injEq, Option.some_bind]
         cases x <;> simp [Nat.succ_ne_zero]
         rw [hg (Nat.pair_lt_pair_left _ k'.lt_succ_self)]
   (Primrec.option_bind
-    (Primrec.list_get?.comp (this.comp (_root_.Primrec.const ())
+    (Primrec.list_getElem?.comp (this.comp (_root_.Primrec.const ())
       (Primrec.encode_iff.2 Primrec.fst)) Primrec.snd) Primrec.snd.to₂).of_eq
     fun ⟨⟨k, c⟩, n⟩ => by simp [evaln_map, Option.bind_map]
 
@@ -970,56 +1002,56 @@ end
 
 section
 
-open Partrec Computable
+open RecursiveIn ComputableIn
 
-theorem eval_eq_rfindOpt (c n) : eval c n = Nat.rfindOpt fun k => evaln k c n :=
+theorem eval_eq_rfindOpt (c n) : eval O c n = Nat.rfindOpt fun k => evaln O k c n :=
   Part.ext fun x => by
     refine evaln_complete.trans (Nat.rfindOpt_mono ?_).symm
     intro a m n hl; apply evaln_mono hl
 
-theorem eval_part : Partrec₂ eval :=
-  (Partrec.rfindOpt
-    (evaln_prim.to_comp.comp ((Computable.snd.pair (fst.comp fst)).pair (snd.comp fst))).to₂).of_eq
+theorem eval_part : RecursiveIn O₂ (eval O) :=
+  (RecursiveIn.rfindOpt
+    (evaln_prim.to_compIn.comp ((ComputableIn.snd.pair (fst.comp fst)).pair (snd.comp fst))).to₂).of_eq
     fun a => by simp [eval_eq_rfindOpt]
 
 /-- **Roger's fixed-point theorem**: any total, computable `f` has a fixed point.
-That is, under the interpretation given by `Nat.Partrec.Code.eval`, there is a code `c`
+That is, under the interpretation given by `Nat.RecursiveIn.Code.eval`, there is a code `c`
 such that `c` and `f c` have the same evaluation.
 -/
-theorem fixed_point {f : Code → Code} (hf : Computable f) : ∃ c : Code, eval (f c) = eval c :=
-  let g (x y : ℕ) : Part ℕ := eval (ofNat Code x) x >>= fun b => eval (ofNat Code b) y
-  have : Partrec₂ g :=
-    (eval_part.comp ((Computable.ofNat _).comp fst) fst).bind
-      (eval_part.comp ((Computable.ofNat _).comp snd) (snd.comp fst)).to₂
+theorem fixed_point {f : Code → Code} (hf : ComputableIn O f) : ∃ c : Code, eval O (f c) = eval O c :=
+  let g (x y : ℕ) : Part ℕ := eval O (ofNat Code x) x >>= fun b => eval O (ofNat Code b) y
+  have : RecursiveIn O₂ g :=
+    (eval_part.comp ((ComputableIn.ofNat _).comp fst) fst).bind
+      (eval_part.comp ((ComputableIn.ofNat _).comp snd) (snd.comp fst)).to₂
   let ⟨cg, eg⟩ := exists_code.1 this
-  have eg' : ∀ a n, eval cg (Nat.pair a n) = Part.map encode (g a n) := by simp [eg]
+  have eg' : ∀ a n, eval O cg (Nat.pair a n) = Part.map encode (g a n) := by simp [eg]
   let F (x : ℕ) : Code := f (curry cg x)
-  have : Computable F :=
-    hf.comp (curry_prim.comp (_root_.Primrec.const cg) _root_.Primrec.id).to_comp
+  have : ComputableIn O F :=
+    hf.comp (curry_prim.comp (_root_.Primrec.const cg) _root_.Primrec.id).to_compIn
   let ⟨cF, eF⟩ := exists_code.1 this
-  have eF' : eval cF (encode cF) = Part.some (encode (F (encode cF))) := by simp [eF]
+  have eF' : eval O cF (encode cF) = Part.some (encode (F (encode cF))) := by simp [eF]
   ⟨curry cg (encode cF),
     funext fun n =>
-      show eval (f (curry cg (encode cF))) n = eval (curry cg (encode cF)) n by
+      show eval O (f (curry cg (encode cF))) n = eval O (curry cg (encode cF)) n by
         simp [F, g, eg', eF', Part.map_id']⟩
 
 /-- **Kleene's second recursion theorem** -/
-theorem fixed_point₂ {f : Code → ℕ →. ℕ} (hf : Partrec₂ f) : ∃ c : Code, eval c = f c :=
+theorem fixed_point₂ {f : Code → ℕ →. ℕ} (hf : RecursiveIn O₂ f) : ∃ c : Code, eval O c = f c :=
   let ⟨cf, ef⟩ := exists_code.1 hf
-  (fixed_point (curry_prim.comp (_root_.Primrec.const cf) Primrec.encode).to_comp).imp fun c e =>
+  (fixed_point (curry_prim.comp (_root_.Primrec.const cf) Primrec.encode).to_compIn).imp fun c e =>
     funext fun n => by simp [e.symm, ef, Part.map_id']
 
 end
 
 /-- There are only countably many partial recursive partial functions `ℕ →. ℕ`. -/
-instance : Countable {f : ℕ →. ℕ // _root_.Partrec f} := by
-  apply Function.Surjective.countable (f := fun c => ⟨eval c, eval_part.comp (.const c) .id⟩)
+instance : Countable {f : ℕ →. ℕ // _root_.RecursiveIn O f} := by
+  apply Function.Surjective.countable (f := fun c => ⟨eval O c, eval_part.comp (.const c) .id⟩)
   intro ⟨f, hf⟩; simpa using exists_code.1 hf
 
 /-- There are only countably many computable functions `ℕ → ℕ`. -/
-instance : Countable {f : ℕ → ℕ // Computable f} :=
-  @Function.Injective.countable {f : ℕ → ℕ // Computable f} {f : ℕ →. ℕ // _root_.Partrec f} _
+instance : Countable {f : ℕ → ℕ // ComputableIn O f} :=
+  @Function.Injective.countable {f : ℕ → ℕ // ComputableIn O f} {f : ℕ →. ℕ // _root_.RecursiveIn O f} _
     (fun f => ⟨f.val, f.2⟩)
     (fun _ _ h => Subtype.val_inj.1 (PFun.lift_injective (by simpa using h)))
 
-end Nat.Partrec.Code
+end Nat.RecursiveIn.Code
