Computability/SingleOracle/Encoding2.lean
@@ -1,0 +1,1062 @@
+import Computability.SingleOracle.TuringDegree
+
+-- import Mathlib.Computability.RecursiveIn O
+import Mathlib.Data.Option.Basic
+
+-- set_option maxHeartbeats 20000000
+
+
+
+
+open Encodable Denumerable
+-- open ComputableIn O
+
+
+namespace Nat.RecursiveIn
+
+#check Computable.comp
+
+theorem rfind' {f} (hf : Nat.RecursiveIn O f) :
+    Nat.RecursiveIn O
+      (Nat.unpaired fun a m =>
+        (Nat.rfind fun n => (fun m => m = 0) <$> f (Nat.pair a (n + m))).map (· + m)) :=
+  RecursiveIn₂.unpaired'.2 <| by
+    refine
+      RecursiveIn.map
+        ((@RecursiveIn₂.unpaired' O fun a b : ℕ =>
+              Nat.rfind fun n => (fun m => m = 0) <$> f (Nat.pair a (n + b))).1
+          ?_)
+        (PrimrecIn.nat_add.comp PrimrecIn.snd <| PrimrecIn.snd.comp PrimrecIn.fst).to_compIn.to₂
+        -- (ComputableIn.to₂ (ComputableIn O₂.to_compIn (PrimrecIn.nat_add.comp PrimrecIn.snd <| PrimrecIn.snd.comp PrimrecIn.fst)))
+    have : Nat.RecursiveIn O (fun a => Nat.rfind (fun n => (fun m => decide (m = 0)) <$>
+      Nat.unpaired (fun a b => f (Nat.pair (Nat.unpair a).1 (b + (Nat.unpair a).2)))
+        (Nat.pair a n))) :=
+      rfind
+        (RecursiveIn₂.unpaired'.2
+          ((RecursiveIn.nat_iff.2 hf).comp
+              (PrimrecIn₂.pair.comp (PrimrecIn.fst.comp <| PrimrecIn.unpair.comp PrimrecIn.fst)
+                  (PrimrecIn.nat_add.comp PrimrecIn.snd
+                    (PrimrecIn.snd.comp <| PrimrecIn.unpair.comp PrimrecIn.fst))).to_compIn))
+    simpa
+
+inductive Code : Type
+| zero : Code
+| succ : Code
+| left : Code
+| right : Code
+| oracle : Code
+| pair : Code → Code → Code
+| comp : Code → Code → Code
+| prec : Code → Code → Code
+| rfind' : Code → Code
+
+
+compile_inductive% Code
+
+end Nat.RecursiveIn
+
+namespace Nat.RecursiveIn.Code
+
+instance instInhabited : Inhabited Code :=
+  ⟨zero⟩
+
+/-- Returns a code for the constant function outputting a particular natural. -/
+protected def const : ℕ → Code
+  | 0 => zero
+  | n + 1 => comp succ (Code.const n)
+
+theorem const_inj : ∀ {n₁ n₂}, Nat.RecursiveIn.Code.const n₁ = Nat.RecursiveIn.Code.const n₂ → n₁ = n₂
+  | 0, 0, _ => by simp
+  | n₁ + 1, n₂ + 1, h => by
+    dsimp [Nat.RecursiveIn.Code.const] at h
+    injection h with h₁ h₂
+    simp only [const_inj h₂]
+
+/-- A code for the identity function. -/
+protected def id : Code :=
+  pair left right
+
+/-- Given a code `c` taking a pair as input, returns a code using `n` as the first argument to `c`.
+-/
+def curry (c : Code) (n : ℕ) : Code :=
+  comp c (pair (Code.const n) Code.id)
+
+
+
+
+
+
+
+
+
+
+def encodeCode : Code → ℕ
+| Code.zero        => 0
+| Code.succ        => 1
+| Code.left        => 2
+| Code.right       => 3
+| Code.oracle      => 4
+| Code.pair cf cg  => 2*(2*(Nat.pair (encodeCode cf) (encodeCode cg))  )   + 5
+| Code.comp cf cg  => 2*(2*(Nat.pair (encodeCode cf) (encodeCode cg))  )+1 + 5
+| Code.prec cf cg  => 2*(2*(Nat.pair (encodeCode cf) (encodeCode cg))+1)   + 5
+| Code.rfind' cf   => 2*(2*(encodeCode cf                            )+1)+1 + 5
+
+/--
+Procedure for decoding:
+
+If n≤4. trivial.
+
+Otherwise if n≥5, check n%4. The 4 possible values correspond to
+pair
+comp
+prec
+rfind'
+-/
+def decodeCode : ℕ → Code
+| 0 => Code.zero
+| 1 => Code.succ
+| 2 => Code.left
+| 3 => Code.right
+| 4 => Code.oracle
+| n + 5 =>
+  let m := n.div2.div2
+  have hm : m < n + 5 := by
+    simp only [m, Nat.div2_val]
+    exact
+      lt_of_le_of_lt (le_trans (Nat.div_le_self _ _) (Nat.div_le_self _ _))
+        (Nat.succ_le_succ (Nat.le_add_right _ _))
+  have _m1 : m.unpair.1 < n + 5 := lt_of_le_of_lt m.unpair_left_le hm
+  have _m2 : m.unpair.2 < n + 5 := lt_of_le_of_lt m.unpair_right_le hm
+  match n.bodd, n.div2.bodd with
+  | false, false => Code.pair (decodeCode m.unpair.1) (decodeCode m.unpair.2) -- n%4=0
+  | true , false => Code.comp (decodeCode m.unpair.1) (decodeCode m.unpair.2) -- n%4=1
+  | false, true  => Code.prec (decodeCode m.unpair.1) (decodeCode m.unpair.2) -- n%4=2
+  | true , true  => Code.rfind' (decodeCode m)                                 -- n%4=3
+
+instance : OfNat (Code) m where ofNat := decodeCode m
+instance : Coe ℕ Code := ⟨decodeCode⟩
+instance : Coe Code ℕ := ⟨encodeCode⟩
+/-- Converts an `Code` into a `ℕ`. -/ @[coe] def ofCode : Code → ℕ := encodeCode
+abbrev ofNatCode := decodeCode
+@[simp] theorem decodeCode_encodeCode : ∀ c, decodeCode (encodeCode c) = c := fun c => by
+  induction c <;> (simp [encodeCode, decodeCode, Nat.div2_val, *])
+@[simp] theorem encodeCode_decodeCode : ∀ c, encodeCode (decodeCode c) = c :=
+λ c => match c with
+  | 0 => by simp only [decodeCode, encodeCode]
+  | 1 => by simp only [decodeCode, encodeCode]
+  | 2 => by simp only [decodeCode, encodeCode]
+  | 3 => by simp only [decodeCode, encodeCode]
+  | 4 => by simp only [decodeCode, encodeCode]
+  | n + 5 => by
+    let m := n.div2.div2
+    have hm : m < n + 5 := by
+      simp only [m, Nat.div2_val]
+      exact lt_of_le_of_lt (le_trans (Nat.div_le_self _ _) (Nat.div_le_self _ _)) (Nat.succ_le_succ (Nat.le_add_right _ _))
+    have _m1 : m.unpair.1 < n + 5 := lt_of_le_of_lt m.unpair_left_le hm
+    have _m2 : m.unpair.2 < n + 5 := lt_of_le_of_lt m.unpair_right_le hm
+    have IH := encodeCode_decodeCode m
+    have IH1 := encodeCode_decodeCode m.unpair.1
+    have IH2 := encodeCode_decodeCode m.unpair.2
+    conv_rhs => rw [← Nat.bit_decomp n, ← Nat.bit_decomp n.div2]
+    simp only [decodeCode.eq_6]
+    cases n.bodd <;> cases n.div2.bodd <;> simp [m, encodeCode, IH, IH1, IH2, Nat.bit_val]
+instance instDenumerable : Denumerable Code := mk' ⟨encodeCode, decodeCode, decodeCode_encodeCode, encodeCode_decodeCode⟩
+
+
+
+
+/-- Proof that `Nat.RecursiveIn.Code.ofNatCode` is the inverse of `Nat.RecursiveIn.Code.encodeCode` -/
+private theorem encode_ofNatCode : ∀ n, encodeCode (ofNatCode n) = n := by exact fun n ↦encodeCode_decodeCode n
+
+
+theorem encodeCode_eq : encode = encodeCode :=
+  rfl
+
+theorem ofNatCode_eq : ofNat Code = ofNatCode :=
+  rfl
+
+theorem encode_lt_pair (cf cg) :
+    encode cf < encode (pair cf cg) ∧ encode cg < encode (pair cf cg) := by
+  simp only [encodeCode_eq, encodeCode]
+  have := Nat.mul_le_mul_right (Nat.pair cf.encodeCode cg.encodeCode) (by decide : 1 ≤ 2 * 2)
+  rw [one_mul, mul_assoc] at this
+  have := lt_of_le_of_lt this (lt_add_of_pos_right _ (by decide : 0 < 5))
+  exact ⟨lt_of_le_of_lt (Nat.left_le_pair _ _) this, lt_of_le_of_lt (Nat.right_le_pair _ _) this⟩
+
+theorem encode_lt_comp (cf cg) :
+    encode cf < encode (comp cf cg) ∧ encode cg < encode (comp cf cg) := by
+  have : encode (pair cf cg) < encode (comp cf cg) := by simp [encodeCode_eq, encodeCode]
+  exact (encode_lt_pair cf cg).imp (fun h => lt_trans h this) fun h => lt_trans h this
+
+theorem encode_lt_prec (cf cg) :
+    encode cf < encode (prec cf cg) ∧ encode cg < encode (prec cf cg) := by
+  have : encode (pair cf cg) < encode (prec cf cg) := by simp [encodeCode_eq, encodeCode]
+  exact (encode_lt_pair cf cg).imp (fun h => lt_trans h this) fun h => lt_trans h this
+
+theorem encode_lt_rfind' (cf) : encode cf < encode (rfind' cf) := by
+  simp only [encodeCode_eq, encodeCode]
+  omega
+
+end Nat.RecursiveIn.Code
+
+section
+open PrimrecIn
+namespace Nat.RecursiveIn.Code
+
+theorem pair_prim : PrimrecIn₂ O pair :=
+  PrimrecIn₂.ofNat_iff.2 <|
+    PrimrecIn₂.encode_iff.1 <|
+      nat_add.comp
+        (nat_double.comp <|
+          nat_double.comp <|
+            PrimrecIn₂.natPair.comp (encode_iff.2 <| (PrimrecIn.ofNat Code).comp fst)
+              (encode_iff.2 <| (PrimrecIn.ofNat Code).comp snd))
+        (PrimrecIn₂.const 5)
+
+theorem comp_prim : PrimrecIn₂ O comp :=
+  PrimrecIn₂.ofNat_iff.2 <|
+    PrimrecIn₂.encode_iff.1 <|
+      nat_add.comp
+        (
+          nat_double_succ.comp <|
+          nat_double.comp <|
+            PrimrecIn₂.natPair.comp (encode_iff.2 <| (PrimrecIn.ofNat Code).comp fst)
+              (encode_iff.2 <| (PrimrecIn.ofNat Code).comp snd))
+        (PrimrecIn₂.const 5)
+
+theorem prec_prim : PrimrecIn₂ O prec :=
+  PrimrecIn₂.ofNat_iff.2 <|
+    PrimrecIn₂.encode_iff.1 <|
+      nat_add.comp
+        (
+          nat_double.comp <|
+          nat_double_succ.comp <|
+            PrimrecIn₂.natPair.comp (encode_iff.2 <| (PrimrecIn.ofNat Code).comp fst)
+              (encode_iff.2 <| (PrimrecIn.ofNat Code).comp snd))
+        (PrimrecIn₂.const 5)
+
+theorem rfind_prim : PrimrecIn O rfind' :=
+  ofNat_iff.2 <|
+    encode_iff.1 <|
+      nat_add.comp
+        (nat_double_succ.comp <| nat_double_succ.comp <|
+          encode_iff.2 <| PrimrecIn.ofNat Code)
+        (const 5)
+
+theorem rec_prim' {α σ} [Primcodable α] [Primcodable σ] {c : α → Code} (hc : PrimrecIn O c) {z : α → σ}
+    (hz : PrimrecIn O z) {s : α → σ} (hs : PrimrecIn O s) {l : α → σ} (hl : PrimrecIn O l) {r : α → σ}
+    (hr : PrimrecIn O r)
+    {o : α → σ} (ho : PrimrecIn O o)
+    {pr : α → Code × Code × σ × σ → σ} (hpr : PrimrecIn₂ O pr)
+    {co : α → Code × Code × σ × σ → σ} (hco : PrimrecIn₂ O co) {pc : α → Code × Code × σ × σ → σ}
+    (hpc : PrimrecIn₂ O pc) {rf : α → Code × σ → σ} (hrf : PrimrecIn₂ O rf) :
+    let PR (a) cf cg hf hg := pr a (cf, cg, hf, hg)
+    let CO (a) cf cg hf hg := co a (cf, cg, hf, hg)
+    let PC (a) cf cg hf hg := pc a (cf, cg, hf, hg)
+    let RF (a) cf hf := rf a (cf, hf)
+    let F (a : α) (c : Code) : σ :=
+      Nat.RecursiveIn.Code.recOn c (z a) (s a) (l a) (r a) (o a) (PR a) (CO a) (PC a) (RF a)
+    PrimrecIn O (fun a => F a (c a) : α → σ) := by
+  intros _ _ _ _ F
+  let G₁ : (α × List σ) × ℕ × ℕ → Option σ := fun p =>
+    letI a := p.1.1; letI IH := p.1.2; letI n := p.2.1; letI m := p.2.2
+    (IH[m]?).bind fun s =>
+    (IH[m.unpair.1]?).bind fun s₁ =>
+    (IH[m.unpair.2]?).map fun s₂ =>
+    cond n.bodd
+      (cond n.div2.bodd (rf a (ofNat Code m, s))
+        (co a (ofNat Code m.unpair.1, ofNat Code m.unpair.2, s₁, s₂)))
+      (cond n.div2.bodd (pc a (ofNat Code m.unpair.1, ofNat Code m.unpair.2, s₁, s₂))
+        (pr a (ofNat Code m.unpair.1, ofNat Code m.unpair.2, s₁, s₂)))
+  have : PrimrecIn O G₁ :=
+    option_bind (list_getElem?.comp (snd.comp fst) (snd.comp snd)) <| .mk <|
+    option_bind ((list_getElem?.comp (snd.comp fst)
+      (fst.comp <| PrimrecIn.unpair.comp (snd.comp snd))).comp fst) <| .mk <|
+    option_map ((list_getElem?.comp (snd.comp fst)
+      (snd.comp <| PrimrecIn.unpair.comp (snd.comp snd))).comp <| fst.comp fst) <| .mk <|
+    have a := fst.comp (fst.comp <| fst.comp <| fst.comp fst)
+    have n := fst.comp (snd.comp <| fst.comp <| fst.comp fst)
+    have m := snd.comp (snd.comp <| fst.comp <| fst.comp fst)
+    have m₁ := fst.comp (PrimrecIn.unpair.comp m)
+    have m₂ := snd.comp (PrimrecIn.unpair.comp m)
+    have s := snd.comp (fst.comp fst)
+    have s₁ := snd.comp fst
+    have s₂ := snd
+    (nat_bodd.comp n).cond
+      ((nat_bodd.comp <| nat_div2.comp n).cond
+        (hrf.comp a (((PrimrecIn.ofNat Code).comp m).pair s))
+        (hco.comp a (((PrimrecIn.ofNat Code).comp m₁).pair <| ((PrimrecIn.ofNat Code).comp m₂).pair <| s₁.pair s₂)))
+      (PrimrecIn.cond (nat_bodd.comp <| nat_div2.comp n)
+        (hpc.comp a (((PrimrecIn.ofNat Code).comp m₁).pair <| ((PrimrecIn.ofNat Code).comp m₂).pair <| s₁.pair s₂))
+        (hpr.comp a (((PrimrecIn.ofNat Code).comp m₁).pair <| ((PrimrecIn.ofNat Code).comp m₂).pair <| s₁.pair s₂)))
+  let G : α → List σ → Option σ := fun a IH =>
+    IH.length.casesOn (some (z a)) fun n =>
+    n.casesOn (some (s a)) fun n =>
+    n.casesOn (some (l a)) fun n =>
+    n.casesOn (some (r a)) fun n =>
+    n.casesOn (some (o a)) fun n =>
+    G₁ ((a, IH), n, n.div2.div2)
+  have : PrimrecIn₂ O G := .mk <|
+    nat_casesOn (list_length.comp snd) (option_some_iff.2 (hz.comp fst)) <| .mk <|
+    nat_casesOn snd (option_some_iff.2 (hs.comp (fst.comp fst))) <| .mk <|
+    nat_casesOn snd (option_some_iff.2 (hl.comp (fst.comp <| fst.comp fst))) <| .mk <|
+    nat_casesOn snd (option_some_iff.2 (hr.comp (fst.comp <| fst.comp <| fst.comp fst))) <| .mk <|
+    nat_casesOn snd (option_some_iff.2 (ho.comp (fst.comp <| fst.comp <| fst.comp <| fst.comp fst))) <| .mk <|
+    this.comp <|
+      -- ((fst.pair snd).comp <| fst.comp <| fst.comp <| fst.comp <| fst).pair <|
+      ((fst.pair snd).comp <| fst.comp <| fst.comp <| fst.comp <| fst.comp <| fst).pair <|
+      snd.pair <| nat_div2.comp <| nat_div2.comp snd
+  refine (nat_strong_rec (fun a n => F a (ofNat Code n)) this.to₂ fun a n => ?_)
+    |>.comp .id (encode_iff.2 hc) |>.of_eq fun a => by simp
+  iterate 5 rcases n with - | n; · simp [ofNatCode_eq, ofNatCode, decodeCode]; rfl
+  -- · simp [ofNatCode_eq, ofNatCode, decodeCode];
+  --   exact?
+  simp only [G]; rw [List.length_map, List.length_range]
+  let m := n.div2.div2
+  show G₁ ((a, (List.range (n + 5)).map fun n => F a (ofNat Code n)), n, m)
+    = some (F a (ofNat Code (n + 5)))
+  have hm : m < n + 5 := by
+    simp only [m, div2_val]
+    exact lt_of_le_of_lt
+      (le_trans (Nat.div_le_self ..) (Nat.div_le_self ..))
+      (Nat.succ_le_succ (Nat.le_add_right ..))
+  have m1 : m.unpair.1 < n + 5 := lt_of_le_of_lt m.unpair_left_le hm
+  have m2 : m.unpair.2 < n + 5 := lt_of_le_of_lt m.unpair_right_le hm
+  simp [G₁, m, List.getElem?_map, List.getElem?_range, hm, m1, m2]
+  rw [show ofNat Code (n + 5) = ofNatCode (n + 5) from rfl]
+  unfold decodeCode
+  simp
+  cases n.bodd <;> cases n.div2.bodd <;> rfl
+
+
+/-- Recursion on `Nat.RecursiveIn.Code` is primitive recursive. -/
+theorem rec_prim {α σ} [Primcodable α] [Primcodable σ] {c : α → Code} (hc : PrimrecIn O c) {z : α → σ}
+    (hz : PrimrecIn O z) {s : α → σ} (hs : PrimrecIn O s) {l : α → σ} (hl : PrimrecIn O l) {r : α → σ}
+    (hr : PrimrecIn O r) {o : α → σ}
+    (ho : PrimrecIn O o) {pr : α → Code → Code → σ → σ → σ}
+    (hpr : PrimrecIn O fun a : α × Code × Code × σ × σ => pr a.1 a.2.1 a.2.2.1 a.2.2.2.1 a.2.2.2.2)
+    {co : α → Code → Code → σ → σ → σ}
+    (hco : PrimrecIn O fun a : α × Code × Code × σ × σ => co a.1 a.2.1 a.2.2.1 a.2.2.2.1 a.2.2.2.2)
+    {pc : α → Code → Code → σ → σ → σ}
+    (hpc : PrimrecIn O fun a : α × Code × Code × σ × σ => pc a.1 a.2.1 a.2.2.1 a.2.2.2.1 a.2.2.2.2)
+    {rf : α → Code → σ → σ} (hrf : PrimrecIn O fun a : α × Code × σ => rf a.1 a.2.1 a.2.2) :
+    let F (a : α) (c : Code) : σ :=
+      Nat.RecursiveIn.Code.recOn c (z a) (s a) (l a) (r a) (o a) (pr a) (co a) (pc a) (rf a)
+    PrimrecIn O fun a => F a (c a) :=
+  rec_prim' hc hz hs hl hr ho
+    (pr := fun a b => pr a b.1 b.2.1 b.2.2.1 b.2.2.2) (.mk hpr)
+    (co := fun a b => co a b.1 b.2.1 b.2.2.1 b.2.2.2) (.mk hco)
+    (pc := fun a b => pc a b.1 b.2.1 b.2.2.1 b.2.2.2) (.mk hpc)
+    (rf := fun a b => rf a b.1 b.2) (.mk hrf)
+
+end Nat.RecursiveIn.Code
+end
+
+namespace Nat.RecursiveIn.Code
+section
+
+open ComputableIn
+
+/-- Recursion on `Nat.RecursiveIn.Code` is computable. -/
+theorem rec_computable {α σ} [Primcodable α] [Primcodable σ] {c : α → Code} (hc : ComputableIn O c)
+    {z : α → σ} (hz : ComputableIn O z) {s : α → σ} (hs : ComputableIn O s) {l : α → σ} (hl : ComputableIn O l)
+    {r : α → σ} (hr : ComputableIn O r) {o : α → σ} (ho : ComputableIn O o) {pr : α → Code × Code × σ × σ → σ} (hpr : ComputableIn₂ O pr)
+    {co : α → Code × Code × σ × σ → σ} (hco : ComputableIn₂ O co) {pc : α → Code × Code × σ × σ → σ}
+    (hpc : ComputableIn₂ O pc) {rf : α → Code × σ → σ} (hrf : ComputableIn₂ O rf) :
+    let PR (a) cf cg hf hg := pr a (cf, cg, hf, hg)
+    let CO (a) cf cg hf hg := co a (cf, cg, hf, hg)
+    let PC (a) cf cg hf hg := pc a (cf, cg, hf, hg)
+    let RF (a) cf hf := rf a (cf, hf)
+    let F (a : α) (c : Code) : σ :=
+      Nat.RecursiveIn.Code.recOn c (z a) (s a) (l a) (r a) (o a) (PR a) (CO a) (PC a) (RF a)
+    ComputableIn O fun a => F a (c a) := by
+  -- TODO(Mario): less copy-paste from previous proof
+  intros _ _ _ _ F
+  let G₁ : (α × List σ) × ℕ × ℕ → Option σ := fun p =>
+    letI a := p.1.1; letI IH := p.1.2; letI n := p.2.1; letI m := p.2.2
+    (IH[m]?).bind fun s =>
+    (IH[m.unpair.1]?).bind fun s₁ =>
+    (IH[m.unpair.2]?).map fun s₂ =>
+    cond n.bodd
+      (cond n.div2.bodd (rf a (ofNat Code m, s))
+        (co a (ofNat Code m.unpair.1, ofNat Code m.unpair.2, s₁, s₂)))
+      (cond n.div2.bodd (pc a (ofNat Code m.unpair.1, ofNat Code m.unpair.2, s₁, s₂))
+        (pr a (ofNat Code m.unpair.1, ofNat Code m.unpair.2, s₁, s₂)))
+  have : ComputableIn O G₁ := by
+    refine option_bind (list_getElem?.comp (snd.comp fst) (snd.comp snd)) <| .mk ?_
+    refine option_bind ((list_getElem?.comp (snd.comp fst)
+      (fst.comp <| ComputableIn.unpair.comp (snd.comp snd))).comp fst) <| .mk ?_
+    refine option_map ((list_getElem?.comp (snd.comp fst)
+      (snd.comp <| ComputableIn.unpair.comp (snd.comp snd))).comp <| fst.comp fst) <| .mk ?_
+    exact
+      have a := fst.comp (fst.comp <| fst.comp <| fst.comp fst)
+      have n := fst.comp (snd.comp <| fst.comp <| fst.comp fst)
+      have m := snd.comp (snd.comp <| fst.comp <| fst.comp fst)
+      have m₁ := fst.comp (ComputableIn.unpair.comp m)
+      have m₂ := snd.comp (ComputableIn.unpair.comp m)
+      have s := snd.comp (fst.comp fst)
+      have s₁ := snd.comp fst
+      have s₂ := snd
+      (nat_bodd.comp n).cond
+        ((nat_bodd.comp <| nat_div2.comp n).cond
+          (hrf.comp a (((ComputableIn.ofNat Code).comp m).pair s))
+          (hco.comp a (((ComputableIn.ofNat Code).comp m₁).pair <|
+            ((ComputableIn.ofNat Code).comp m₂).pair <| s₁.pair s₂)))
+        (ComputableIn.cond (nat_bodd.comp <| nat_div2.comp n)
+          (hpc.comp a (((ComputableIn.ofNat Code).comp m₁).pair <|
+            ((ComputableIn.ofNat Code).comp m₂).pair <| s₁.pair s₂))
+          (hpr.comp a (((ComputableIn.ofNat Code).comp m₁).pair <|
+            ((ComputableIn.ofNat Code).comp m₂).pair <| s₁.pair s₂)))
+  let G : α → List σ → Option σ := fun a IH =>
+    IH.length.casesOn (some (z a)) fun n =>
+    n.casesOn (some (s a)) fun n =>
+    n.casesOn (some (l a)) fun n =>
+    n.casesOn (some (r a)) fun n =>
+    n.casesOn (some (o a)) fun n =>
+    G₁ ((a, IH), n, n.div2.div2)
+  have : ComputableIn₂ O G := .mk <|
+    nat_casesOn (list_length.comp snd) (option_some_iff.2 (hz.comp fst)) <| .mk <|
+    nat_casesOn snd (option_some_iff.2 (hs.comp (fst.comp fst))) <| .mk <|
+    nat_casesOn snd (option_some_iff.2 (hl.comp (fst.comp <| fst.comp fst))) <| .mk <|
+    nat_casesOn snd (option_some_iff.2 (hr.comp (fst.comp <| fst.comp <| fst.comp fst))) <| .mk <|
+    nat_casesOn snd (option_some_iff.2 (ho.comp (fst.comp <| fst.comp <| fst.comp <| fst.comp fst))) <| .mk <|
+    this.comp <|
+      -- ((fst.pair snd).comp <| fst.comp <| fst.comp <| fst.comp <| fst).pair <|
+      ((fst.pair snd).comp <| fst.comp <| fst.comp <| fst.comp <| fst.comp <| fst).pair <|
+      snd.pair <| nat_div2.comp <| nat_div2.comp snd
+  refine (nat_strong_rec (fun a n => F a (ofNat Code n)) this.to₂ fun a n => ?_)
+    |>.comp .id (encode_iff.2 hc) |>.of_eq fun a => by simp
+  iterate 5 rcases n with - | n; · simp [ofNatCode_eq, ofNatCode, decodeCode]; rfl
+  simp only [G]; rw [List.length_map, List.length_range]
+  let m := n.div2.div2
+  show G₁ ((a, (List.range (n + 5)).map fun n => F a (ofNat Code n)), n, m)
+    = some (F a (ofNat Code (n + 5)))
+  have hm : m < n + 5 := by
+    simp only [m, div2_val]
+    exact lt_of_le_of_lt
+      (le_trans (Nat.div_le_self ..) (Nat.div_le_self ..))
+      (Nat.succ_le_succ (Nat.le_add_right ..))
+  have m1 : m.unpair.1 < n + 5 := lt_of_le_of_lt m.unpair_left_le hm
+  have m2 : m.unpair.2 < n + 5 := lt_of_le_of_lt m.unpair_right_le hm
+  simp [G₁, m, List.getElem?_map, List.getElem?_range, hm, m1, m2]
+  rw [show ofNat Code (n + 5) = ofNatCode (n + 5) from rfl]
+  unfold decodeCode
+  simp
+  cases n.bodd <;> cases n.div2.bodd <;> rfl
+
+end
+
+/-- The interpretation of a `Nat.RecursiveIn.Code` as a partial function.
+* `Nat.RecursiveIn.Code.zero`: The constant zero function.
+* `Nat.RecursiveIn.Code.succ`: The successor function.
+* `Nat.RecursiveIn.Code.left`: Left unpairing of a pair of ℕ (encoded by `Nat.pair`)
+* `Nat.RecursiveIn.Code.right`: Right unpairing of a pair of ℕ (encoded by `Nat.pair`)
+* `Nat.RecursiveIn.Code.pair`: Pairs the outputs of argument codes using `Nat.pair`.
+* `Nat.RecursiveIn.Code.comp`: Composition of two argument codes.
+* `Nat.RecursiveIn.Code.prec`: Primitive recursion. Given an argument of the form `Nat.pair a n`:
+  * If `n = 0`, returns `eval O cf a`.
+  * If `n = succ k`, returns `eval O cg (pair a (pair k (eval O (prec cf cg) (pair a k))))`
+* `Nat.RecursiveIn.Code.rfind'`: Minimization. For `f` an argument of the form `Nat.pair a m`,
+  `rfind' f m` returns the least `a` such that `f a m = 0`, if one exists and `f b m` terminates
+  for `b < a`
+-/
+def eval (O : ℕ → ℕ) : Code → ℕ →. ℕ
+| zero => pure 0
+| succ => fun n => some (n + 1)
+| left => fun n => some (Nat.unpair n).1
+| right => fun n => some (Nat.unpair n).2
+| oracle => O
+| pair cf cg =>
+    fun n => Nat.pair <$> eval O cf n <*> eval O cg n
+| comp cf cg =>
+    fun n => eval O cg n >>= eval O cf
+| prec cf cg =>
+    Nat.unpaired fun a n =>
+      n.rec (eval O cf a) fun y IH => do
+        let i ← IH
+        eval O cg (Nat.pair a (Nat.pair y i))
+| rfind' cf =>
+    Nat.unpaired fun a m =>
+      (Nat.rfind fun n => (fun x => x = 0) <$> eval O cf (Nat.pair a (n + m))).map (· + m)
+
+/-- Helper lemma for the evaluation of `prec` in the base case. -/
+@[simp]
+theorem eval_prec_zero (cf cg : Code) (a : ℕ) : eval O (prec cf cg) (Nat.pair a 0) = eval O cf a := by
+  rw [eval, Nat.unpaired, Nat.unpair_pair]
+  simp (config := { Lean.Meta.Simp.neutralConfig with proj := true }) only []
+  rw [Nat.rec_zero]
+
+/-- Helper lemma for the evaluation of `prec` in the recursive case. -/
+theorem eval_prec_succ (cf cg : Code) (a k : ℕ) :
+    eval O (prec cf cg) (Nat.pair a (Nat.succ k)) =
+      do {let ih ← eval O (prec cf cg) (Nat.pair a k); eval O cg (Nat.pair a (Nat.pair k ih))} := by
+  rw [eval, Nat.unpaired, Part.bind_eq_bind, Nat.unpair_pair]
+  simp
+
+-- instance : Membership (ℕ →. ℕ) Code :=
+--   ⟨fun c f => eval O c = f⟩
+
+@[simp]
+theorem eval_const : ∀ n m, eval O (Code.const n) m = Part.some n
+  | 0, _ => rfl
+  | n + 1, m => by simp! [eval_const n m]
+
+@[simp]
+theorem eval_id (n) : eval O Code.id n = Part.some n := by simp! [Seq.seq, Code.id]
+
+@[simp]
+theorem eval_curry (c n x) : eval O (curry c n) x = eval O c (Nat.pair n x) := by simp! [Seq.seq, curry]
+
+theorem const_prim : PrimrecIn O Code.const :=
+  (_root_.PrimrecIn.id.nat_iterate (_root_.PrimrecIn.const zero)
+    (comp_prim.comp (_root_.PrimrecIn.const succ) PrimrecIn.snd).to₂).of_eq
+    fun n => by simp; induction n <;>
+      simp [*, Code.const, Function.iterate_succ', -Function.iterate_succ]
+
+theorem curry_prim : PrimrecIn₂ O curry :=
+  comp_prim.comp PrimrecIn.fst <| pair_prim.comp (const_prim.comp PrimrecIn.snd)
+    (_root_.PrimrecIn.const Code.id)
+
+theorem curry_inj {c₁ c₂ n₁ n₂} (h : curry c₁ n₁ = curry c₂ n₂) : c₁ = c₂ ∧ n₁ = n₂ :=
+  ⟨by injection h, by
+    injection h with h₁ h₂
+    injection h₂ with h₃ h₄
+    exact const_inj h₃⟩
+
+/--
+The $S_n^m$ theorem: There is a computable function, namely `Nat.RecursiveIn.Code.curry`, that takes a
+program and a ℕ `n`, and returns a new program using `n` as the first argument.
+-/
+theorem smn :
+    ∃ f : Code → ℕ → Code, ComputableIn₂ O f ∧ ∀ c n x, eval O (f c n) x = eval O c (Nat.pair n x) :=
+  ⟨curry, PrimrecIn₂.to_compIn curry_prim, eval_curry⟩
+
+/-- A function is partial recursive if and only if there is a code implementing it. Therefore,
+`eval` is a **universal partial recursive function**. -/
+theorem exists_code {f : ℕ →. ℕ} : Nat.RecursiveIn O f ↔ ∃ c : Code, eval O c = f := by
+  refine ⟨fun h => ?_, ?_⟩
+  · induction h with
+    | zero => exact ⟨zero, rfl⟩
+    | succ => exact ⟨succ, rfl⟩
+    | left => exact ⟨left, rfl⟩
+    | right => exact ⟨right, rfl⟩
+    | oracle => exact ⟨oracle, rfl⟩
+    | pair pf pg hf hg =>
+      rcases hf with ⟨cf, rfl⟩; rcases hg with ⟨cg, rfl⟩
+      exact ⟨pair cf cg, rfl⟩
+    | comp pf pg hf hg =>
+      rcases hf with ⟨cf, rfl⟩; rcases hg with ⟨cg, rfl⟩
+      exact ⟨comp cf cg, rfl⟩
+    | prec pf pg hf hg =>
+      rcases hf with ⟨cf, rfl⟩; rcases hg with ⟨cg, rfl⟩
+      exact ⟨prec cf cg, rfl⟩
+    | rfind pf hf =>
+      rcases hf with ⟨cf, rfl⟩
+      refine ⟨comp (rfind' cf) (pair Code.id zero), ?_⟩
+      simp [eval, Seq.seq, pure, PFun.pure, Part.map_id']
+  · rintro ⟨c, rfl⟩
+    induction c with
+    | zero => exact Nat.RecursiveIn.zero
+    | succ => exact Nat.RecursiveIn.succ
+    | left => exact Nat.RecursiveIn.left
+    | right => exact Nat.RecursiveIn.right
+    | oracle => exact Nat.RecursiveIn.oracle
+    | pair cf cg pf pg => exact pf.pair pg
+    | comp cf cg pf pg => exact pf.comp pg
+    | prec cf cg pf pg => exact pf.prec pg
+    | rfind' cf pf => exact pf.rfind'
+
+/- A modified evaluation for the code which returns an `Option ℕ` instead of a `Part ℕ`. To avoid
+undecidability, `evaln` takes a parameter `k` and fails if it encounters a number ≥ k in the course
+of its execution. Other than this, the semantics are the same as in `Nat.RecursiveIn.Code.eval`.
+-/
+open Classical in
+noncomputable
+def evaln (O:ℕ→ℕ) : ℕ → Code → ℕ → Option ℕ
+  | 0, _ => fun _ => Option.none
+  | k + 1, zero => fun n => do
+    guard (n ≤ k)
+    return 0
+  | k + 1, succ => fun n => do
+    guard (n ≤ k)
+    return (Nat.succ n)
+  | k + 1, left => fun n => do
+    guard (n ≤ k)
+    return n.unpair.1
+  | k + 1, right => fun n => do
+    guard (n ≤ k)
+    pure n.unpair.2
+  | k + 1, oracle => fun n => do
+    guard (n ≤ k)
+    -- (O n).toOption
+    -- umm. this is a contradiction. um.
+    pure (O n)
+  | k + 1, pair cf cg => fun n => do
+    guard (n ≤ k)
+    Nat.pair <$> evaln O (k + 1) cf n <*> evaln O (k + 1) cg n
+  | k + 1, comp cf cg => fun n => do
+    guard (n ≤ k)
+    let x ← evaln O (k + 1) cg n
+    evaln O (k + 1) cf x
+  | k + 1, prec cf cg => fun n => do
+    guard (n ≤ k)
+    n.unpaired fun a n =>
+      n.casesOn (evaln O (k + 1) cf a) fun y => do
+        let i ← evaln O k (prec cf cg) (Nat.pair a y)
+        evaln O (k + 1) cg (Nat.pair a (Nat.pair y i))
+  | k + 1, rfind' cf => fun n => do
+    guard (n ≤ k)
+    n.unpaired fun a m => do
+      let x ← evaln O (k + 1) cf (Nat.pair a m)
+      if x = 0 then
+        pure m
+      else
+        evaln O k (rfind' cf) (Nat.pair a (m + 1))
+
+theorem evaln_bound : ∀ {k c n x}, x ∈ evaln O k c n → n < k
+  | 0, c, n, x, h => by simp [evaln] at h
+  | k + 1, c, n, x, h => by
+    suffices ∀ {o : Option ℕ}, x ∈ do { guard (n ≤ k); o } → n < k + 1 by
+      cases c <;> rw [evaln] at h <;> exact this h
+    simpa [Option.bind_eq_some] using Nat.lt_succ_of_le
+
+theorem evaln_mono : ∀ {k₁ k₂ c n x}, k₁ ≤ k₂ → x ∈ evaln O k₁ c n → x ∈ evaln O k₂ c n
+  | 0, k₂, c, n, x, _, h => by simp [evaln] at h
+  | k + 1, k₂ + 1, c, n, x, hl, h => by
+    have hl' := Nat.le_of_succ_le_succ hl
+    have :
+      ∀ {k k₂ n x : ℕ} {o₁ o₂ : Option ℕ},
+        k ≤ k₂ → (x ∈ o₁ → x ∈ o₂) →
+          x ∈ do { guard (n ≤ k); o₁ } → x ∈ do { guard (n ≤ k₂); o₂ } := by
+      simp only [Option.mem_def, bind, Option.bind_eq_some, Option.guard_eq_some', exists_and_left,
+        exists_const, and_imp]
+      introv h h₁ h₂ h₃
+      exact ⟨le_trans h₂ h, h₁ h₃⟩
+    simp? at h ⊢ says simp only [Option.mem_def] at h ⊢
+    induction' c with cf cg hf hg cf cg hf hg cf cg hf hg cf hf generalizing x n <;>
+      rw [evaln] at h ⊢ <;> refine this hl' (fun h => ?_) h
+    iterate 5 exact h
+    · -- pair cf cg
+      simp? [Seq.seq, Option.bind_eq_some] at h ⊢ says
+        simp only [Seq.seq, Option.map_eq_map, Option.mem_def, Option.bind_eq_some,
+          Option.map_eq_some', exists_exists_and_eq_and] at h ⊢
+      exact h.imp fun a => And.imp (hf _ _) <| Exists.imp fun b => And.imp_left (hg _ _)
+    · -- comp cf cg
+      simp? [Bind.bind, Option.bind_eq_some] at h ⊢ says
+        simp only [bind, Option.mem_def, Option.bind_eq_some] at h ⊢
+      exact h.imp fun a => And.imp (hg _ _) (hf _ _)
+    · -- prec cf cg
+      revert h
+      simp only [unpaired, bind, Option.mem_def]
+      induction n.unpair.2 <;> simp [Option.bind_eq_some]
+      · apply hf
+      · exact fun y h₁ h₂ => ⟨y, evaln_mono hl' h₁, hg _ _ h₂⟩
+    · -- rfind' cf
+      simp? [Bind.bind, Option.bind_eq_some] at h ⊢ says
+        simp only [unpaired, bind, pair_unpair, Option.pure_def, Option.mem_def,
+          Option.bind_eq_some] at h ⊢
+      refine h.imp fun x => And.imp (hf _ _) ?_
+      by_cases x0 : x = 0 <;> simp [x0]
+      exact evaln_mono hl'
+
+theorem evaln_sound : ∀ {k c n x}, x ∈ evaln O k c n → x ∈ eval O c n
+  | 0, _, n, x, h => by simp [evaln] at h
+  | k + 1, c, n, x, h => by
+    induction' c with cf cg hf hg cf cg hf hg cf cg hf hg cf hf generalizing x n <;>
+        simp [eval, evaln, Option.bind_eq_some, Seq.seq] at h ⊢ <;>
+      obtain ⟨_, h⟩ := h
+    iterate 5 simpa [pure, PFun.pure, eq_comm] using h
+    · -- pair cf cg
+      rcases h with ⟨y, ef, z, eg, rfl⟩
+      exact ⟨_, hf _ _ ef, _, hg _ _ eg, rfl⟩
+    · --comp hf hg
+      rcases h with ⟨y, eg, ef⟩
+      exact ⟨_, hg _ _ eg, hf _ _ ef⟩
+    · -- prec cf cg
+      revert h
+      induction' n.unpair.2 with m IH generalizing x <;> simp [Option.bind_eq_some]
+      · apply hf
+      · refine fun y h₁ h₂ => ⟨y, IH _ ?_, ?_⟩
+        · have := evaln_mono k.le_succ h₁
+          simp [evaln, Option.bind_eq_some] at this
+          exact this.2
+        · exact hg _ _ h₂
+    · -- rfind' cf
+      rcases h with ⟨m, h₁, h₂⟩
+      by_cases m0 : m = 0 <;> simp [m0] at h₂
+      · exact
+          ⟨0, ⟨by simpa [m0] using hf _ _ h₁, fun {m} => (Nat.not_lt_zero _).elim⟩, by simp [h₂]⟩
+      · have := evaln_sound h₂
+        simp [eval] at this
+        rcases this with ⟨y, ⟨hy₁, hy₂⟩, rfl⟩
+        refine
+          ⟨y + 1, ⟨by simpa [add_comm, add_left_comm] using hy₁, fun {i} im => ?_⟩, by
+            simp [add_comm, add_left_comm]⟩
+        rcases i with - | i
+        · exact ⟨m, by simpa using hf _ _ h₁, m0⟩
+        · rcases hy₂ (Nat.lt_of_succ_lt_succ im) with ⟨z, hz, z0⟩
+          exact ⟨z, by simpa [add_comm, add_left_comm] using hz, z0⟩
+
+theorem evaln_complete {c n x} : x ∈ eval O c n ↔ ∃ k, x ∈ evaln O k c n := by
+  refine ⟨fun h => ?_, fun ⟨k, h⟩ => evaln_sound h⟩
+  rsuffices ⟨k, h⟩ : ∃ k, x ∈ evaln O (k + 1) c n
+  · exact ⟨k + 1, h⟩
+  induction c generalizing n x with
+      simp [eval, evaln, pure, PFun.pure, Seq.seq, Option.bind_eq_some] at h ⊢
+  | pair cf cg hf hg =>
+    rcases h with ⟨x, hx, y, hy, rfl⟩
+    rcases hf hx with ⟨k₁, hk₁⟩; rcases hg hy with ⟨k₂, hk₂⟩
+    refine ⟨max k₁ k₂, ?_⟩
+    refine
+      ⟨le_max_of_le_left <| Nat.le_of_lt_succ <| evaln_bound hk₁, _,
+        evaln_mono (Nat.succ_le_succ <| le_max_left _ _) hk₁, _,
+        evaln_mono (Nat.succ_le_succ <| le_max_right _ _) hk₂, rfl⟩
+  | comp cf cg hf hg =>
+    rcases h with ⟨y, hy, hx⟩
+    rcases hg hy with ⟨k₁, hk₁⟩; rcases hf hx with ⟨k₂, hk₂⟩
+    refine ⟨max k₁ k₂, ?_⟩
+    exact
+      ⟨le_max_of_le_left <| Nat.le_of_lt_succ <| evaln_bound hk₁, _,
+        evaln_mono (Nat.succ_le_succ <| le_max_left _ _) hk₁,
+        evaln_mono (Nat.succ_le_succ <| le_max_right _ _) hk₂⟩
+  | prec cf cg hf hg =>
+    revert h
+    generalize n.unpair.1 = n₁; generalize n.unpair.2 = n₂
+    induction' n₂ with m IH generalizing x n <;> simp [Option.bind_eq_some]
+    · intro h
+      rcases hf h with ⟨k, hk⟩
+      exact ⟨_, le_max_left _ _, evaln_mono (Nat.succ_le_succ <| le_max_right _ _) hk⟩
+    · intro y hy hx
+      rcases IH hy with ⟨k₁, nk₁, hk₁⟩
+      rcases hg hx with ⟨k₂, hk₂⟩
+      refine
+        ⟨(max k₁ k₂).succ,
+          Nat.le_succ_of_le <| le_max_of_le_left <|
+            le_trans (le_max_left _ (Nat.pair n₁ m)) nk₁, y,
+          evaln_mono (Nat.succ_le_succ <| le_max_left _ _) ?_,
+          evaln_mono (Nat.succ_le_succ <| Nat.le_succ_of_le <| le_max_right _ _) hk₂⟩
+      simp only [evaln, bind, unpaired, unpair_pair, Option.mem_def, Option.bind_eq_some,
+        Option.guard_eq_some', exists_and_left, exists_const]
+      exact ⟨le_trans (le_max_right _ _) nk₁, hk₁⟩
+
+  | rfind' cf hf =>
+    rcases h with ⟨y, ⟨hy₁, hy₂⟩, rfl⟩
+    suffices ∃ k, y + n.unpair.2 ∈ evaln O (k + 1) (rfind' cf) (Nat.pair n.unpair.1 n.unpair.2) by
+      simpa [evaln, Option.bind_eq_some]
+    revert hy₁ hy₂
+    generalize n.unpair.2 = m
+    intro hy₁ hy₂
+    induction' y with y IH generalizing m <;> simp [evaln, Option.bind_eq_some]
+    · simp at hy₁
+      rcases hf hy₁ with ⟨k, hk⟩
+      exact ⟨_, Nat.le_of_lt_succ <| evaln_bound hk, _, hk, by simp⟩
+    · rcases hy₂ (Nat.succ_pos _) with ⟨a, ha, a0⟩
+      rcases hf ha with ⟨k₁, hk₁⟩
+      rcases IH m.succ (by simpa [Nat.succ_eq_add_one, add_comm, add_left_comm] using hy₁)
+          fun {i} hi => by
+          simpa [Nat.succ_eq_add_one, add_comm, add_left_comm] using
+            hy₂ (Nat.succ_lt_succ hi) with
+        ⟨k₂, hk₂⟩
+      use (max k₁ k₂).succ
+      rw [zero_add] at hk₁
+      use Nat.le_succ_of_le <| le_max_of_le_left <| Nat.le_of_lt_succ <| evaln_bound hk₁
+      use a
+      use evaln_mono (Nat.succ_le_succ <| Nat.le_succ_of_le <| le_max_left _ _) hk₁
+      simpa [a0, add_comm, add_left_comm] using
+        evaln_mono (Nat.succ_le_succ <| le_max_right _ _) hk₂
+  | _ => exact ⟨⟨_, le_rfl⟩, h.symm⟩
+
+section
+
+open PrimrecIn
+
+private def lup (L : List (List (Option ℕ))) (p : ℕ × Code) (n : ℕ) := do
+  let l ← L[(encode p)]?
+  let o ← l[n]?
+  o
+
+private theorem hlup : PrimrecIn O fun p : _ × (_ × _) × _ => lup p.1 p.2.1 p.2.2 :=
+  PrimrecIn.option_bind
+    (PrimrecIn.list_getElem?.comp PrimrecIn.fst (PrimrecIn.encode.comp <| PrimrecIn.fst.comp PrimrecIn.snd))
+    (PrimrecIn.option_bind (PrimrecIn.list_getElem?.comp PrimrecIn.snd <| PrimrecIn.snd.comp <|
+      PrimrecIn.snd.comp PrimrecIn.fst) PrimrecIn.snd)
+
+private def G (O:ℕ→ℕ) (L : List (List (Option ℕ))) : Option (List (Option ℕ)) :=
+  Option.some <|
+    let a := ofNat (ℕ × Code) L.length
+    let k := a.1
+    let c := a.2
+    (List.range k).map fun n =>
+      k.casesOn Option.none fun k' =>
+        Nat.RecursiveIn.Code.recOn c
+          (some 0) -- zero
+          (some (Nat.succ n))
+          (some n.unpair.1)
+          (some n.unpair.2)
+          (some (O n)) -- oracle
+          (fun cf cg _ _ => do
+            let x ← lup L (k, cf) n
+            let y ← lup L (k, cg) n
+            some (Nat.pair x y))
+          (fun cf cg _ _ => do
+            let x ← lup L (k, cg) n
+            lup L (k, cf) x)
+          (fun cf cg _ _ =>
+            let z := n.unpair.1
+            n.unpair.2.casesOn (lup L (k, cf) z) fun y => do
+              let i ← lup L (k', c) (Nat.pair z y)
+              lup L (k, cg) (Nat.pair z (Nat.pair y i)))
+          (fun cf _ =>
+            let z := n.unpair.1
+            let m := n.unpair.2
+            do
+              let x ← lup L (k, cf) (Nat.pair z m)
+              x.casesOn (some m) fun _ => lup L (k', c) (Nat.pair z (m + 1)))
+
+
+private theorem evaln_map (k c n) :
+    ((List.range k)[n]?.bind fun a ↦ evaln O k c a) = evaln O k c n := by
+  by_cases kn : n < k
+  · simp [List.getElem?_range kn]
+  · rw [List.getElem?_eq_none]
+    · cases e : evaln O k c n
+      · rfl
+      exact kn.elim (evaln_bound e)
+    simpa using kn
+
+
+
+private theorem hG {O} : PrimrecIn O (G O) := by
+  have a := (@PrimrecIn.ofNat O (ℕ × Code)).comp (PrimrecIn.list_length (α := List (Option ℕ)))
+  have k := PrimrecIn.fst.comp a
+  refine PrimrecIn.option_some.comp (PrimrecIn.list_map (PrimrecIn.list_range.comp k) (?_ : PrimrecIn O _))
+  replace k := k.comp (PrimrecIn.fst (β := ℕ))
+  have n := @PrimrecIn.snd O (α := List (List (Option ℕ))) (β := ℕ)
+  refine PrimrecIn.nat_casesOn k (_root_.PrimrecIn.const Option.none) (?_ : PrimrecIn O _)
+  have k := k.comp (PrimrecIn.fst (β := ℕ))
+  have n := n.comp (PrimrecIn.fst (β := ℕ))
+  have k' := @PrimrecIn.snd O (α := List (List (Option ℕ)) × ℕ) (β := ℕ)
+  have c := PrimrecIn.snd.comp (a.comp <| (PrimrecIn.fst (β := ℕ)).comp (PrimrecIn.fst (β := ℕ)))
+  apply
+    Nat.RecursiveIn.Code.rec_prim c
+      (_root_.PrimrecIn.const (some 0))
+      (PrimrecIn.option_some.comp (_root_.PrimrecIn.succ.comp n))
+      (PrimrecIn.option_some.comp (PrimrecIn.fst.comp <| PrimrecIn.unpair.comp n))
+      (PrimrecIn.option_some.comp (PrimrecIn.snd.comp <| PrimrecIn.unpair.comp n))
+      (PrimrecIn.option_some.comp (_root_.PrimrecIn.oracle.comp n))
+  · have L := ((@PrimrecIn.fst O).comp PrimrecIn.fst).comp
+      (PrimrecIn.fst (α := (List (List (Option ℕ)) × ℕ) × ℕ)
+        (β := Code × Code × Option ℕ × Option ℕ))
+    have k := k.comp (PrimrecIn.fst (β := Code × Code × Option ℕ × Option ℕ))
+    have n := n.comp (PrimrecIn.fst (β := Code × Code × Option ℕ × Option ℕ))
+    have cf := (@PrimrecIn.fst O).comp (PrimrecIn.snd (α := (List (List (Option ℕ)) × ℕ) × ℕ)
+        (β := Code × Code × Option ℕ × Option ℕ))
+    have cg := ((@PrimrecIn.fst O).comp PrimrecIn.snd).comp
+      (PrimrecIn.snd (α := (List (List (Option ℕ)) × ℕ) × ℕ)
+        (β := Code × Code × Option ℕ × Option ℕ))
+    refine PrimrecIn.option_bind (hlup.comp <| L.pair <| (k.pair cf).pair n) ?_
+    unfold PrimrecIn₂
+    sorry
+    -- conv =>
+    --   congr
+    --   · ext p
+    --     dsimp only []
+    --     erw [Option.bind_eq_bind, ← Option.map_eq_bind]
+    -- refine PrimrecIn.option_map ((hlup.comp <| L.pair <| (k.pair cg).pair n).comp PrimrecIn.fst) ?_
+    -- unfold PrimrecIn₂
+    -- exact PrimrecIn₂.natPair.comp (PrimrecIn.snd.comp PrimrecIn.fst) PrimrecIn.snd
+  · have L := ((@PrimrecIn.fst O).comp PrimrecIn.fst).comp
+      (PrimrecIn.fst (α := (List (List (Option ℕ)) × ℕ) × ℕ)
+        (β := Code × Code × Option ℕ × Option ℕ))
+    have k := k.comp (PrimrecIn.fst (β := Code × Code × Option ℕ × Option ℕ))
+    have n := n.comp (PrimrecIn.fst (β := Code × Code × Option ℕ × Option ℕ))
+    have cf := (@PrimrecIn.fst O).comp (PrimrecIn.snd (α := (List (List (Option ℕ)) × ℕ) × ℕ)
+        (β := Code × Code × Option ℕ × Option ℕ))
+    have cg := ((@PrimrecIn.fst O).comp PrimrecIn.snd).comp
+      (PrimrecIn.snd (α := (List (List (Option ℕ)) × ℕ) × ℕ)
+        (β := Code × Code × Option ℕ × Option ℕ))
+    refine PrimrecIn.option_bind (hlup.comp <| L.pair <| (k.pair cg).pair n) ?_
+    unfold PrimrecIn₂
+    have h :=
+      hlup.comp ((L.comp PrimrecIn.fst).pair <| ((k.pair cf).comp PrimrecIn.fst).pair PrimrecIn.snd)
+    exact h
+  · have L := ((@PrimrecIn.fst O).comp PrimrecIn.fst).comp
+      (PrimrecIn.fst (α := (List (List (Option ℕ)) × ℕ) × ℕ)
+        (β := Code × Code × Option ℕ × Option ℕ))
+    have k := k.comp (PrimrecIn.fst (β := Code × Code × Option ℕ × Option ℕ))
+    have n := n.comp (PrimrecIn.fst (β := Code × Code × Option ℕ × Option ℕ))
+    have cf := (@PrimrecIn.fst O).comp (PrimrecIn.snd (α := (List (List (Option ℕ)) × ℕ) × ℕ)
+        (β := Code × Code × Option ℕ × Option ℕ))
+    have cg := ((@PrimrecIn.fst O).comp PrimrecIn.snd).comp
+      (PrimrecIn.snd (α := (List (List (Option ℕ)) × ℕ) × ℕ)
+        (β := Code × Code × Option ℕ × Option ℕ))
+    have z := PrimrecIn.fst.comp (PrimrecIn.unpair.comp n)
+    refine
+      PrimrecIn.nat_casesOn (PrimrecIn.snd.comp (PrimrecIn.unpair.comp n))
+        (hlup.comp <| L.pair <| (k.pair cf).pair z)
+        (?_ : PrimrecIn O _)
+    have L := L.comp (PrimrecIn.fst (β := ℕ))
+    have z := z.comp (PrimrecIn.fst (β := ℕ))
+    have y := @PrimrecIn.snd O
+      (α := ((List (List (Option ℕ)) × ℕ) × ℕ) × Code × Code × Option ℕ × Option ℕ) (β := ℕ)
+    have h₁ := hlup.comp <| L.pair <| (((k'.pair c).comp PrimrecIn.fst).comp PrimrecIn.fst).pair
+      (PrimrecIn₂.natPair.comp z y)
+    refine PrimrecIn.option_bind h₁ (?_ : PrimrecIn O _)
+    have z := z.comp (PrimrecIn.fst (β := ℕ))
+    have y := y.comp (PrimrecIn.fst (β := ℕ))
+    have i := @PrimrecIn.snd O
+      (α := (((List (List (Option ℕ)) × ℕ) × ℕ) × Code × Code × Option ℕ × Option ℕ) × ℕ)
+      (β := ℕ)
+    have h₂ := hlup.comp ((L.comp PrimrecIn.fst).pair <|
+      ((k.pair cg).comp <| PrimrecIn.fst.comp PrimrecIn.fst).pair <|
+        PrimrecIn₂.natPair.comp z <| PrimrecIn₂.natPair.comp y i)
+    exact h₂
+  · have L := ((@PrimrecIn.fst O).comp PrimrecIn.fst).comp
+      (PrimrecIn.fst (α := (List (List (Option ℕ)) × ℕ) × ℕ)
+        (β := Code × Option ℕ))
+    have k := k.comp (PrimrecIn.fst (β := Code × Option ℕ))
+    have n := n.comp (PrimrecIn.fst (β := Code × Option ℕ))
+    have cf := (@PrimrecIn.fst O).comp (PrimrecIn.snd (α := (List (List (Option ℕ)) × ℕ) × ℕ)
+        (β := Code × Option ℕ))
+    have z := PrimrecIn.fst.comp (PrimrecIn.unpair.comp n)
+    have m := PrimrecIn.snd.comp (PrimrecIn.unpair.comp n)
+    have h₁ := hlup.comp <| L.pair <| (k.pair cf).pair (PrimrecIn₂.natPair.comp z m)
+    refine PrimrecIn.option_bind h₁ (?_ : PrimrecIn O _)
+    have m := m.comp (PrimrecIn.fst (β := ℕ))
+    refine PrimrecIn.nat_casesOn PrimrecIn.snd (PrimrecIn.option_some.comp m) ?_
+    unfold PrimrecIn₂
+    exact (hlup.comp ((L.comp PrimrecIn.fst).pair <|
+      ((k'.pair c).comp <| PrimrecIn.fst.comp PrimrecIn.fst).pair
+        (PrimrecIn₂.natPair.comp (z.comp PrimrecIn.fst) (_root_.PrimrecIn.succ.comp m)))).comp
+      PrimrecIn.fst
+
+
+
+
+
+/-- The `Nat.RecursiveIn.Code.evaln` function is primitive recursive. -/
+
+
+theorem evaln_prim : PrimrecIn O fun a : (ℕ × Code) × ℕ => evaln O a.1.1 a.1.2 a.2 :=
+  have :
+    PrimrecIn₂ O fun (_ : Unit) (n : ℕ) =>
+      let a := ofNat (ℕ × Code) n
+      (List.range a.1).map (evaln O a.1 a.2) :=
+    PrimrecIn.nat_strong_rec _ (hG.comp PrimrecIn.snd).to₂ fun _ p => by
+      simp only [G, prod_ofNat_val, ofNat_nat, List.length_map, List.length_range,
+        Nat.pair_unpair, Option.some_inj]
+      refine List.map_congr_left fun n => ?_
+      have : List.range p = List.range (Nat.pair p.unpair.1 (encode (ofNat Code p.unpair.2))) := by
+        simp
+      rw [this]
+      generalize p.unpair.1 = k
+      generalize ofNat Code p.unpair.2 = c
+      intro nk
+      rcases k with - | k'
+      · simp [evaln]
+      let k := k' + 1
+      simp only [show k'.succ = k from rfl]
+      simp? [Nat.lt_succ_iff] at nk says simp only [List.mem_range, Nat.lt_succ_iff] at nk
+      have hg :
+        ∀ {k' c' n},
+          Nat.pair k' (encode c') < Nat.pair k (encode c) →
+            lup ((List.range (Nat.pair k (encode c))).map fun n =>
+              (List.range n.unpair.1).map (evaln O n.unpair.1 (ofNat Code n.unpair.2))) (k', c') n =
+            evaln O k' c' n := by
+        intro k₁ c₁ n₁ hl
+        simp [lup, List.getElem?_range hl, evaln_map, Bind.bind, Option.bind_map]
+      obtain - | - | - | - | - | ⟨cf, cg⟩ | ⟨cf, cg⟩ | ⟨cf, cg⟩ | cf := c <;>
+        simp [evaln, nk, Bind.bind, Functor.map, Seq.seq, pure]
+      · obtain ⟨lf, lg⟩ := encode_lt_pair cf cg
+        rw [hg (Nat.pair_lt_pair_right _ lf), hg (Nat.pair_lt_pair_right _ lg)]
+        cases evaln O k cf n
+        · rfl
+        cases evaln O k cg n <;> rfl
+      · obtain ⟨lf, lg⟩ := encode_lt_comp cf cg
+        rw [hg (Nat.pair_lt_pair_right _ lg)]
+        cases evaln O k cg n
+        · rfl
+        simp [k, hg (Nat.pair_lt_pair_right _ lf)]
+      · obtain ⟨lf, lg⟩ := encode_lt_prec cf cg
+        rw [hg (Nat.pair_lt_pair_right _ lf)]
+        cases n.unpair.2
+        · rfl
+        simp only [decode_eq_ofNat, Option.some.injEq]
+        rw [hg (Nat.pair_lt_pair_left _ k'.lt_succ_self)]
+        cases evaln O k' _ _
+        · rfl
+        simp [k, hg (Nat.pair_lt_pair_right _ lg)]
+      · have lf := encode_lt_rfind' cf
+        rw [hg (Nat.pair_lt_pair_right _ lf)]
+        rcases evaln O k cf n with - | x
+        · rfl
+        simp only [decode_eq_ofNat, Option.some.injEq, Option.some_bind]
+        cases x <;> simp [Nat.succ_ne_zero]
+        rw [hg (Nat.pair_lt_pair_left _ k'.lt_succ_self)]
+
+
+
+
+
+  (PrimrecIn.option_bind
+    (PrimrecIn.list_getElem?.comp (this.comp (_root_.PrimrecIn.const ())
+      (PrimrecIn.encode_iff.2 PrimrecIn.fst)) PrimrecIn.snd) PrimrecIn.snd.to₂).of_eq
+    fun ⟨⟨k, c⟩, n⟩ => by simp [evaln_map, Option.bind_map]
+
+end
+
+section
+
+open RecursiveIn ComputableIn
+
+theorem eval_eq_rfindOpt (c n) : eval O c n = Nat.rfindOpt fun k => evaln O k c n :=
+  Part.ext fun x => by
+    refine evaln_complete.trans (Nat.rfindOpt_mono ?_).symm
+    intro a m n hl; apply evaln_mono hl
+
+theorem eval_part : RecursiveIn O₂ (eval O) :=
+  (RecursiveIn.rfindOpt
+    (evaln_prim.to_compIn.comp ((ComputableIn.snd.pair (fst.comp fst)).pair (snd.comp fst))).to₂).of_eq
+    fun a => by simp [eval_eq_rfindOpt]
+
+/-- **Roger's fixed-point theorem**: any total, computable `f` has a fixed point.
+That is, under the interpretation given by `Nat.RecursiveIn.Code.eval`, there is a code `c`
+such that `c` and `f c` have the same evaluation.
+-/
+theorem fixed_point {f : Code → Code} (hf : ComputableIn O f) : ∃ c : Code, eval O (f c) = eval O c :=
+  let g (x y : ℕ) : Part ℕ := eval O (ofNat Code x) x >>= fun b => eval O (ofNat Code b) y
+  have : RecursiveIn O₂ g :=
+    (eval_part.comp ((ComputableIn.ofNat _).comp fst) fst).bind
+      (eval_part.comp ((ComputableIn.ofNat _).comp snd) (snd.comp fst)).to₂
+  let ⟨cg, eg⟩ := exists_code.1 this
+  have eg' : ∀ a n, eval O cg (Nat.pair a n) = Part.map encode (g a n) := by simp [eg]
+  let F (x : ℕ) : Code := f (curry cg x)
+  have : ComputableIn O F :=
+    hf.comp (curry_prim.comp (_root_.PrimrecIn.const cg) _root_.PrimrecIn.id).to_compIn
+  let ⟨cF, eF⟩ := exists_code.1 this
+  have eF' : eval O cF (encode cF) = Part.some (encode (F (encode cF))) := by simp [eF]
+  ⟨curry cg (encode cF),
+    funext fun n =>
+      show eval O (f (curry cg (encode cF))) n = eval O (curry cg (encode cF)) n by
+        simp [F, g, eg', eF', Part.map_id']⟩
+
+/-- **Kleene's second recursion theorem** -/
+theorem fixed_point₂ {f : Code → ℕ →. ℕ} (hf : RecursiveIn O₂ f) : ∃ c : Code, eval O c = f c :=
+  let ⟨cf, ef⟩ := exists_code.1 hf
+  (fixed_point (curry_prim.comp (_root_.PrimrecIn.const cf) PrimrecIn.encode).to_compIn).imp fun c e =>
+    funext fun n => by simp [e.symm, ef, Part.map_id']
+
+end
+
+/-- There are only countably many partial recursive partial functions `ℕ →. ℕ`. -/
+instance : Countable {f : ℕ →. ℕ // _root_.RecursiveIn O f} := by
+  apply Function.Surjective.countable (f := fun c => ⟨eval O c, eval_part.comp (.const c) .id⟩)
+  intro ⟨f, hf⟩; simpa using exists_code.1 hf
+
+/-- There are only countably many computable functions `ℕ → ℕ`. -/
+instance : Countable {f : ℕ → ℕ // ComputableIn O f} :=
+  @Function.Injective.countable {f : ℕ → ℕ // ComputableIn O f} {f : ℕ →. ℕ // _root_.RecursiveIn O f} _
+    (fun f => ⟨f.val, f.2⟩)
+    (fun _ _ h => Subtype.val_inj.1 (PFun.lift_injective (by simpa using h)))
+
+end Nat.RecursiveIn.Code
