Computability/SingleOracle/PrimrecIn.lean
@@ -1,0 +1,1407 @@
+import Mathlib.Computability.Primrec
+
+
+open List (Vector)
+open Denumerable Encodable Function
+
+namespace Nat
+
+-- /-- Calls the given function on a pair of entries `n`, encoded via the pairing function. -/
+-- @[simp, reducible]
+-- def unpaired {α} (f : ℕ → ℕ → α) (n : ℕ) : α :=
+--   f n.unpair.1 n.unpair.2
+
+/-- The primitive recursive functions `ℕ → ℕ`. -/
+protected inductive PrimrecIn (O:ℕ→ℕ) : (ℕ → ℕ) → Prop
+  | zero : Nat.PrimrecIn O fun _ => 0
+  | protected succ : Nat.PrimrecIn O succ
+  | left : Nat.PrimrecIn O fun n => n.unpair.1
+  | right : Nat.PrimrecIn O fun n => n.unpair.2
+  | oracle : Nat.PrimrecIn O O
+  | pair {f g} : Nat.PrimrecIn O f → Nat.PrimrecIn O g → Nat.PrimrecIn O fun n => pair (f n) (g n)
+  | comp {f g} : Nat.PrimrecIn O f → Nat.PrimrecIn O g → Nat.PrimrecIn O fun n => f (g n)
+  | prec {f g} :
+      Nat.PrimrecIn O f →
+        Nat.PrimrecIn O g →
+          Nat.PrimrecIn O (unpaired fun z n => n.rec (f z) fun y IH => g <| pair z <| pair y IH)
+
+theorem Primrec.to_PrimrecIn (hf : Nat.Primrec f) : Nat.PrimrecIn O f := by
+  induction' hf
+  · exact PrimrecIn.zero
+  · exact PrimrecIn.succ
+  · exact PrimrecIn.left
+  · exact PrimrecIn.right
+  · (expose_names; exact PrimrecIn.pair a_ih a_ih_1)
+  · (expose_names; exact PrimrecIn.comp a_ih a_ih_1)
+  · (expose_names; exact PrimrecIn.prec a_ih a_ih_1)
+
+
+namespace PrimrecIn
+
+theorem of_eq {f g : ℕ → ℕ} (hf : Nat.PrimrecIn O f) (H : ∀ n, f n = g n) : Nat.PrimrecIn O g :=
+  (funext H : f = g) ▸ hf
+
+theorem const : ∀ n : ℕ, Nat.PrimrecIn O fun _ => n
+  | 0 => zero
+  | n + 1 => PrimrecIn.succ.comp (const n)
+
+protected theorem id : Nat.PrimrecIn O id :=
+  (left.pair right).of_eq fun n => by simp
+
+theorem prec1 {f} (m : ℕ) (hf : Nat.PrimrecIn O f) :
+    Nat.PrimrecIn O fun n => n.rec m fun y IH => f <| Nat.pair y IH :=
+  ((prec (const m) (hf.comp right)).comp (zero.pair PrimrecIn.id)).of_eq fun n => by simp
+
+theorem casesOn1 {f} (m : ℕ) (hf : Nat.PrimrecIn O f) : Nat.PrimrecIn O (Nat.casesOn · m f) :=
+  (prec1 m (hf.comp left)).of_eq <| by simp
+
+-- Porting note: `Nat.PrimrecIn.casesOn` is already declared as a recursor.
+theorem casesOn' {f g} (hf : Nat.PrimrecIn O f) (hg : Nat.PrimrecIn O g) :
+    Nat.PrimrecIn O (unpaired fun z n => n.casesOn (f z) fun y => g <| Nat.pair z y) :=
+  (prec hf (hg.comp (pair left (left.comp right)))).of_eq fun n => by simp
+
+protected theorem swap : Nat.PrimrecIn O (unpaired (swap Nat.pair)) :=
+  (pair right left).of_eq fun n => by simp
+
+theorem swap' {f} (hf : Nat.PrimrecIn O (unpaired f)) : Nat.PrimrecIn O (unpaired (swap f)) :=
+  (hf.comp .swap).of_eq fun n => by simp
+
+theorem pred : Nat.PrimrecIn O pred :=
+  (casesOn1 0 PrimrecIn.id).of_eq fun n => by cases n <;> simp [*]
+
+theorem add : Nat.PrimrecIn O (unpaired (· + ·)) :=
+  (prec .id ((PrimrecIn.succ.comp right).comp right)).of_eq fun p => by
+    simp; induction p.unpair.2 <;> simp [*, Nat.add_assoc]
+
+theorem sub : Nat.PrimrecIn O (unpaired (· - ·)) :=
+  (prec .id ((pred.comp right).comp right)).of_eq fun p => by
+    simp; induction p.unpair.2 <;> simp [*, Nat.sub_add_eq]
+
+theorem mul : Nat.PrimrecIn O (unpaired (· * ·)) :=
+  (prec zero (add.comp (pair left (right.comp right)))).of_eq fun p => by
+    simp; induction p.unpair.2 <;> simp [*, mul_succ, add_comm _ (unpair p).fst]
+
+theorem pow : Nat.PrimrecIn O (unpaired (· ^ ·)) :=
+  (prec (const 1) (mul.comp (pair (right.comp right) left))).of_eq fun p => by
+    simp; induction p.unpair.2 <;> simp [*, Nat.pow_succ]
+
+end PrimrecIn
+
+end Nat
+
+-- /-- A `Primcodable` type is an `Encodable` type for which
+--   the encode/decode functions are primitive recursive. -/
+-- class Primcodable (α : Type*) extends Encodable α where
+--   -- Porting note: was `prim [] `.
+--   -- This means that `prim` does not take the type explicitly in Lean 4
+--   prim : Nat.PrimrecIn O fun n => Encodable.encode (decode n)
+
+-- namespace Primcodable
+
+-- open Nat.PrimrecIn O
+
+-- instance (priority := 10) ofDenumerable (α) [Denumerable α] : Primcodable α :=
+--   ⟨Nat.PrimrecIn.succ.of_eq <| by simp⟩
+
+-- /-- Builds a `Primcodable` instance from an equivalence to a `Primcodable` type. -/
+-- def ofEquiv (α) {β} [Primcodable α] (e : β ≃ α) : Primcodable β :=
+--   { __ := Encodable.ofEquiv α e
+--     prim := (@Primcodable.prim α _).of_eq fun n => by
+--       rw [decode_ofEquiv]
+--       cases (@decode α _ n) <;>
+--         simp [encode_ofEquiv] }
+
+-- instance empty : Primcodable Empty :=
+--   ⟨zero⟩
+
+-- instance unit : Primcodable PUnit :=
+--   ⟨(casesOn1 1 zero).of_eq fun n => by cases n <;> simp⟩
+
+-- instance option {α : Type*} [h : Primcodable α] : Primcodable (Option α) :=
+--   ⟨(casesOn1 1 ((casesOn1 0 (.comp .succ .succ)).comp (@Primcodable.prim α _))).of_eq fun n => by
+--     cases n with
+--       | zero => rfl
+--       | succ n =>
+--         rw [decode_option_succ]
+--         cases H : @decode α _ n <;> simp [H]⟩
+
+-- instance bool : Primcodable Bool :=
+--   ⟨(casesOn1 1 (casesOn1 2 zero)).of_eq fun n => match n with
+--     | 0 => rfl
+--     | 1 => rfl
+--     | (n + 2) => by rw [decode_ge_two] <;> simp⟩
+
+-- end Primcodable
+
+/-- `PrimrecIn O f` means `f` is primitive recursive (after
+  encoding its input and output as natural numbers). -/
+def PrimrecIn (O:ℕ→ℕ) {α β} [Primcodable α] [Primcodable β] (f : α → β) : Prop :=
+  Nat.PrimrecIn O fun n => encode ((@decode α _ n).map f)
+
+theorem Primrec.to_PrimrecIn {O} {α β} [Primcodable α] [Primcodable β] (f : α → β) (hf : Primrec f) : PrimrecIn O f := by exact Nat.Primrec.to_PrimrecIn hf
+
+
+namespace PrimrecIn
+
+variable {α : Type*} {β : Type*} {σ : Type*}
+variable [Primcodable α] [Primcodable β] [Primcodable σ]
+
+open Nat.PrimrecIn
+
+protected theorem encode : PrimrecIn O (@encode α _) := Nat.Primrec.to_PrimrecIn Primrec.encode
+protected theorem decode : PrimrecIn O (@decode α _) := Nat.Primrec.to_PrimrecIn Primrec.decode
+
+theorem dom_denumerable {α β} [Denumerable α] [Primcodable β] {f : α → β} :
+    PrimrecIn O f ↔ Nat.PrimrecIn O fun n => encode (f (ofNat α n)) :=
+  ⟨fun h => (pred.comp h).of_eq fun n => by simp, fun h =>
+    (Nat.PrimrecIn.succ.comp h).of_eq fun n => by simp⟩
+
+theorem nat_iff {f : ℕ → ℕ} : PrimrecIn O f ↔ Nat.PrimrecIn O f := dom_denumerable
+theorem encdec : PrimrecIn O fun n => encode (@decode α _ n) := Nat.Primrec.to_PrimrecIn Primrec.encdec
+theorem option_some : PrimrecIn O (@some α) := Nat.Primrec.to_PrimrecIn Primrec.option_some
+theorem of_eq {f g : α → σ} (hf : PrimrecIn O f) (H : ∀ n, f n = g n) : PrimrecIn O g := (funext H : f = g) ▸ hf
+theorem const (x : σ) : PrimrecIn O fun _ : α => x := Nat.Primrec.to_PrimrecIn (Primrec.const x)
+protected theorem id : PrimrecIn O (@id α) := Nat.Primrec.to_PrimrecIn Primrec.id
+
+theorem comp {f : β → σ} {g : α → β} (hf : PrimrecIn O f) (hg : PrimrecIn O g) : PrimrecIn O fun a => f (g a) :=
+  ((casesOn1 0 (.comp hf (pred.comp hg))).comp (Nat.Primrec.to_PrimrecIn (@Primcodable.prim α _))).of_eq fun n => by
+    cases @decode α _ n <;> simp [encodek]
+
+theorem succ : PrimrecIn O Nat.succ :=
+  nat_iff.2 Nat.PrimrecIn.succ
+
+theorem oracle : PrimrecIn O O := nat_iff.2 Nat.PrimrecIn.oracle
+
+theorem pred : PrimrecIn O Nat.pred :=
+  nat_iff.2 Nat.PrimrecIn.pred
+
+theorem encode_iff {f : α → σ} : (PrimrecIn O fun a => encode (f a)) ↔ PrimrecIn O f :=
+  ⟨fun h => Nat.PrimrecIn.of_eq h fun n => by cases @decode α _ n <;> rfl, PrimrecIn.encode.comp⟩
+
+theorem ofNat_iff {α β} [Denumerable α] [Primcodable β] {f : α → β} :
+    PrimrecIn O f ↔ PrimrecIn O fun n => f (ofNat α n) :=
+  dom_denumerable.trans <| nat_iff.symm.trans encode_iff
+
+protected theorem ofNat (α) [Denumerable α] : PrimrecIn O (ofNat α) :=
+  ofNat_iff.1 PrimrecIn.id
+
+theorem option_some_iff {f : α → σ} : (PrimrecIn O fun a => some (f a)) ↔ PrimrecIn O f :=
+  ⟨fun h => encode_iff.1 <| pred.comp <| encode_iff.2 h, option_some.comp⟩
+
+theorem of_equiv {β} {e : β ≃ α} :
+    haveI := Primcodable.ofEquiv α e
+    PrimrecIn O e :=
+  letI : Primcodable β := Primcodable.ofEquiv α e
+  encode_iff.1 PrimrecIn.encode
+
+theorem of_equiv_symm {β} {e : β ≃ α} :
+    haveI := Primcodable.ofEquiv α e
+    PrimrecIn O e.symm :=
+  letI := Primcodable.ofEquiv α e
+  encode_iff.1 (show PrimrecIn O fun a => encode (e (e.symm a)) by simp [PrimrecIn.encode])
+
+theorem of_equiv_iff {β} (e : β ≃ α) {f : σ → β} :
+    haveI := Primcodable.ofEquiv α e
+    (PrimrecIn O fun a => e (f a)) ↔ PrimrecIn O f :=
+  letI := Primcodable.ofEquiv α e
+  ⟨fun h => (of_equiv_symm.comp h).of_eq fun a => by simp, of_equiv.comp⟩
+
+theorem of_equiv_symm_iff {β} (e : β ≃ α) {f : σ → α} :
+    haveI := Primcodable.ofEquiv α e
+    (PrimrecIn O fun a => e.symm (f a)) ↔ PrimrecIn O f :=
+  letI := Primcodable.ofEquiv α e
+  ⟨fun h => (of_equiv.comp h).of_eq fun a => by simp, of_equiv_symm.comp⟩
+
+end PrimrecIn
+
+namespace Primcodable
+
+open Nat.PrimrecIn
+
+-- instance prod {α β} [Primcodable α] [Primcodable β] : Primcodable (α × β) :=
+--   ⟨((casesOn' zero ((casesOn' zero .succ).comp (pair right ((@Primcodable.prim β).comp left)))).comp
+--           (pair right ((@Primcodable.prim α).comp left))).of_eq
+--       fun n => by
+--       simp only [Nat.unpaired, Nat.unpair_pair, decode_prod_val]
+--       cases @decode α _ n.unpair.1; · simp
+--       cases @decode β _ n.unpair.2 <;> simp⟩
+
+end Primcodable
+
+namespace PrimrecIn
+
+variable {α : Type*} [Primcodable α]
+
+open Nat.PrimrecIn
+
+theorem fst {α β} [Primcodable α] [Primcodable β] : PrimrecIn O (@Prod.fst α β) :=
+  ((casesOn' zero
+            ((casesOn' zero (Nat.PrimrecIn.succ.comp left)).comp
+              (pair right ((Nat.Primrec.to_PrimrecIn (@Primcodable.prim β _)).comp left)))).comp
+        (pair right ((Nat.Primrec.to_PrimrecIn (@Primcodable.prim α _)).comp left))).of_eq
+    fun n => by
+    simp only [Nat.unpaired, Nat.unpair_pair, decode_prod_val]
+    cases @decode α _ n.unpair.1 <;> simp
+    cases @decode β _ n.unpair.2 <;> simp
+
+theorem snd {α β} [Primcodable α] [Primcodable β] : PrimrecIn O (@Prod.snd α β) :=
+  ((casesOn' zero
+            ((casesOn' zero (Nat.PrimrecIn.succ.comp right)).comp
+              (pair right ((Nat.Primrec.to_PrimrecIn (@Primcodable.prim β _)).comp left)))).comp
+        (pair right ((Nat.Primrec.to_PrimrecIn (@Primcodable.prim α _)).comp left))).of_eq
+    fun n => by
+    simp only [Nat.unpaired, Nat.unpair_pair, decode_prod_val]
+    cases @decode α _ n.unpair.1 <;> simp
+    cases @decode β _ n.unpair.2 <;> simp
+
+theorem pair {α β γ} [Primcodable α] [Primcodable β] [Primcodable γ] {f : α → β} {g : α → γ}
+    (hf : PrimrecIn O f) (hg : PrimrecIn O g) : PrimrecIn O fun a => (f a, g a) :=
+  ((casesOn1 0
+            (Nat.PrimrecIn.succ.comp <|
+              .pair (Nat.PrimrecIn.pred.comp hf) (Nat.PrimrecIn.pred.comp hg))).comp
+        (Nat.Primrec.to_PrimrecIn (@Primcodable.prim α _))).of_eq
+    fun n => by cases @decode α _ n <;> simp [encodek]
+
+theorem unpair : PrimrecIn O Nat.unpair :=
+  (pair (nat_iff.2 .left) (nat_iff.2 .right)).of_eq fun n => by simp
+
+theorem list_get?₁ : ∀ l : List α, PrimrecIn O l.get?
+  | [] => dom_denumerable.2 zero
+  | a :: l =>
+    dom_denumerable.2 <|
+      (casesOn1 (encode a).succ <| dom_denumerable.1 <| list_get?₁ l).of_eq fun n => by
+        cases n <;> simp
+
+end PrimrecIn
+
+/-- `PrimrecIn₂ O f` means `f` is a binary primitive recursive function.
+  This is technically unnecessary since we can always curry all
+  the arguments together, but there are enough natural two-arg
+  functions that it is convenient to express this directly. -/
+def PrimrecIn₂ (O) {α β σ} [Primcodable α] [Primcodable β] [Primcodable σ] (f : α → β → σ) :=
+  PrimrecIn O fun p : α × β => f p.1 p.2
+
+/-- `PrimrecInPred O p` means `p : α → Prop` is a (decidable)
+  primitive recursive predicate, which is to say that
+  `decide ∘ p : α → Bool` is primitive recursive. -/
+def PrimrecInPred (O) {α} [Primcodable α] (p : α → Prop) [DecidablePred p] :=
+  PrimrecIn O fun a => decide (p a)
+
+/-- `PrimrecInRel O p` means `p : α → β → Prop` is a (decidable)
+  primitive recursive relation, which is to say that
+  `decide ∘ p : α → β → Bool` is primitive recursive. -/
+def PrimrecInRel (O) {α β} [Primcodable α] [Primcodable β] (s : α → β → Prop)
+    [∀ a b, Decidable (s a b)] :=
+  PrimrecIn₂ O fun a b => decide (s a b)
+
+namespace PrimrecIn₂
+
+variable {α : Type*} {β : Type*} {σ : Type*}
+variable [Primcodable α] [Primcodable β] [Primcodable σ]
+
+theorem mk {f : α → β → σ} (hf : PrimrecIn O fun p : α × β => f p.1 p.2) : PrimrecIn₂ O f := hf
+
+theorem of_eq {f g : α → β → σ} (hg : PrimrecIn₂ O f) (H : ∀ a b, f a b = g a b) : PrimrecIn₂ O g :=
+  (by funext a b; apply H : f = g) ▸ hg
+
+theorem const (x : σ) : PrimrecIn₂ O fun (_ : α) (_ : β) => x :=
+  PrimrecIn.const _
+
+protected theorem pair : PrimrecIn₂ O (@Prod.mk α β) :=
+  PrimrecIn.pair .fst .snd
+
+theorem left : PrimrecIn₂ O fun (a : α) (_ : β) => a :=
+  .fst
+
+theorem right : PrimrecIn₂ O fun (_ : α) (b : β) => b :=
+  .snd
+
+theorem natPair : PrimrecIn₂ O Nat.pair := by simp [PrimrecIn₂, PrimrecIn]; constructor
+
+theorem unpaired {f : ℕ → ℕ → α} : PrimrecIn O (Nat.unpaired f) ↔ PrimrecIn₂ O f :=
+  ⟨fun h => by simpa using h.comp natPair, fun h => h.comp PrimrecIn.unpair⟩
+
+theorem unpaired' {f : ℕ → ℕ → ℕ} : Nat.PrimrecIn O (Nat.unpaired f) ↔ PrimrecIn₂ O f :=
+  PrimrecIn.nat_iff.symm.trans unpaired
+
+theorem encode_iff {f : α → β → σ} : (PrimrecIn₂ O fun a b => encode (f a b)) ↔ PrimrecIn₂ O f :=
+  PrimrecIn.encode_iff
+
+theorem option_some_iff {f : α → β → σ} : (PrimrecIn₂ O fun a b => some (f a b)) ↔ PrimrecIn₂ O f :=
+  PrimrecIn.option_some_iff
+
+theorem ofNat_iff {α β σ} [Denumerable α] [Denumerable β] [Primcodable σ] {f : α → β → σ} :
+    PrimrecIn₂ O f ↔ PrimrecIn₂ O fun m n : ℕ => f (ofNat α m) (ofNat β n) :=
+  (PrimrecIn.ofNat_iff.trans <| by simp).trans unpaired
+
+theorem uncurry {f : α → β → σ} : PrimrecIn O (Function.uncurry f) ↔ PrimrecIn₂ O f := by
+  rw [show Function.uncurry f = fun p : α × β => f p.1 p.2 from funext fun ⟨a, b⟩ => rfl]; rfl
+
+theorem curry {f : α × β → σ} : PrimrecIn₂ O (Function.curry f) ↔ PrimrecIn O f := by
+  rw [← uncurry, Function.uncurry_curry]
+
+end PrimrecIn₂
+
+section Comp
+
+variable {α : Type*} {β : Type*} {γ : Type*} {δ : Type*} {σ : Type*}
+variable [Primcodable α] [Primcodable β] [Primcodable γ] [Primcodable δ] [Primcodable σ]
+
+theorem PrimrecIn.comp₂ {f : γ → σ} {g : α → β → γ} (hf : PrimrecIn O f) (hg : PrimrecIn₂ O g) :
+    PrimrecIn₂ O fun a b => f (g a b) :=
+  hf.comp hg
+
+theorem PrimrecIn₂.comp {f : β → γ → σ} {g : α → β} {h : α → γ} (hf : PrimrecIn₂ O f) (hg : PrimrecIn O g)
+    (hh : PrimrecIn O h) : PrimrecIn O fun a => f (g a) (h a) :=
+  PrimrecIn.comp hf (hg.pair hh)
+
+theorem PrimrecIn₂.comp₂ {f : γ → δ → σ} {g : α → β → γ} {h : α → β → δ} (hf : PrimrecIn₂ O f)
+    (hg : PrimrecIn₂ O g) (hh : PrimrecIn₂ O h) : PrimrecIn₂ O fun a b => f (g a b) (h a b) :=
+  hf.comp hg hh
+
+theorem PrimrecInPred.comp {p : β → Prop} [DecidablePred p] {f : α → β} :
+    PrimrecInPred O p → PrimrecIn O f → PrimrecInPred O fun a => p (f a) :=
+  PrimrecIn.comp
+
+theorem PrimrecInRel.comp {R : β → γ → Prop} [∀ a b, Decidable (R a b)] {f : α → β} {g : α → γ} :
+    PrimrecInRel O R → PrimrecIn O f → PrimrecIn O g → PrimrecInPred O fun a => R (f a) (g a) :=
+  PrimrecIn₂.comp
+
+theorem PrimrecInRel.comp₂ {R : γ → δ → Prop} [∀ a b, Decidable (R a b)] {f : α → β → γ}
+    {g : α → β → δ} :
+    PrimrecInRel O R → PrimrecIn₂ O f → PrimrecIn₂ O g → PrimrecInRel O fun a b => R (f a b) (g a b) :=
+  PrimrecInRel.comp
+
+end Comp
+
+theorem PrimrecInPred.of_eq {α} [Primcodable α] {p q : α → Prop} [DecidablePred p] [DecidablePred q]
+    (hp : PrimrecInPred O p) (H : ∀ a, p a ↔ q a) : PrimrecInPred O q :=
+  PrimrecIn.of_eq hp fun a => Bool.decide_congr (H a)
+
+theorem PrimrecInRel.of_eq {α β} [Primcodable α] [Primcodable β] {r s : α → β → Prop}
+    [∀ a b, Decidable (r a b)] [∀ a b, Decidable (s a b)] (hr : PrimrecInRel O r)
+    (H : ∀ a b, r a b ↔ s a b) : PrimrecInRel O s :=
+  PrimrecIn₂.of_eq hr fun a b => Bool.decide_congr (H a b)
+
+namespace PrimrecIn₂
+
+variable {α : Type*} {β : Type*} {σ : Type*}
+variable [Primcodable α] [Primcodable β] [Primcodable σ]
+
+open Nat.PrimrecIn
+
+theorem swap {f : α → β → σ} (h : PrimrecIn₂ O f) : PrimrecIn₂ O (swap f) :=
+  h.comp₂ PrimrecIn₂.right PrimrecIn₂.left
+
+theorem nat_iff {f : α → β → σ} : PrimrecIn₂ O f ↔ Nat.PrimrecIn O
+    (.unpaired fun m n => encode <| (@decode α _ m).bind fun a => (@decode β _ n).map (f a)) := by
+  have :
+    ∀ (a : Option α) (b : Option β),
+      Option.map (fun p : α × β => f p.1 p.2)
+          (Option.bind a fun a : α => Option.map (Prod.mk a) b) =
+        Option.bind a fun a => Option.map (f a) b := fun a b => by
+          cases a <;> cases b <;> rfl
+  simp [PrimrecIn₂, PrimrecIn, this]
+
+theorem nat_iff' {f : α → β → σ} :
+    PrimrecIn₂ O f ↔
+      PrimrecIn₂ O fun m n : ℕ => (@decode α _ m).bind fun a => Option.map (f a) (@decode β _ n) :=
+  nat_iff.trans <| unpaired'.trans encode_iff
+
+end PrimrecIn₂
+
+namespace PrimrecIn
+
+variable {α : Type*} {β : Type*} {σ : Type*}
+variable [Primcodable α] [Primcodable β] [Primcodable σ]
+
+theorem to₂ {f : α × β → σ} (hf : PrimrecIn O f) : PrimrecIn₂ O fun a b => f (a, b) :=
+  hf.of_eq fun _ => rfl
+
+theorem nat_rec {f : α → β} {g : α → ℕ × β → β} (hf : PrimrecIn O f) (hg : PrimrecIn₂ O g) :
+    PrimrecIn₂ O fun a (n : ℕ) => n.rec (motive := fun _ => β) (f a) fun n IH => g a (n, IH) :=
+  PrimrecIn₂.nat_iff.2 <|
+    ((Nat.PrimrecIn.casesOn' .zero <|
+              (Nat.PrimrecIn.prec hf <|
+                    .comp hg <|
+                      Nat.PrimrecIn.left.pair <|
+                        (Nat.PrimrecIn.left.comp .right).pair <|
+                          Nat.PrimrecIn.pred.comp <| Nat.PrimrecIn.right.comp .right).comp <|
+                Nat.PrimrecIn.right.pair <| Nat.PrimrecIn.right.comp Nat.PrimrecIn.left).comp <|
+          Nat.PrimrecIn.id.pair <| (Nat.Primrec.to_PrimrecIn (@Primcodable.prim α _)).comp Nat.PrimrecIn.left).of_eq
+      fun n => by
+      simp only [Nat.unpaired, id_eq, Nat.unpair_pair, decode_prod_val, decode_nat,
+        Option.some_bind, Option.map_map, Option.map_some']
+      rcases @decode α _ n.unpair.1 with - | a; · rfl
+      simp only [Nat.pred_eq_sub_one, encode_some, Nat.succ_eq_add_one, encodek, Option.map_some',
+        Option.some_bind, Option.map_map]
+      induction' n.unpair.2 with m <;> simp [encodek]
+      simp [*, encodek]
+
+theorem nat_rec' {f : α → ℕ} {g : α → β} {h : α → ℕ × β → β}
+    (hf : PrimrecIn O f) (hg : PrimrecIn O g) (hh : PrimrecIn₂ O h) :
+    PrimrecIn O fun a => (f a).rec (motive := fun _ => β) (g a) fun n IH => h a (n, IH) :=
+  (nat_rec hg hh).comp .id hf
+
+theorem nat_rec₁ {f : ℕ → α → α} (a : α) (hf : PrimrecIn₂ O f) : PrimrecIn O (Nat.rec a f) :=
+  nat_rec' .id (const a) <| comp₂ hf PrimrecIn₂.right
+
+theorem nat_casesOn' {f : α → β} {g : α → ℕ → β} (hf : PrimrecIn O f) (hg : PrimrecIn₂ O g) :
+    PrimrecIn₂ O fun a (n : ℕ) => (n.casesOn (f a) (g a) : β) :=
+  nat_rec hf <| hg.comp₂ PrimrecIn₂.left <| comp₂ fst PrimrecIn₂.right
+
+theorem nat_casesOn {f : α → ℕ} {g : α → β} {h : α → ℕ → β} (hf : PrimrecIn O f) (hg : PrimrecIn O g)
+    (hh : PrimrecIn₂ O h) : PrimrecIn O fun a => ((f a).casesOn (g a) (h a) : β) :=
+  (nat_casesOn' hg hh).comp .id hf
+
+theorem nat_casesOn₁ {f : ℕ → α} (a : α) (hf : PrimrecIn O f) :
+    PrimrecIn O (fun (n : ℕ) => (n.casesOn a f : α)) :=
+  nat_casesOn .id (const a) (comp₂ hf .right)
+
+theorem nat_iterate {f : α → ℕ} {g : α → β} {h : α → β → β} (hf : PrimrecIn O f) (hg : PrimrecIn O g)
+    (hh : PrimrecIn₂ O h) : PrimrecIn O fun a => (h a)^[f a] (g a) :=
+  (nat_rec' hf hg (hh.comp₂ PrimrecIn₂.left <| snd.comp₂ PrimrecIn₂.right)).of_eq fun a => by
+    induction f a <;> simp [*, -Function.iterate_succ, Function.iterate_succ']
+
+theorem option_casesOn {o : α → Option β} {f : α → σ} {g : α → β → σ} (ho : PrimrecIn O o)
+    (hf : PrimrecIn O f) (hg : PrimrecIn₂ O g) :
+    @PrimrecIn O _ σ _ _ fun a => Option.casesOn (o a) (f a) (g a) :=
+  encode_iff.1 <|
+    (nat_casesOn (encode_iff.2 ho) (encode_iff.2 hf) <|
+          pred.comp₂ <|
+            PrimrecIn₂.encode_iff.2 <|
+              (PrimrecIn₂.nat_iff'.1 hg).comp₂ ((@PrimrecIn.encode α _).comp fst).to₂
+                PrimrecIn₂.right).of_eq
+      fun a => by rcases o a with - | b <;> simp [encodek]
+
+theorem option_bind {f : α → Option β} {g : α → β → Option σ} (hf : PrimrecIn O f) (hg : PrimrecIn₂ O g) :
+    PrimrecIn O fun a => (f a).bind (g a) :=
+  (option_casesOn hf (const none) hg).of_eq fun a => by cases f a <;> rfl
+
+theorem option_bind₁ {f : α → Option σ} (hf : PrimrecIn O f) : PrimrecIn O fun o => Option.bind o f :=
+  option_bind .id (hf.comp snd).to₂
+
+theorem option_map {f : α → Option β} {g : α → β → σ} (hf : PrimrecIn O f) (hg : PrimrecIn₂ O g) :
+    PrimrecIn O fun a => (f a).map (g a) :=
+  (option_bind hf (option_some.comp₂ hg)).of_eq fun x => by cases f x <;> rfl
+
+theorem option_map₁ {f : α → σ} (hf : PrimrecIn O f) : PrimrecIn O (Option.map f) :=
+  option_map .id (hf.comp snd).to₂
+
+theorem option_iget [Inhabited α] : PrimrecIn O (@Option.iget α _) :=
+  (option_casesOn .id (const <| @default α _) .right).of_eq fun o => by cases o <;> rfl
+
+theorem option_isSome : PrimrecIn O (@Option.isSome α) :=
+  (option_casesOn .id (const false) (const true).to₂).of_eq fun o => by cases o <;> rfl
+
+theorem option_getD : PrimrecIn₂ O (@Option.getD α) :=
+  PrimrecIn.of_eq (option_casesOn PrimrecIn₂.left PrimrecIn₂.right .right) fun ⟨o, a⟩ => by
+    cases o <;> rfl
+
+theorem bind_decode_iff {f : α → β → Option σ} :
+    (PrimrecIn₂ O fun a n => (@decode β _ n).bind (f a)) ↔ PrimrecIn₂ O f :=
+  ⟨fun h => by simpa [encodek] using h.comp fst ((@PrimrecIn.encode β _).comp snd), fun h =>
+    option_bind (PrimrecIn.decode.comp snd) <| h.comp (fst.comp fst) snd⟩
+
+theorem map_decode_iff {f : α → β → σ} :
+    (PrimrecIn₂ O fun a n => (@decode β _ n).map (f a)) ↔ PrimrecIn₂ O f := by
+  simp only [Option.map_eq_bind]
+  exact bind_decode_iff.trans PrimrecIn₂.option_some_iff
+
+theorem nat_add : PrimrecIn₂ O ((· + ·) : ℕ → ℕ → ℕ) :=
+  PrimrecIn₂.unpaired'.1 Nat.PrimrecIn.add
+
+theorem nat_sub : PrimrecIn₂ O ((· - ·) : ℕ → ℕ → ℕ) :=
+  PrimrecIn₂.unpaired'.1 Nat.PrimrecIn.sub
+
+theorem nat_mul : PrimrecIn₂ O ((· * ·) : ℕ → ℕ → ℕ) :=
+  PrimrecIn₂.unpaired'.1 Nat.PrimrecIn.mul
+
+theorem cond {c : α → Bool} {f : α → σ} {g : α → σ} (hc : PrimrecIn O c) (hf : PrimrecIn O f)
+    (hg : PrimrecIn O g) : PrimrecIn O fun a => bif (c a) then (f a) else (g a) :=
+  (nat_casesOn (encode_iff.2 hc) hg (hf.comp fst).to₂).of_eq fun a => by cases c a <;> rfl
+
+theorem ite {c : α → Prop} [DecidablePred c] {f : α → σ} {g : α → σ} (hc : PrimrecInPred O c)
+    (hf : PrimrecIn O f) (hg : PrimrecIn O g) : PrimrecIn O fun a => if c a then f a else g a := by
+  simpa [Bool.cond_decide] using cond hc hf hg
+
+theorem nat_le : PrimrecInRel O ((· ≤ ·) : ℕ → ℕ → Prop) :=
+  (nat_casesOn nat_sub (const true) (const false).to₂).of_eq fun p => by
+    dsimp [swap]
+    rcases e : p.1 - p.2 with - | n
+    · simp [Nat.sub_eq_zero_iff_le.1 e]
+    · simp [not_le.2 (Nat.lt_of_sub_eq_succ e)]
+
+theorem nat_min : PrimrecIn₂ O (@min ℕ _) :=
+  ite nat_le fst snd
+
+theorem nat_max : PrimrecIn₂ O (@max ℕ _) :=
+  ite (nat_le.comp fst snd) snd fst
+
+theorem dom_bool (f : Bool → α) : PrimrecIn O f :=
+  (cond .id (const (f true)) (const (f false))).of_eq fun b => by cases b <;> rfl
+
+theorem dom_bool₂ (f : Bool → Bool → α) : PrimrecIn₂ O f :=
+  (cond fst ((dom_bool (f true)).comp snd) ((dom_bool (f false)).comp snd)).of_eq fun ⟨a, b⟩ => by
+    cases a <;> rfl
+
+protected theorem not : PrimrecIn O not :=
+  dom_bool _
+
+protected theorem and : PrimrecIn₂ O and :=
+  dom_bool₂ _
+
+protected theorem or : PrimrecIn₂ O or :=
+  dom_bool₂ _
+
+theorem _root_.PrimrecInPred.not {p : α → Prop} [DecidablePred p] (hp : PrimrecInPred O p) :
+    PrimrecInPred O fun a => ¬p a :=
+  (PrimrecIn.not.comp hp).of_eq fun n => by simp
+
+theorem _root_.PrimrecInPred.and {p q : α → Prop} [DecidablePred p] [DecidablePred q]
+    (hp : PrimrecInPred O p) (hq : PrimrecInPred O q) : PrimrecInPred O fun a => p a ∧ q a :=
+  (PrimrecIn.and.comp hp hq).of_eq fun n => by simp
+
+theorem _root_.PrimrecInPred.or {p q : α → Prop} [DecidablePred p] [DecidablePred q]
+    (hp : PrimrecInPred O p) (hq : PrimrecInPred O q) : PrimrecInPred O fun a => p a ∨ q a :=
+  (PrimrecIn.or.comp hp hq).of_eq fun n => by simp
+
+protected theorem beq [DecidableEq α] : PrimrecIn₂ O (@BEq.beq α _) :=
+  have : PrimrecInRel O fun a b : ℕ => a = b :=
+    (PrimrecInPred.and nat_le nat_le.swap).of_eq fun a => by simp [le_antisymm_iff]
+  (this.comp₂ (PrimrecIn.encode.comp₂ PrimrecIn₂.left) (PrimrecIn.encode.comp₂ PrimrecIn₂.right)).of_eq
+    fun _ _ => encode_injective.eq_iff
+
+protected theorem eq [DecidableEq α] : PrimrecInRel O (@Eq α) := PrimrecIn.beq
+
+theorem nat_lt : PrimrecInRel O ((· < ·) : ℕ → ℕ → Prop) :=
+  -- (nat_le.comp snd fst).not.of_eq fun p => by simp
+  (PrimrecInPred.not (nat_le.comp snd fst)).of_eq fun p => by simp
+
+theorem option_guard {p : α → β → Prop} [∀ a b, Decidable (p a b)] (hp : PrimrecInRel O p) {f : α → β}
+    (hf : PrimrecIn O f) : PrimrecIn O fun a => Option.guard (p a) (f a) :=
+  -- ite (hp.comp PrimrecIn.id hf) (option_some_iff.2 hf) (const none)
+  ite (by
+    refine PrimrecInRel.comp ?_ ?_ ?_
+    exact PrimrecIn.eq
+    simp [*] at *
+    · refine ite ?_ ?_ ?_
+      · refine PrimrecInRel.comp hp ?_ hf
+        exact PrimrecIn.id
+      · exact const true
+      · exact const false
+    exact const true
+    ) (option_some_iff.2 hf) (const none)
+  -- ite (PrimrecInRel.comp hp PrimrecIn.id hf) (option_some_iff.2 hf) (const none)
+
+theorem option_orElse : PrimrecIn₂ O ((· <|> ·) : Option α → Option α → Option α) :=
+  (option_casesOn fst snd (fst.comp fst).to₂).of_eq fun ⟨o₁, o₂⟩ => by cases o₁ <;> cases o₂ <;> rfl
+
+protected theorem decode₂ : PrimrecIn O (decode₂ α) :=
+  option_bind .decode <|
+    option_guard (PrimrecIn.beq.comp₂ (by exact encode_iff.mpr snd) (by exact fst.comp fst)) snd
+
+theorem list_findIdx₁ {p : α → β → Bool} (hp : PrimrecIn₂ O p) :
+    ∀ l : List β, PrimrecIn O fun a => l.findIdx (p a)
+| [] => const 0
+| a :: l => (cond (hp.comp .id (const a)) (const 0) (succ.comp (list_findIdx₁ hp l))).of_eq fun n =>
+  by simp [List.findIdx_cons]
+
+theorem list_idxOf₁ [DecidableEq α] (l : List α) : PrimrecIn O fun a => l.idxOf a :=
+  list_findIdx₁ (.swap .beq) l
+
+@[deprecated (since := "2025-01-30")] alias list_indexOf₁ := list_idxOf₁
+
+theorem dom_fintype [Finite α] (f : α → σ) : PrimrecIn O f :=
+  let ⟨l, _, m⟩ := Finite.exists_univ_list α
+  option_some_iff.1 <| by
+    haveI := decidableEqOfEncodable α
+    refine ((list_get?₁ (l.map f)).comp (list_idxOf₁ l)).of_eq fun a => ?_
+    rw [List.get?_eq_getElem?, List.getElem?_map, List.getElem?_idxOf (m a), Option.map_some']
+
+-- Porting note: These are new lemmas
+-- I added it because it actually simplified the proofs
+-- and because I couldn't understand the original proof
+/-- A function is `PrimrecInBounded O` if its size is bounded by a primitive recursive function -/
+def PrimrecInBounded (O:ℕ→ℕ) (f : α → β) : Prop :=
+  ∃ g : α → ℕ, PrimrecIn O g ∧ ∀ x, encode (f x) ≤ g x
+
+theorem nat_findGreatest {f : α → ℕ} {p : α → ℕ → Prop} [∀ x n, Decidable (p x n)]
+    (hf : PrimrecIn O f) (hp : PrimrecInRel O p) : PrimrecIn O fun x => (f x).findGreatest (p x) :=
+  (nat_rec' (h := fun x nih => if p x (nih.1 + 1) then nih.1 + 1 else nih.2)
+    hf (const 0) (ite (hp.comp fst (snd |> fst.comp |> succ.comp))
+      (snd |> fst.comp |> succ.comp) (snd.comp snd))).of_eq fun x => by
+        induction f x <;> simp [Nat.findGreatest, *]
+
+/-- To show a function `f : α → ℕ` is primitive recursive, it is enough to show that the function
+  is bounded by a primitive recursive function and that its graph is primitive recursive -/
+theorem of_graph {f : α → ℕ} (h₁ : PrimrecInBounded O f)
+    (h₂ : PrimrecInRel O fun a b => f a = b) : PrimrecIn O f := by
+  rcases h₁ with ⟨g, pg, hg : ∀ x, f x ≤ g x⟩
+  refine (nat_findGreatest pg h₂).of_eq fun n => ?_
+  exact (Nat.findGreatest_spec (P := fun b => f n = b) (hg n) rfl).symm
+
+-- We show that division is primitive recursive by showing that the graph is
+theorem nat_div : PrimrecIn₂ O ((· / ·) : ℕ → ℕ → ℕ) := by
+  refine of_graph ⟨_, fst, fun p => Nat.div_le_self _ _⟩ ?_
+  have : PrimrecInRel O fun (a : ℕ × ℕ) (b : ℕ) => (a.2 = 0 ∧ b = 0) ∨
+      (0 < a.2 ∧ b * a.2 ≤ a.1 ∧ a.1 < (b + 1) * a.2) :=
+    PrimrecInPred.or
+      (.and (const 0 |> PrimrecIn.eq.comp (fst |> snd.comp)) (const 0 |> PrimrecIn.eq.comp snd))
+      (.and (nat_lt.comp (const 0) (fst |> snd.comp)) <|
+          .and (nat_le.comp (nat_mul.comp snd (fst |> snd.comp)) (fst |> fst.comp))
+          (nat_lt.comp (fst.comp fst) (nat_mul.comp (PrimrecIn.succ.comp snd) (snd.comp fst))))
+  refine this.of_eq ?_
+  rintro ⟨a, k⟩ q
+  if H : k = 0 then simp [H, eq_comm]
+  else
+    have : q * k ≤ a ∧ a < (q + 1) * k ↔ q = a / k := by
+      rw [le_antisymm_iff, ← (@Nat.lt_succ _ q), Nat.le_div_iff_mul_le (Nat.pos_of_ne_zero H),
+          Nat.div_lt_iff_lt_mul (Nat.pos_of_ne_zero H)]
+    simpa [H, zero_lt_iff, eq_comm (b := q)]
+
+theorem nat_mod : PrimrecIn₂ O ((· % ·) : ℕ → ℕ → ℕ) :=
+  (nat_sub.comp fst (nat_mul.comp snd nat_div)).to₂.of_eq fun m n => by
+    apply Nat.sub_eq_of_eq_add
+    simp [add_comm (m % n), Nat.div_add_mod]
+
+theorem nat_bodd : PrimrecIn O Nat.bodd :=
+  (PrimrecIn.beq.comp (nat_mod.comp .id (const 2)) (const 1)).of_eq fun n => by
+    cases H : n.bodd <;> simp [Nat.mod_two_of_bodd, H]
+
+theorem nat_div2 : PrimrecIn O Nat.div2 :=
+  (nat_div.comp .id (const 2)).of_eq fun n => n.div2_val.symm
+
+theorem nat_double : PrimrecIn O (fun n : ℕ => 2 * n) :=
+  nat_mul.comp (const _) PrimrecIn.id
+
+theorem nat_double_succ : PrimrecIn O (fun n : ℕ => 2 * n + 1) :=
+  nat_double |> PrimrecIn.succ.comp
+
+end PrimrecIn
+
+section
+
+variable {α : Type*} {β : Type*} {σ : Type*}
+variable [Primcodable α] [Primcodable β] [Primcodable σ]
+variable (H : Nat.Primrec fun n => Encodable.encode (@decode (List β) _ n))
+
+open PrimrecIn
+
+private def prim : Primcodable (List β) := ⟨H⟩
+
+private theorem list_casesOn' {f : α → List β} {g : α → σ} {h : α → β × List β → σ}
+    (hf : haveI := prim H; PrimrecIn O f) (hg : PrimrecIn O g) (hh : haveI := prim H; PrimrecIn₂ O h) :
+    @PrimrecIn O _ σ _ _ fun a => List.casesOn (f a) (g a) fun b l => h a (b, l) :=
+  letI := prim H
+  have :
+    @PrimrecIn O _ (Option σ) _ _ fun a =>
+      (@decode (Option (β × List β)) _ (encode (f a))).map fun o => Option.casesOn o (g a) (h a) :=
+    ((@map_decode_iff _ (Option (β × List β)) _ _ _ _ _).2 <|
+      to₂ <|
+        option_casesOn snd (hg.comp fst) (hh.comp₂ (fst.comp₂ PrimrecIn₂.left) PrimrecIn₂.right)).comp
+      .id (encode_iff.2 hf)
+  option_some_iff.1 <| this.of_eq fun a => by rcases f a with - | ⟨b, l⟩ <;> simp [encodek]
+
+private theorem list_foldl' {f : α → List β} {g : α → σ} {h : α → σ × β → σ}
+    (hf : haveI := prim H; PrimrecIn O f) (hg : PrimrecIn O g) (hh : haveI := prim H; PrimrecIn₂ O h) :
+    PrimrecIn O fun a => (f a).foldl (fun s b => h a (s, b)) (g a) := by
+  letI := prim H
+  let G (a : α) (IH : σ × List β) : σ × List β := List.casesOn IH.2 IH fun b l => (h a (IH.1, b), l)
+  have hG : PrimrecIn₂ O G := list_casesOn' H (snd.comp snd) snd <|
+    to₂ <|
+    pair (hh.comp (fst.comp fst) <| pair ((fst.comp snd).comp fst) (fst.comp snd))
+      (snd.comp snd)
+  let F := fun (a : α) (n : ℕ) => (G a)^[n] (g a, f a)
+  have hF : PrimrecIn O fun a => (F a (encode (f a))).1 :=
+    (fst.comp <|
+      nat_iterate (encode_iff.2 hf) (pair hg hf) <|
+      hG)
+  suffices ∀ a n, F a n = (((f a).take n).foldl (fun s b => h a (s, b)) (g a), (f a).drop n) by
+    refine hF.of_eq fun a => ?_
+    rw [this, List.take_of_length_le (length_le_encode _)]
+  introv
+  dsimp only [F]
+  generalize f a = l
+  generalize g a = x
+  induction n generalizing l x with
+  | zero => rfl
+  | succ n IH =>
+    simp only [iterate_succ, comp_apply]
+    rcases l with - | ⟨b, l⟩ <;> simp [G, IH]
+
+private theorem list_cons' : (haveI := prim H; PrimrecIn₂ O (@List.cons β)) :=
+  letI := prim H
+  encode_iff.1 (succ.comp <| PrimrecIn₂.natPair.comp (encode_iff.2 fst) (encode_iff.2 snd))
+
+private theorem list_reverse' :
+    haveI := prim H
+    PrimrecIn O (@List.reverse β) :=
+  letI := prim H
+  (list_foldl' H .id (const []) <| to₂ <| ((list_cons' H).comp snd fst).comp snd).of_eq
+    (suffices ∀ l r, List.foldl (fun (s : List β) (b : β) => b :: s) r l = List.reverseAux l r from
+      fun l => this l []
+    fun l => by induction l <;> simp [*, List.reverseAux])
+
+end
+
+namespace Primcodable
+
+variable {α : Type*} {β : Type*}
+variable [Primcodable α] [Primcodable β]
+
+open PrimrecIn
+
+-- instance sum : Primcodable (α ⊕ β) :=
+--   ⟨PrimrecIn.nat_iff.1 <|
+--       (encode_iff.2
+--             (cond nat_bodd
+--               (((@PrimrecIn.decode β _).comp nat_div2).option_map <|
+--                 to₂ <| nat_double_succ.comp (PrimrecIn.encode.comp snd))
+--               (((@PrimrecIn.decode α _).comp nat_div2).option_map <|
+--                 to₂ <| nat_double.comp (PrimrecIn.encode.comp snd)))).of_eq
+--         fun n =>
+--         show _ = encode (decodeSum n) by
+--           simp only [decodeSum, Nat.boddDiv2_eq]
+--           cases Nat.bodd n <;> simp [decodeSum]
+--           · cases @decode α _ n.div2 <;> rfl
+--           · cases @decode β _ n.div2 <;> rfl⟩
+
+-- instance list : Primcodable (List α) :=
+--   ⟨letI H := @Primcodable.prim (List ℕ) _
+--     have : PrimrecIn₂ O fun (a : α) (o : Option (List ℕ)) => o.map (List.cons (encode a)) :=
+--       option_map snd <| (list_cons' H).comp ((@PrimrecIn.encode α _).comp (fst.comp fst)) snd
+--     have :
+--       PrimrecIn O fun n =>
+--         (ofNat (List ℕ) n).reverse.foldl
+--           (fun o m => (@decode α _ m).bind fun a => o.map (List.cons (encode a))) (some []) :=
+--       list_foldl' H ((list_reverse' H).comp (.ofNat (List ℕ))) (const (some []))
+--         (PrimrecIn.comp₂ (bind_decode_iff.2 <| .swap this) PrimrecIn₂.right)
+--     nat_iff.1 <|
+--       (encode_iff.2 this).of_eq fun n => by
+--         rw [List.foldl_reverse]
+--         apply Nat.case_strong_induction_on n; · simp
+--         intro n IH; simp
+--         rcases @decode α _ n.unpair.1 with - | a; · rfl
+--         simp only [decode_eq_ofNat, Option.some.injEq, Option.some_bind, Option.map_some']
+--         suffices ∀ (o : Option (List ℕ)) (p), encode o = encode p →
+--             encode (Option.map (List.cons (encode a)) o) = encode (Option.map (List.cons a) p) from
+--           this _ _ (IH _ (Nat.unpair_right_le n))
+--         intro o p IH
+--         cases o <;> cases p
+--         · rfl
+--         · injection IH
+--         · injection IH
+--         · exact congr_arg (fun k => (Nat.pair (encode a) k).succ.succ) (Nat.succ.inj IH)⟩
+end Primcodable
+
+namespace PrimrecIn
+
+variable {α : Type*} {β : Type*} {γ : Type*} {σ : Type*}
+variable [Primcodable α] [Primcodable β] [Primcodable γ] [Primcodable σ]
+
+theorem sumInl : PrimrecIn O (@Sum.inl α β) :=
+  encode_iff.1 <| nat_double.comp PrimrecIn.encode
+
+theorem sumInr : PrimrecIn O (@Sum.inr α β) :=
+  encode_iff.1 <| nat_double_succ.comp PrimrecIn.encode
+
+@[deprecated (since := "2025-02-21")] alias sum_inl := PrimrecIn.sumInl
+@[deprecated (since := "2025-02-21")] alias sum_inr := PrimrecIn.sumInr
+
+theorem sumCasesOn {f : α → β ⊕ γ} {g : α → β → σ} {h : α → γ → σ} (hf : PrimrecIn O f)
+    (hg : PrimrecIn₂ O g) (hh : PrimrecIn₂ O h) : @PrimrecIn O _ σ _ _ fun a => Sum.casesOn (f a) (g a) (h a) :=
+  option_some_iff.1 <|
+    (cond (nat_bodd.comp <| encode_iff.2 hf)
+          (option_map (PrimrecIn.decode.comp <| nat_div2.comp <| encode_iff.2 hf) hh)
+          (option_map (PrimrecIn.decode.comp <| nat_div2.comp <| encode_iff.2 hf) hg)).of_eq
+      fun a => by rcases f a with b | c <;> simp [Nat.div2_val, encodek]
+
+@[deprecated (since := "2025-02-21")] alias sum_casesOn := PrimrecIn.sumCasesOn
+
+theorem list_cons : PrimrecIn₂ O (@List.cons α) :=
+  list_cons' Primcodable.prim
+
+theorem list_casesOn {f : α → List β} {g : α → σ} {h : α → β × List β → σ} :
+    PrimrecIn O f →
+      PrimrecIn O g →
+        PrimrecIn₂ O h → @PrimrecIn O _ σ _ _ fun a => List.casesOn (f a) (g a) fun b l => h a (b, l) :=
+  list_casesOn' Primcodable.prim
+
+theorem list_foldl {f : α → List β} {g : α → σ} {h : α → σ × β → σ} :
+    PrimrecIn O f →
+      PrimrecIn O g → PrimrecIn₂ O h → PrimrecIn O fun a => (f a).foldl (fun s b => h a (s, b)) (g a) :=
+  list_foldl' Primcodable.prim
+
+theorem list_reverse : PrimrecIn O (@List.reverse α) :=
+  list_reverse' Primcodable.prim
+
+theorem list_foldr {f : α → List β} {g : α → σ} {h : α → β × σ → σ} (hf : PrimrecIn O f)
+    (hg : PrimrecIn O g) (hh : PrimrecIn₂ O h) :
+    PrimrecIn O fun a => (f a).foldr (fun b s => h a (b, s)) (g a) :=
+  (list_foldl (list_reverse.comp hf) hg <| to₂ <| hh.comp fst <| (pair snd fst).comp snd).of_eq
+    fun a => by simp [List.foldl_reverse]
+
+theorem list_head? : PrimrecIn O (@List.head? α) :=
+  (list_casesOn .id (const none) (option_some_iff.2 <| fst.comp snd).to₂).of_eq fun l => by
+    cases l <;> rfl
+
+theorem list_headI [Inhabited α] : PrimrecIn O (@List.headI α _) :=
+  (option_iget.comp list_head?).of_eq fun l => l.head!_eq_head?.symm
+
+theorem list_tail : PrimrecIn O (@List.tail α) :=
+  (list_casesOn .id (const []) (snd.comp snd).to₂).of_eq fun l => by cases l <;> rfl
+
+theorem list_rec {f : α → List β} {g : α → σ} {h : α → β × List β × σ → σ} (hf : PrimrecIn O f)
+    (hg : PrimrecIn O g) (hh : PrimrecIn₂ O h) :
+    @PrimrecIn O _ σ _ _ fun a => List.recOn (f a) (g a) fun b l IH => h a (b, l, IH) :=
+  let F (a : α) := (f a).foldr (fun (b : β) (s : List β × σ) => (b :: s.1, h a (b, s))) ([], g a)
+  have : PrimrecIn O F :=
+    list_foldr hf (pair (const []) hg) <|
+      to₂ <| pair ((list_cons.comp fst (fst.comp snd)).comp snd) hh
+  (snd.comp this).of_eq fun a => by
+    suffices F a = (f a, List.recOn (f a) (g a) fun b l IH => h a (b, l, IH)) by rw [this]
+    dsimp [F]
+    induction' f a with b l IH <;> simp [*]
+
+theorem list_get? : PrimrecIn₂ O (@List.get? α) :=
+  let F (l : List α) (n : ℕ) :=
+    l.foldl
+      (fun (s : ℕ ⊕ α) (a : α) =>
+        Sum.casesOn s (@Nat.casesOn (fun _ => ℕ ⊕ α) · (Sum.inr a) Sum.inl) Sum.inr)
+      (Sum.inl n)
+  have hF : PrimrecIn₂ O F :=
+    (list_foldl fst (sumInl.comp snd)
+      ((sumCasesOn fst (nat_casesOn snd (sumInr.comp <| snd.comp fst) (sumInl.comp snd).to₂).to₂
+              (sumInr.comp snd).to₂).comp
+          snd).to₂).to₂
+  have :
+    @PrimrecIn O _ (Option α) _ _ fun p : List α × ℕ => Sum.casesOn (F p.1 p.2) (fun _ => none) some :=
+    sumCasesOn hF (const none).to₂ (option_some.comp snd).to₂
+  this.to₂.of_eq fun l n => by
+    dsimp; symm
+    induction' l with a l IH generalizing n; · rfl
+    rcases n with - | n
+    · dsimp [F]
+      clear IH
+      induction' l with _ l IH <;> simp [*]
+    · apply IH
+
+theorem list_getElem? : PrimrecIn₂ O (fun (l : List α) (n : ℕ) => l[n]?) := by
+  convert list_get?
+  ext
+  simp
+
+theorem list_getD (d : α) : PrimrecIn₂ O fun l n => List.getD l n d := by
+  simp only [List.getD_eq_getElem?_getD]
+  exact option_getD.comp₂ list_getElem? (const _)
+
+theorem list_getI [Inhabited α] : PrimrecIn₂ O (@List.getI α _) :=
+  list_getD _
+
+theorem list_append : PrimrecIn₂ O ((· ++ ·) : List α → List α → List α) :=
+  -- (list_foldr fst snd <| to₂ <| comp (@list_cons α _) snd).to₂.of_eq fun l₁ l₂ => by
+  (list_foldr fst snd <| to₂ <| PrimrecIn.comp (list_cons) snd).to₂.of_eq fun l₁ l₂ => by
+    induction l₁ <;> simp [*]
+
+theorem list_concat : PrimrecIn₂ O fun l (a : α) => l ++ [a] :=
+  list_append.comp fst (list_cons.comp snd (const []))
+
+theorem list_map {f : α → List β} {g : α → β → σ} (hf : PrimrecIn O f) (hg : PrimrecIn₂ O g) :
+    PrimrecIn O fun a => (f a).map (g a) :=
+  (list_foldr hf (const []) <|
+        to₂ <| list_cons.comp (hg.comp fst (fst.comp snd)) (snd.comp snd)).of_eq
+    fun a => by induction f a <;> simp [*]
+
+theorem list_range : PrimrecIn O List.range :=
+  (nat_rec' .id (const []) ((list_concat.comp snd fst).comp snd).to₂).of_eq fun n => by
+    simp; induction n <;> simp [*, List.range_succ]
+
+theorem list_flatten : PrimrecIn O (@List.flatten α) :=
+  -- (list_foldr .id (const []) <| to₂ <| comp (@list_append α _) snd).of_eq fun l => by
+  (list_foldr .id (const []) <| to₂ <| PrimrecIn.comp (list_append) snd).of_eq fun l => by
+    dsimp; induction l <;> simp [*]
+
+@[deprecated (since := "2024-10-15")] alias list_join := list_flatten
+
+theorem list_flatMap {f : α → List β} {g : α → β → List σ} (hf : PrimrecIn O f) (hg : PrimrecIn₂ O g) :
+    PrimrecIn O (fun a => (f a).flatMap (g a)) := list_flatten.comp (list_map hf hg)
+
+@[deprecated (since := "2024-10-16")] alias list_bind := list_flatMap
+
+theorem optionToList : PrimrecIn O (Option.toList : Option α → List α) :=
+  (option_casesOn PrimrecIn.id (const [])
+    ((list_cons.comp PrimrecIn.id (const [])).comp₂ PrimrecIn₂.right)).of_eq
+  (fun o => by rcases o <;> simp)
+
+theorem listFilterMap {f : α → List β} {g : α → β → Option σ}
+    (hf : PrimrecIn O f) (hg : PrimrecIn₂ O g) : PrimrecIn O fun a => (f a).filterMap (g a) :=
+  (list_flatMap hf (comp₂ optionToList hg)).of_eq
+    fun _ ↦ Eq.symm <| List.filterMap_eq_flatMap_toList _ _
+
+theorem list_length : PrimrecIn O (@List.length α) :=
+  -- (list_foldr (@PrimrecIn.id (List α) _) (const 0) <| to₂ <| (succ.comp <| snd.comp snd).to₂).of_eq
+  --   fun l => by dsimp; induction l <;> simp [*]
+  (list_foldr (PrimrecIn.id) (const 0) <| to₂ <| (succ.comp <| snd.comp snd).to₂).of_eq
+    fun l => by dsimp; induction l <;> simp [*]
+
+theorem list_findIdx {f : α → List β} {p : α → β → Bool}
+    (hf : PrimrecIn O f) (hp : PrimrecIn₂ O p) : PrimrecIn O fun a => (f a).findIdx (p a) :=
+  (list_foldr hf (const 0) <|
+        to₂ <| cond (hp.comp fst <| fst.comp snd) (const 0) (succ.comp <| snd.comp snd)).of_eq
+    fun a => by dsimp; induction f a <;> simp [List.findIdx_cons, *]
+
+theorem list_idxOf [DecidableEq α] : PrimrecIn₂ O (@List.idxOf α _) :=
+  to₂ <| list_findIdx snd <| PrimrecIn.beq.comp₂ snd.to₂ (fst.comp fst).to₂
+
+@[deprecated (since := "2025-01-30")] alias list_indexOf := list_idxOf
+
+theorem nat_strong_rec (f : α → ℕ → σ) {g : α → List σ → Option σ} (hg : PrimrecIn₂ O g)
+    (H : ∀ a n, g a ((List.range n).map (f a)) = some (f a n)) : PrimrecIn₂ O f :=
+  suffices PrimrecIn₂ O fun a n => (List.range n).map (f a) from
+    PrimrecIn₂.option_some_iff.1 <|
+      (list_get?.comp (this.comp fst (succ.comp snd)) snd).to₂.of_eq fun a n => by
+        simp [List.getElem?_range (Nat.lt_succ_self n)]
+  PrimrecIn₂.option_some_iff.1 <|
+    (nat_rec (const (some []))
+          (to₂ <|
+            option_bind (snd.comp snd) <|
+              to₂ <|
+                option_map (hg.comp (fst.comp fst) snd)
+                  (to₂ <| list_concat.comp (snd.comp fst) snd))).of_eq
+      fun a n => by
+      induction n with
+      | zero => rfl
+      | succ n IH => simp [IH, H, List.range_succ]
+
+theorem listLookup [DecidableEq α] : PrimrecIn₂ O (List.lookup : α → List (α × β) → Option β) :=
+  (to₂ <| list_rec snd (const none) <|
+    to₂ <|
+      cond (PrimrecIn.beq.comp (fst.comp fst) (fst.comp <| fst.comp snd))
+        (option_some.comp <| snd.comp <| fst.comp snd)
+        (snd.comp <| snd.comp snd)).of_eq
+  fun a ps => by
+  induction' ps with p ps ih <;> simp [List.lookup, *]
+  cases ha : a == p.1 <;> simp [ha]
+
+theorem nat_omega_rec' (f : β → σ) {m : β → ℕ} {l : β → List β} {g : β → List σ → Option σ}
+    (hm : PrimrecIn O m) (hl : PrimrecIn O l) (hg : PrimrecIn₂ O g)
+    (Ord : ∀ b, ∀ b' ∈ l b, m b' < m b)
+    (H : ∀ b, g b ((l b).map f) = some (f b)) : PrimrecIn O f := by
+  haveI : DecidableEq β := Encodable.decidableEqOfEncodable β
+  let mapGraph (M : List (β × σ)) (bs : List β) : List σ := bs.flatMap (Option.toList <| M.lookup ·)
+  let bindList (b : β) : ℕ → List β := fun n ↦ n.rec [b] fun _ bs ↦ bs.flatMap l
+  let graph (b : β) : ℕ → List (β × σ) := fun i ↦ i.rec [] fun i ih ↦
+    (bindList b (m b - i)).filterMap fun b' ↦ (g b' <| mapGraph ih (l b')).map (b', ·)
+  have mapGraph_primrec : PrimrecIn₂ O mapGraph :=
+    to₂ <| list_flatMap snd <| optionToList.comp₂ <| listLookup.comp₂ .right (fst.comp₂ .left)
+  have bindList_primrec : PrimrecIn₂ O (bindList) :=
+    nat_rec' snd
+      (list_cons.comp fst (const []))
+      (to₂ <| list_flatMap (snd.comp snd) (hl.comp₂ .right))
+  have graph_primrec : PrimrecIn₂ O (graph) :=
+    to₂ <| nat_rec' snd (const []) <|
+      to₂ <| listFilterMap
+        (bindList_primrec.comp
+          (fst.comp fst)
+          (nat_sub.comp (hm.comp <| fst.comp fst) (fst.comp snd))) <|
+            to₂ <| option_map
+              (hg.comp snd (mapGraph_primrec.comp (snd.comp <| snd.comp fst) (hl.comp snd)))
+              (PrimrecIn₂.pair.comp₂ (snd.comp₂ .left) .right)
+  have : PrimrecIn O (fun b => ((graph b (m b + 1)).get? 0).map Prod.snd) :=
+    option_map (list_get?.comp (graph_primrec.comp PrimrecIn.id (succ.comp hm)) (const 0))
+      (snd.comp₂ PrimrecIn₂.right)
+  exact option_some_iff.mp <| this.of_eq <| fun b ↦ by
+    have graph_eq_map_bindList (i : ℕ) (hi : i ≤ m b + 1) :
+        graph b i = (bindList b (m b + 1 - i)).map fun x ↦ (x, f x) := by
+      have bindList_eq_nil : bindList b (m b + 1) = [] :=
+        have bindList_m_lt (k : ℕ) : ∀ b' ∈ bindList b k, m b' < m b + 1 - k := by
+          induction' k with k ih <;> simp [bindList]
+          intro a₂ a₁ ha₁ ha₂
+          have : k ≤ m b :=
+            Nat.lt_succ.mp (by simpa using Nat.add_lt_of_lt_sub <| Nat.zero_lt_of_lt (ih a₁ ha₁))
+          have : m a₁ ≤ m b - k :=
+            Nat.lt_succ.mp (by rw [← Nat.succ_sub this]; simpa using ih a₁ ha₁)
+          exact lt_of_lt_of_le (Ord a₁ a₂ ha₂) this
+        List.eq_nil_iff_forall_not_mem.mpr
+          (by intro b' ha'; by_contra; simpa using bindList_m_lt (m b + 1) b' ha')
+      have mapGraph_graph {bs bs' : List β} (has : bs' ⊆ bs) :
+          mapGraph (bs.map <| fun x => (x, f x)) bs' = bs'.map f := by
+        induction' bs' with b bs' ih <;> simp [mapGraph]
+        · have : b ∈ bs ∧ bs' ⊆ bs := by simpa using has
+          rcases this with ⟨ha, has'⟩
+          simpa [List.lookup_graph f ha] using ih has'
+      have graph_succ : ∀ i, graph b (i + 1) =
+        (bindList b (m b - i)).filterMap fun b' =>
+          (g b' <| mapGraph (graph b i) (l b')).map (b', ·) := fun _ => rfl
+      have bindList_succ : ∀ i, bindList b (i + 1) = (bindList b i).flatMap l := fun _ => rfl
+      induction' i with i ih
+      · symm; simpa [graph] using bindList_eq_nil
+      · simp only [graph_succ, ih (Nat.le_of_lt hi), Nat.succ_sub (Nat.lt_succ.mp hi),
+          Nat.succ_eq_add_one, bindList_succ, Nat.reduceSubDiff]
+        apply List.filterMap_eq_map_iff_forall_eq_some.mpr
+        intro b' ha'; simp; rw [mapGraph_graph]
+        · exact H b'
+        · exact (List.infix_flatMap_of_mem ha' l).subset
+    simp [graph_eq_map_bindList (m b + 1) (Nat.le_refl _), bindList]
+
+theorem nat_omega_rec (f : α → β → σ) {m : α → β → ℕ}
+    {l : α → β → List β} {g : α → β × List σ → Option σ}
+    (hm : PrimrecIn₂ O m) (hl : PrimrecIn₂ O l) (hg : PrimrecIn₂ O g)
+    (Ord : ∀ a b, ∀ b' ∈ l a b, m a b' < m a b)
+    (H : ∀ a b, g a (b, (l a b).map (f a)) = some (f a b)) : PrimrecIn₂ O f :=
+  PrimrecIn₂.uncurry.mp <|
+    nat_omega_rec' (Function.uncurry f)
+      (PrimrecIn₂.uncurry.mpr hm)
+      (list_map (hl.comp fst snd) (PrimrecIn₂.pair.comp₂ (fst.comp₂ .left) .right))
+      (hg.comp₂ (fst.comp₂ .left) (PrimrecIn₂.pair.comp₂ (snd.comp₂ .left) .right))
+      (by simpa using Ord) (by simpa [Function.comp] using H)
+
+end PrimrecIn
+
+namespace Primcodable
+
+variable {α : Type*} [Primcodable α]
+
+open PrimrecIn
+
+-- /-- A subtype of a primitive recursive predicate is `Primcodable`. -/
+-- def subtype {p : α → Prop} [DecidablePred p] (hp : PrimrecInPred O p) : Primcodable (Subtype p) :=
+--   ⟨have : PrimrecIn O fun n => (@decode α _ n).bind fun a => Option.guard p a :=
+--     option_bind .decode (option_guard (hp.comp snd).to₂ snd)
+--   nat_iff.1 <| (encode_iff.2 this).of_eq fun n =>
+--     show _ = encode ((@decode α _ n).bind fun _ => _) by
+--       rcases @decode α _ n with - | a; · rfl
+--       dsimp [Option.guard]
+--       by_cases h : p a <;> simp [h]; rfl⟩
+
+-- instance fin {n} : Primcodable (Fin n) :=
+--   @ofEquiv _ _ (subtype <| nat_lt.comp .id (const n)) Fin.equivSubtype
+
+-- instance vector {n} : Primcodable (List.Vector α n) :=
+--   subtype ((@PrimrecIn.eq ℕ _ _).comp list_length (const _))
+
+-- instance finArrow {n} : Primcodable (Fin n → α) :=
+--   ofEquiv _ (Equiv.vectorEquivFin _ _).symm
+
+
+-- section ULower
+
+-- attribute [local instance] Encodable.decidableRangeEncode Encodable.decidableEqOfEncodable
+
+-- theorem mem_range_encode : PrimrecInPred O (fun n => n ∈ Set.range (encode : α → ℕ)) :=
+--   have : PrimrecInPred O fun n => Encodable.decode₂ α n ≠ none :=
+--     .not
+--       (PrimrecIn.eq.comp
+--         (.option_bind .decode
+--           (.ite (PrimrecIn.eq.comp (PrimrecIn.encode.comp .snd) .fst)
+--             (PrimrecIn.option_some.comp .snd) (.const _)))
+--         (.const _))
+--   this.of_eq fun _ => decode₂_ne_none_iff
+
+-- instance ulower : Primcodable (ULower α) :=
+--   Primcodable.subtype mem_range_encode
+
+-- end ULower
+
+end Primcodable
+
+namespace PrimrecIn
+
+-- variable {α : Type*} {β : Type*} {σ : Type*}
+-- variable [Primcodable α] [Primcodable β] [Primcodable σ]
+
+-- theorem subtype_val {p : α → Prop} [DecidablePred p] {hp : PrimrecInPred O p} :
+--     haveI := Primcodable.subtype hp
+--     PrimrecIn O (@Subtype.val α p) := by
+--   letI := Primcodable.subtype hp
+--   refine (@Primcodable.prim (Subtype p)).of_eq fun n => ?_
+--   rcases @decode (Subtype p) _ n with (_ | ⟨a, h⟩) <;> rfl
+
+-- theorem subtype_val_iff {p : β → Prop} [DecidablePred p] {hp : PrimrecInPred O p} {f : α → Subtype p} :
+--     haveI := Primcodable.subtype hp
+--     (PrimrecIn O fun a => (f a).1) ↔ PrimrecIn O f := by
+--   letI := Primcodable.subtype hp
+--   refine ⟨fun h => ?_, fun hf => subtype_val.comp hf⟩
+--   refine Nat.PrimrecIn.of_eq h fun n => ?_
+--   rcases @decode α _ n with - | a; · rfl
+--   simp; rfl
+
+-- theorem subtype_mk {p : β → Prop} [DecidablePred p] {hp : PrimrecInPred O p} {f : α → β}
+--     {h : ∀ a, p (f a)} (hf : PrimrecIn O f) :
+--     haveI := Primcodable.subtype hp
+--     PrimrecIn O fun a => @Subtype.mk β p (f a) (h a) :=
+--   subtype_val_iff.1 hf
+
+-- theorem option_get {f : α → Option β} {h : ∀ a, (f a).isSome} :
+--     PrimrecIn O f → PrimrecIn O fun a => (f a).get (h a) := by
+--   intro hf
+--   refine (Nat.PrimrecIn.pred.comp hf).of_eq fun n => ?_
+--   generalize hx : @decode α _ n = x
+--   cases x <;> simp
+
+-- theorem ulower_down : PrimrecIn O (ULower.down : α → ULower α) :=
+--   letI : ∀ a, Decidable (a ∈ Set.range (encode : α → ℕ)) := decidableRangeEncode _
+--   subtype_mk .encode
+
+-- theorem ulower_up : PrimrecIn O (ULower.up : ULower α → α) :=
+--   letI : ∀ a, Decidable (a ∈ Set.range (encode : α → ℕ)) := decidableRangeEncode _
+--   option_get (PrimrecIn.decode₂.comp subtype_val)
+
+-- theorem fin_val_iff {n} {f : α → Fin n} : (PrimrecIn O fun a => (f a).1) ↔ PrimrecIn O f := by
+--   letI : Primcodable { a // id a < n } := Primcodable.subtype (nat_lt.comp .id (const _))
+--   exact (Iff.trans (by rfl) subtype_val_iff).trans (of_equiv_iff _)
+
+-- theorem fin_val {n} : PrimrecIn O (fun (i : Fin n) => (i : ℕ)) :=
+--   fin_val_iff.2 .id
+
+-- theorem fin_succ {n} : PrimrecIn O (@Fin.succ n) :=
+--   fin_val_iff.1 <| by simp [succ.comp fin_val]
+
+-- theorem vector_toList {n} : PrimrecIn O (@List.Vector.toList α n) :=
+--   subtype_val
+
+-- theorem vector_toList_iff {n} {f : α → List.Vector β n} :
+--     (PrimrecIn O fun a => (f a).toList) ↔ PrimrecIn O f :=
+--   subtype_val_iff
+
+-- theorem vector_cons {n} : PrimrecIn₂ O (@List.Vector.cons α n) :=
+--   vector_toList_iff.1 <| by simpa using list_cons.comp fst (vector_toList_iff.2 snd)
+
+-- theorem vector_length {n} : PrimrecIn O (@List.Vector.length α n) :=
+--   const _
+
+-- theorem vector_head {n} : PrimrecIn O (@List.Vector.head α n) :=
+--   option_some_iff.1 <| (list_head?.comp vector_toList).of_eq fun ⟨_ :: _, _⟩ => rfl
+
+-- theorem vector_tail {n} : PrimrecIn O (@List.Vector.tail α n) :=
+--   vector_toList_iff.1 <| (list_tail.comp vector_toList).of_eq fun ⟨l, h⟩ => by cases l <;> rfl
+
+-- theorem vector_get {n} : PrimrecIn₂ O (@List.Vector.get α n) :=
+--   option_some_iff.1 <|
+--     (list_get?.comp (vector_toList.comp fst) (fin_val.comp snd)).of_eq fun a => by
+--       rw [Vector.get_eq_get_toList, ← List.get?_eq_get]
+--       rfl
+
+-- theorem list_ofFn :
+--     ∀ {n} {f : Fin n → α → σ}, (∀ i, PrimrecIn O (f i)) → PrimrecIn O fun a => List.ofFn fun i => f i a
+--   | 0, _, _ => by simp only [List.ofFn_zero]; exact const []
+--   | n + 1, f, hf => by
+--     simpa [List.ofFn_succ] using list_cons.comp (hf 0) (list_ofFn fun i => hf i.succ)
+
+-- theorem vector_ofFn {n} {f : Fin n → α → σ} (hf : ∀ i, PrimrecIn O (f i)) :
+--     PrimrecIn O fun a => List.Vector.ofFn fun i => f i a :=
+--   vector_toList_iff.1 <| by simp [list_ofFn hf]
+
+-- theorem vector_get' {n} : PrimrecIn O (@List.Vector.get α n) :=
+--   of_equiv_symm
+
+-- theorem vector_ofFn' {n} : PrimrecIn O (@List.Vector.ofFn α n) :=
+--   of_equiv
+
+-- theorem fin_app {n} : PrimrecIn₂ O (@id (Fin n → σ)) :=
+--   (vector_get.comp (vector_ofFn'.comp fst) snd).of_eq fun ⟨v, i⟩ => by simp
+
+-- theorem fin_curry₁ {n} {f : Fin n → α → σ} : PrimrecIn₂ O f ↔ ∀ i, PrimrecIn O (f i) :=
+--   ⟨fun h i => h.comp (const i) .id, fun h =>
+--     (vector_get.comp ((vector_ofFn h).comp snd) fst).of_eq fun a => by simp⟩
+
+-- theorem fin_curry {n} {f : α → Fin n → σ} : PrimrecIn O f ↔ PrimrecIn₂ O f :=
+--   ⟨fun h => fin_app.comp (h.comp fst) snd, fun h =>
+--     (vector_get'.comp
+--           (vector_ofFn fun i => show PrimrecIn O fun a => f a i from h.comp .id (const i))).of_eq
+--       fun a => by funext i; simp⟩
+
+-- end PrimrecIn O
+
+-- namespace Nat
+
+-- open List.Vector
+
+-- /-- An alternative inductive definition of `PrimrecIn O` which
+--   does not use the pairing function on ℕ, and so has to
+--   work with n-ary functions on ℕ instead of unary functions.
+--   We prove that this is equivalent to the regular notion
+--   in `to_prim` and `of_prim`. -/
+-- inductive PrimrecIn O' : ∀ {n}, (List.Vector ℕ n → ℕ) → Prop
+--   | zero : @PrimrecIn O' 0 fun _ => 0
+--   | succ : @PrimrecIn O' 1 fun v => succ v.head
+--   | get {n} (i : Fin n) : PrimrecIn O' fun v => v.get i
+--   | comp {m n f} (g : Fin n → List.Vector ℕ m → ℕ) :
+--       PrimrecIn O' f → (∀ i, PrimrecIn O' (g i)) → PrimrecIn O' fun a => f (List.Vector.ofFn fun i => g i a)
+--   | prec {n f g} :
+--       @PrimrecIn O' n f →
+--         @PrimrecIn O' (n + 2) g →
+--           PrimrecIn O' fun v : List.Vector ℕ (n + 1) =>
+--             v.head.rec (f v.tail) fun y IH => g (y ::ᵥ IH ::ᵥ v.tail)
+
+-- end Nat
+
+-- namespace Nat.PrimrecIn O'
+
+-- open List.Vector PrimrecIn O
+
+-- theorem to_prim {n f} (pf : @Nat.PrimrecIn O' n f) : PrimrecIn O f := by
+--   induction pf with
+--   | zero => exact .const 0
+--   | succ => exact _root_.PrimrecIn.succ.comp .vector_head
+--   | get i => exact PrimrecIn.vector_get.comp .id (.const i)
+--   | comp _ _ _ hf hg => exact hf.comp (.vector_ofFn fun i => hg i)
+--   | @prec n f g _ _ hf hg =>
+--     exact
+--       .nat_rec' .vector_head (hf.comp PrimrecIn.vector_tail)
+--         (hg.comp <|
+--           PrimrecIn.vector_cons.comp (PrimrecIn.fst.comp .snd) <|
+--           PrimrecIn.vector_cons.comp (PrimrecIn.snd.comp .snd) <|
+--             (@PrimrecIn.vector_tail _ _ (n + 1)).comp .fst).to₂
+
+-- theorem of_eq {n} {f g : List.Vector ℕ n → ℕ} (hf : PrimrecIn O' f) (H : ∀ i, f i = g i) :
+--     PrimrecIn O' g :=
+--   (funext H : f = g) ▸ hf
+
+-- theorem const {n} : ∀ m, @PrimrecIn O' n fun _ => m
+--   | 0 => zero.comp Fin.elim0 fun i => i.elim0
+--   | m + 1 => succ.comp _ fun _ => const m
+
+-- theorem head {n : ℕ} : @PrimrecIn O' n.succ head :=
+--   (get 0).of_eq fun v => by simp [get_zero]
+
+-- theorem tail {n f} (hf : @PrimrecIn O' n f) : @PrimrecIn O' n.succ fun v => f v.tail :=
+--   (hf.comp _ fun i => @get _ i.succ).of_eq fun v => by
+--     rw [← ofFn_get v.tail]; congr; funext i; simp
+
+-- /-- A function from vectors to vectors is primitive recursive when all of its projections are. -/
+-- def Vec {n m} (f : List.Vector ℕ n → List.Vector ℕ m) : Prop :=
+--   ∀ i, PrimrecIn O' fun v => (f v).get i
+
+-- protected theorem nil {n} : @Vec n 0 fun _ => nil := fun i => i.elim0
+
+-- protected theorem cons {n m f g} (hf : @PrimrecIn O' n f) (hg : @Vec n m g) :
+--     Vec fun v => f v ::ᵥ g v := fun i => Fin.cases (by simp [*]) (fun i => by simp [hg i]) i
+
+-- theorem idv {n} : @Vec n n id :=
+--   get
+
+-- theorem comp' {n m f g} (hf : @PrimrecIn O' m f) (hg : @Vec n m g) : PrimrecIn O' fun v => f (g v) :=
+--   (hf.comp _ hg).of_eq fun v => by simp
+
+-- theorem comp₁ (f : ℕ → ℕ) (hf : @PrimrecIn O' 1 fun v => f v.head) {n g} (hg : @PrimrecIn O' n g) :
+--     PrimrecIn O' fun v => f (g v) :=
+--   hf.comp _ fun _ => hg
+
+-- theorem comp₂ (f : ℕ → ℕ → ℕ) (hf : @PrimrecIn O' 2 fun v => f v.head v.tail.head) {n g h}
+--     (hg : @PrimrecIn O' n g) (hh : @PrimrecIn O' n h) : PrimrecIn O' fun v => f (g v) (h v) := by
+--   simpa using hf.comp' (hg.cons <| hh.cons PrimrecIn O'.nil)
+
+-- theorem prec' {n f g h} (hf : @PrimrecIn O' n f) (hg : @PrimrecIn O' n g) (hh : @PrimrecIn O' (n + 2) h) :
+--     @PrimrecIn O' n fun v => (f v).rec (g v) fun y IH : ℕ => h (y ::ᵥ IH ::ᵥ v) := by
+--   simpa using comp' (prec hg hh) (hf.cons idv)
+
+-- theorem pred : @PrimrecIn O' 1 fun v => v.head.pred :=
+--   (prec' head (const 0) head).of_eq fun v => by simp; cases v.head <;> rfl
+
+-- theorem add : @PrimrecIn O' 2 fun v => v.head + v.tail.head :=
+--   (prec head (succ.comp₁ _ (tail head))).of_eq fun v => by
+--     simp; induction v.head <;> simp [*, Nat.succ_add]
+
+-- theorem sub : @PrimrecIn O' 2 fun v => v.head - v.tail.head := by
+--   have : @PrimrecIn O' 2 fun v ↦ (fun a b ↦ b - a) v.head v.tail.head := by
+--     refine (prec head (pred.comp₁ _ (tail head))).of_eq fun v => ?_
+--     simp; induction v.head <;> simp [*, Nat.sub_add_eq]
+--   simpa using comp₂ (fun a b => b - a) this (tail head) head
+
+-- theorem mul : @PrimrecIn O' 2 fun v => v.head * v.tail.head :=
+--   (prec (const 0) (tail (add.comp₂ _ (tail head) head))).of_eq fun v => by
+--     simp; induction v.head <;> simp [*, Nat.succ_mul]; rw [add_comm]
+
+-- theorem if_lt {n a b f g} (ha : @PrimrecIn O' n a) (hb : @PrimrecIn O' n b) (hf : @PrimrecIn O' n f)
+--     (hg : @PrimrecIn O' n g) : @PrimrecIn O' n fun v => if a v < b v then f v else g v :=
+--   (prec' (sub.comp₂ _ hb ha) hg (tail <| tail hf)).of_eq fun v => by
+--     cases e : b v - a v
+--     · simp [not_lt.2 (Nat.sub_eq_zero_iff_le.mp e)]
+--     · simp [Nat.lt_of_sub_eq_succ e]
+
+-- theorem natPair : @PrimrecIn O' 2 fun v => v.head.pair v.tail.head :=
+--   if_lt head (tail head) (add.comp₂ _ (tail <| mul.comp₂ _ head head) head)
+--     (add.comp₂ _ (add.comp₂ _ (mul.comp₂ _ head head) head) (tail head))
+
+-- protected theorem encode : ∀ {n}, @PrimrecIn O' n encode
+--   | 0 => (const 0).of_eq fun v => by rw [v.eq_nil]; rfl
+--   | _ + 1 =>
+--     (succ.comp₁ _ (natPair.comp₂ _ head (tail PrimrecIn O'.encode))).of_eq fun ⟨_ :: _, _⟩ => rfl
+
+-- theorem sqrt : @PrimrecIn O' 1 fun v => v.head.sqrt := by
+--   suffices H : ∀ n : ℕ, n.sqrt =
+--       n.rec 0 fun x y => if x.succ < y.succ * y.succ then y else y.succ by
+--     simp only [H, succ_eq_add_one]
+--     have :=
+--       @prec' 1 _ _
+--         (fun v => by
+--           have x := v.head; have y := v.tail.head
+--           exact if x.succ < y.succ * y.succ then y else y.succ)
+--         head (const 0) ?_
+--     · exact this
+--     have x1 : @PrimrecIn O' 3 fun v => v.head.succ := succ.comp₁ _ head
+--     have y1 : @PrimrecIn O' 3 fun v => v.tail.head.succ := succ.comp₁ _ (tail head)
+--     exact if_lt x1 (mul.comp₂ _ y1 y1) (tail head) y1
+--   introv; symm
+--   induction' n with n IH; · simp
+--   dsimp; rw [IH]; split_ifs with h
+--   · exact le_antisymm (Nat.sqrt_le_sqrt (Nat.le_succ _)) (Nat.lt_succ_iff.1 <| Nat.sqrt_lt.2 h)
+--   · exact
+--       Nat.eq_sqrt.2 ⟨not_lt.1 h, Nat.sqrt_lt.1 <| Nat.lt_succ_iff.2 <| Nat.sqrt_succ_le_succ_sqrt _⟩
+
+-- theorem unpair₁ {n f} (hf : @PrimrecIn O' n f) : @PrimrecIn O' n fun v => (f v).unpair.1 := by
+--   have s := sqrt.comp₁ _ hf
+--   have fss := sub.comp₂ _ hf (mul.comp₂ _ s s)
+--   refine (if_lt fss s fss s).of_eq fun v => ?_
+--   simp [Nat.unpair]; split_ifs <;> rfl
+
+-- theorem unpair₂ {n f} (hf : @PrimrecIn O' n f) : @PrimrecIn O' n fun v => (f v).unpair.2 := by
+--   have s := sqrt.comp₁ _ hf
+--   have fss := sub.comp₂ _ hf (mul.comp₂ _ s s)
+--   refine (if_lt fss s s (sub.comp₂ _ fss s)).of_eq fun v => ?_
+--   simp [Nat.unpair]; split_ifs <;> rfl
+
+-- theorem of_prim {n f} : PrimrecIn O f → @PrimrecIn O' n f :=
+--   suffices ∀ f, Nat.PrimrecIn O f → @PrimrecIn O' 1 fun v => f v.head from fun hf =>
+--     (pred.comp₁ _ <|
+--           (this _ hf).comp₁ (fun m => Encodable.encode <| (@decode (List.Vector ℕ n) _ m).map f)
+--             PrimrecIn O'.encode).of_eq
+--       fun i => by simp [encodek]
+--   fun f hf => by
+--   induction hf with
+--   | zero => exact const 0
+--   | succ => exact succ
+--   | left => exact unpair₁ head
+--   | right => exact unpair₂ head
+--   | pair _ _ hf hg => exact natPair.comp₂ _ hf hg
+--   | comp _ _ hf hg => exact hf.comp₁ _ hg
+--   | prec _ _ hf hg =>
+--     simpa using
+--       prec' (unpair₂ head) (hf.comp₁ _ (unpair₁ head))
+--         (hg.comp₁ _ <|
+--           natPair.comp₂ _ (unpair₁ <| tail <| tail head) (natPair.comp₂ _ head (tail head)))
+
+-- theorem prim_iff {n f} : @PrimrecIn O' n f ↔ PrimrecIn O f :=
+--   ⟨to_prim, of_prim⟩
+
+-- theorem prim_iff₁ {f : ℕ → ℕ} : (@PrimrecIn O' 1 fun v => f v.head) ↔ PrimrecIn O f :=
+--   prim_iff.trans
+--     ⟨fun h => (h.comp <| .vector_ofFn fun _ => .id).of_eq fun v => by simp, fun h =>
+--       h.comp .vector_head⟩
+
+-- theorem prim_iff₂ {f : ℕ → ℕ → ℕ} : (@PrimrecIn O' 2 fun v => f v.head v.tail.head) ↔ PrimrecIn₂ O f :=
+--   prim_iff.trans
+--     ⟨fun h => (h.comp <| PrimrecIn.vector_cons.comp .fst <|
+--       PrimrecIn.vector_cons.comp .snd (.const nil)).of_eq fun v => by simp,
+--     fun h => h.comp .vector_head (PrimrecIn.vector_head.comp .vector_tail)⟩
+
+-- theorem vec_iff {m n f} : @Vec m n f ↔ PrimrecIn O f :=
+--   ⟨fun h => by simpa using PrimrecIn.vector_ofFn fun i => to_prim (h i), fun h i =>
+--     of_prim <| PrimrecIn.vector_get.comp h (.const i)⟩
+
+-- end Nat.PrimrecIn O'
+
+-- theorem PrimrecIn.nat_sqrt : PrimrecIn O Nat.sqrt :=
+--   Nat.PrimrecIn O'.prim_iff₁.1 Nat.PrimrecIn O'.sqrt
