Computability/SingleOracle/hy.lean
@@ -1,3 +1,6 @@
+-- import Computability.SingleOracle.Encoding2
+import Computability.SingleOracle.Encoding
+-- import Computability.SingleOracle.Oracle2
 -- some theorems that'd be nice:
 -- 1. K_0 =_T K
 -- 2. characterising the c.e. sets as domains of partial functions is equivalent to characterising them as ranges of partial functions
@@ -6,3 +9,9 @@
 -- there exists an infinite set having no infinite recursively enumerable subset. (problem 5.8 ToRFaEC)
 
 -- THEOREM 10.3.5 of /mnt/Q/Mathematics/Textbooks/Computability/Computability Theory [Cooper] (2004).pdf
+
+open Nat.OracleComp.Code
+open Classical
+
+noncomputable
+def jumpConst (O:ℕ→ℕ) : (ℕ→Option ℕ) := fun x => (evalo O x x).toOption
